examples/formal-languages/regular/regularScript.sml
@@ -1,38 +1,96 @@
 (*===========================================================================*)
-(* Basic automata theory: dfas, nfas, their equivalence via the subset       *)
-(* construction, further closure constructions, regular expressions,         *)
-(* equivalence of regexps and automata, pumping lemma, Myhill-Nerode,        *)
-(* minimization, etc.                                                        *)
+(* Basic automata theory: nfas, dfas, their equivalence via the subset       *)
+(* construction, closure constructions, etc. The approach taken is           *)
+(* set-oriented, rather than computational.                                  *)
 (*===========================================================================*)
 
 open HolKernel Parse boolLib bossLib;
-open combinTheory
-     listTheory
-     mp_then
-     nlistTheory
-     numpairTheory
-     pred_setTheory
-     relationTheory
-     rich_listTheory
-     arithmeticTheory
-     FormalLangTheory;
+open combinTheory pairTheory listTheory
+     mp_then nlistTheory numpairTheory
+     pred_setTheory relationTheory
+     rich_listTheory prim_recTheory
+     arithmeticTheory FormalLangTheory;
 
 infix byA;
 val op byA = BasicProvers.byA;
 
 val subst_all_tac = SUBST_ALL_TAC
+val sym_subst_all_tac = SUBST_ALL_TAC o SYM
 val pop_subst_tac = pop_assum subst_all_tac;
+val pop_sym_subst_tac = pop_assum sym_subst_all_tac;
+val pop_keep_tac = pop_assum mp_tac
+val qpat_keep_tac = Lib.C qpat_x_assum mp_tac;
 val pop_forget_tac = pop_assum kall_tac
-val qpat_weaken_tac = Lib.C qpat_x_assum kall_tac;
-val weaken_tac = WEAKEN_TAC
+val qpat_forget_tac = Lib.C qpat_x_assum kall_tac;
+val forget_tac = WEAKEN_TAC
 
 fun obtain_then q tac ttac = ttac (Q.prove(q,tac))
+
+val PUSH_EXISTS = LIST_CONJ
+  [GSYM RIGHT_OR_EXISTS_THM,
+   GSYM LEFT_OR_EXISTS_THM,
+   RIGHT_EXISTS_IMP_THM,
+   RIGHT_EXISTS_AND_THM,
+   LEFT_EXISTS_IMP_THM,
+   LEFT_EXISTS_AND_THM,
+   EXISTS_OR_THM];
 
 
 val _ = new_theory "regular";
 
+(* NOTE: duplicate theorems:
+
+pred_setTheory.in_max_set (THEOREM)
+-----------------------------------
+⊢ ∀s. FINITE s ⇒ ∀x. x ∈ s ⇒ x ≤ MAX_SET s
+
+pred_setTheory.X_LE_MAX_SET (THEOREM)
+-------------------------------------
+⊢ ∀s. FINITE s ⇒ ∀x. x ∈ s ⇒ x ≤ MAX_SET s
+*)
+
 (*---------------------------------------------------------------------------*)
-(* Local lemmas, possibly of wider use                                       *)
+(* Local lemmas, possibly of wider use. Start with sets                      *)
+(*---------------------------------------------------------------------------*)
+
+Theorem SUBSET_SKOLEM_THM :
+  (!x. P x ==> ?y. Q x y) <=> ?f. !x. P x ==> Q x (f x)
+Proof
+ metis_tac[]
+QED
+
+Triviality SUBSET_UNION_RIGHT:
+ x ⊆ y ⇒ x ⊆ y ∪ z
+Proof
+  rw[SUBSET_DEF]
+QED
+
+Triviality UNION_EQ_DIFF:
+ A ∪ B = C ⇒ A DIFF B = C DIFF B
+Proof
+  rw [EXTENSION] >> metis_tac[]
+QED
+
+Triviality DIFF_EQ_UNION:
+ A DIFF B = C ⇒ A ∪ B = C ∪ B
+Proof
+  rw [EXTENSION] >> metis_tac[]
+QED
+
+Theorem SET_TO_LIST_11[simp]:
+  ∀s1 s2. FINITE s1 ∧ FINITE s2 ⇒ (SET_TO_LIST s1 = SET_TO_LIST s2 ⇔ s1 = s2)
+Proof
+  metis_tac[listTheory.SET_TO_LIST_INV]
+QED
+
+Theorem MAX_SET_BOUNDED:
+  FINITE s ∧ MAX_SET s < n ⇒ n ∉ s
+Proof
+ rw[] >> spose_not_then assume_tac >> drule_all X_LE_MAX_SET >> decide_tac
+QED
+
+(*---------------------------------------------------------------------------*)
+(* List destructors: HD, TL, and LAST                                        *)
 (*---------------------------------------------------------------------------*)
 
 Triviality HD_APPEND[simp]:
@@ -53,17 +111,167 @@ Proof
   Cases >> rw[FRONT_DEF]
 QED
 
+Triviality HD_MAP[simp]:
+ l ≠ [] ⇒ HD (MAP f l) = f (HD l)
+Proof
+ Cases_on ‘l’ >> rw[]
+QED
+
+Triviality TL_APPEND[simp]:
+ ∀l1 l2. l1 ≠ [] ⇒ TL (l1 ++ l2) = TL l1 ++ l2
+Proof
+ Cases >> rw[]
+QED
+
+Triviality LAST_MAP[simp]:
+ l ≠ [] ⇒ LAST (MAP f l) = f (LAST l)
+Proof
+ Cases_on ‘l’ >> rw[]
+QED
+
+Triviality LAST_TL[simp]:
+  ∀l. TL l ≠ [] ⇒ LAST (TL l) = LAST l
+Proof
+ Cases >> rw[LAST_DEF]
+QED
+
+Triviality EL_TL[simp]:
+  ∀l. l ≠ [] ⇒ EL n (TL l) = EL (n+1) l
+Proof
+ Cases >> rw[GSYM ADD1]
+QED
+
+Triviality LENGTH_TL_ALT:
+ n < LENGTH l ⇒ LENGTH (TL l) = LENGTH l − 1
+Proof
+ rw [LENGTH_TL]
+QED
+
 Triviality LESS_FRONT_LENGTH[simp]:
  ∀l n. 0 < n ∧ n < LENGTH l ⇒ n-1 < LENGTH (FRONT l)
 Proof
   Cases >> rw[FRONT_DEF]
 QED
 
-Triviality EVERY_LAST:
-  ∀list. list ≠ [] ∧ EVERY P list ⇒ P (LAST list)
+(*---------------------------------------------------------------------------*)
+(* EXISTS and EVERY                                                          *)
+(*---------------------------------------------------------------------------*)
+
+Theorem EXISTS_EL:
+  EXISTS P l ⇔ ∃n. n < LENGTH l ∧ P (EL n l)
 Proof
- Induct >> rw[LAST_DEF]
+  Induct_on ‘l’ >> rw[] >> pop_forget_tac >> rw[EQ_IMP_THM]
+  >- (irule_at Any (DECIDE “0 < SUC n”) >> rw[])
+  >- (‘SUC n < SUC (LENGTH l)’ by decide_tac >>
+      first_x_assum (irule_at Any) >> rw[])
+  >- (Cases_on ‘n’ >> fs[] >> metis_tac[])
 QED
+
+Theorem EVERY_LAST:
+  list ≠ [] ∧ EVERY P list ⇒ P (LAST list)
+Proof
+ rw[EVERY_EL,LAST_EL] >> fs[NOT_NIL_EQ_LENGTH_NOT_0]
+QED
+
+Theorem EVERY_HD:
+  list ≠ [] ∧ EVERY P list ⇒ P (HD list)
+Proof
+ rw[EVERY_EL] >> metis_tac [EL,NOT_NIL_EQ_LENGTH_NOT_0]
+QED
+
+Triviality EVERY_TL:
+  l ≠ [] ∧ EVERY P l ⇒ EVERY P (TL l)
+Proof
+ Cases_on ‘l’ >> rw[]
+QED
+
+Theorem EVERY_DISJ_LEFT:
+  ∀P Q l. EVERY P l ⇒ EVERY (λx. P x ∨ Q x) l
+Proof
+  Induct_on ‘l’ >> rw[]
+QED
+
+Theorem EVERY_DISJ_RIGHT:
+  ∀P Q l. EVERY Q l ⇒ EVERY (λx. P x ∨ Q x) l
+Proof
+  Induct_on ‘l’ >> rw[]
+QED
+
+Triviality POS_LENGTH_NOT_NIL:
+  n < LENGTH list ⇒ list ≠ []
+Proof
+ Cases_on ‘list’ >> rw[]
+QED
+
+(*---------------------------------------------------------------------------*)
+(* FLAT                                                                      *)
+(*---------------------------------------------------------------------------*)
+
+Triviality FLAT_NOT_NIL:
+  ll ≠ [] ∧ LAST ll ≠ [] ⇒ FLAT ll ≠ []
+Proof
+  rw [FLAT_EQ_NIL,o_DEF,EXISTS_EL] >> rfs [LAST_EL] >>
+  first_x_assum (irule_at Any) >> fs[NOT_NIL_EQ_LENGTH_NOT_0]
+QED
+
+Theorem HD_FLAT:
+  ll ≠ [] ∧ HD ll ≠ []
+  ⇒
+  HD (FLAT ll) = HD (HD ll)
+Proof
+  Cases_on ‘ll’ >> rw[]
+QED
+
+Theorem LAST_FLAT:
+  ll ≠ [] ∧ LAST ll ≠ []
+  ⇒
+  LAST (FLAT ll) = LAST(LAST ll)
+Proof
+  Induct_on ‘ll’ >> rw[LAST_DEF] >> fs[] >>
+  drule FLAT_NOT_NIL >> rw[LAST_APPEND_NOT_NIL,LAST_DEF]
+QED
+
+(*---------------------------------------------------------------------------*)
+(* EL                                                                        *)
+(*---------------------------------------------------------------------------*)
+
+Theorem EL_APPEND2_ALT:
+  (n < LENGTH L2 ==> EL (LENGTH L1 + n) (L1 ++ L2) = EL n L2) ∧
+  (n < LENGTH L2 ==> EL (n + LENGTH L1) (L1 ++ L2) = EL n L2)
+Proof
+  rw [EL_APPEND_EQN]
+QED
+
+Triviality EL_LENGTH_LAST:
+ ∀l1 l2. LENGTH l1 = LENGTH l2 + 1 ⇒ EL (LENGTH l2) l1 = LAST l1
+Proof
+ ho_match_mp_tac SNOC_INDUCT >> rw[ADD1] >>
+ pop_assum (SUBST_ALL_TAC o GSYM) >> rw [EL_LENGTH_SNOC]
+QED
+
+Triviality LAST_MAP2:
+  ∀l1 l2 f.
+    l1 ≠ [] ∧ l2 ≠ [] ∧ LENGTH l1 = LENGTH l2
+    ⇒ LAST (MAP2 f l1 l2) = f (LAST l1) (LAST l2)
+Proof
+  rw[] >>
+  ‘MAP2 f l1 l2 ≠ []’ by (map_every Cases_on [‘l1’, ‘l2’] >> fs[]) >>
+  rw [LAST_EL] >> irule EL_MAP2 >> Cases_on ‘l2’ >> fs[]
+QED
+
+Triviality snoc2:
+ ∀list n. LENGTH list = n+2 ⇒ ∃z f. list = SNOC z f ∧ f ≠ []
+Proof
+  rpt strip_tac >> Cases_on ‘list = []’
+  >- fs[]
+  >- (drule SNOC_LAST_FRONT >> Cases_on ‘FRONT list = []’
+      >- (Cases_on ‘list’ >> fs[])
+      >- metis_tac [])
+QED
+
+(*---------------------------------------------------------------------------*)
+(* KSTAR and RTC                                                             *)
+(*---------------------------------------------------------------------------*)
 
 Theorem KSTAR_FLAT:
   KSTAR L = {FLAT ls | ∀w. MEM w ls ⇒ w ∈ L}
@@ -114,14 +322,8 @@ Proof
   metis_tac [RTC_LIST_LR, RTC_LIST_RL]
 QED
 
-Theorem SET_TO_LIST_11[simp]:
-  ∀s1 s2. FINITE s1 ∧ FINITE s2 ⇒ (SET_TO_LIST s1 = SET_TO_LIST s2 ⇔ s1 = s2)
-Proof
-  metis_tac[listTheory.SET_TO_LIST_INV]
-QED
-
 (*---------------------------------------------------------------------------*)
-(* Non-deterministic finite state automata (NFAs).                           *)
+(* Basic type abbreviations                                                  *)
 (*---------------------------------------------------------------------------*)
 
 Type state  = “:num”
@@ -129,13 +331,17 @@ Type symbol = “:num”
 Type word   = “:symbol list”
 Type language = “:word set”
 
+(*---------------------------------------------------------------------------*)
+(* Non-deterministic finite state automata (NFAs).                           *)
+(*---------------------------------------------------------------------------*)
+
 Datatype:
   nfa = <|
     Q : state set ;
     Sigma : symbol set ;
     delta : state -> symbol -> state set;
     initial : state set;
-    acceptors : state set
+    final : state set
   |>
 End
 
@@ -144,9 +350,19 @@ Definition wf_nfa_def:
     FINITE N.Q ∧
     FINITE N.Sigma ∧
     N.initial ⊆ N.Q ∧
-    N.acceptors ⊆ N.Q ∧
+    N.final ⊆ N.Q ∧
     (∀q a. a ∈ N.Sigma ∧ q ∈ N.Q ⇒ N.delta q a ⊆ N.Q)
 End
+
+Theorem finite_nfa_successors:
+ wf_nfa N ⇒
+  ∀eq a. s ⊆ N.Q ∧ a ∈ N.Sigma ==> FINITE (BIGUNION {N.delta q a | q ∈ s})
+Proof
+  rw [] >>
+  ‘FINITE s’ by metis_tac [SUBSET_FINITE,wf_nfa_def]
+  >- (fs[GSPEC_IMAGE,o_DEF,IN_DEF] >> metis_tac [IMAGE_FINITE])
+  >- (fs [wf_nfa_def] >> metis_tac [SUBSET_FINITE,SUBSET_DEF])
+QED
 
 (*---------------------------------------------------------------------------*)
 (* A deterministic finite state automaton (DFA) is an NFA with a single      *)
@@ -155,22 +371,24 @@ End
 (*---------------------------------------------------------------------------*)
 
 Definition is_dfa_def:
-  is_dfa N ⇔ wf_nfa N ∧ (∃q_0. N.initial = {q_0}) ∧
-             (∀q a. q ∈ N.Q ∧ a ∈ N.Sigma ⇒ ∃q'. N.delta q a = {q'})
+  is_dfa N ⇔
+    wf_nfa N ∧
+    (∃q_0. N.initial = {q_0}) ∧
+    (∀q a. q ∈ N.Q ∧ a ∈ N.Sigma ⇒ ∃q'. N.delta q a = {q'})
 End
 
-(*
+(*---------------------------------------------------------------------------
+
                                            /-----------\
                                            v           |
-   --> ( 1 )  --a-->  (( 2 ))  --a,b-->  ( 4 )  --a,b -'
+   --> ( 1 )  --a-->  (( 2 ))  --a,b-->  ( 4 ) --a,b --'
          |                                 ^
          b                                 |
          |                                 |
-         \______________a,b________________/
+         V______________a,b________________/
        ( 3 )
 
-
-*)
+ ---------------------------------------------------------------------------*)
 
 Definition example_dfa_def:
   example_dfa =
@@ -184,7 +402,7 @@ Definition example_dfa_def:
               | 4 => (λc. if (c = 1) \/ (c = 2) then {4} else {0})
               | _ => \c.{0} ) ;
       initial := {1};
-      acceptors := {2} |>
+      final := {2} |>
 End
 
 Theorem example_dfa_wellformed:
@@ -195,39 +413,43 @@ QED
 
 
 (*---------------------------------------------------------------------------*)
+(* There's a coercion between symbols in the alphabet and the words needed   *)
+(* for application of KSTAR                                                  *)
+(*---------------------------------------------------------------------------*)
+
+Definition Symbol_Word_def[simp]:
+  Symbol_Word a = [a]
+End
+
+Triviality KSTAR_Symbols[simp]:
+  ∀w. w ∈ KSTAR (IMAGE Symbol_Word symbols) <=> EVERY (λa. a ∈ symbols) w
+Proof
+  Induct >> simp [Once IN_KSTAR_THM] >> rw [EQ_IMP_THM,PULL_EXISTS]
+QED
+
+(*---------------------------------------------------------------------------*)
 (* NFA acceptance                                                            *)
 (*---------------------------------------------------------------------------*)
 
 Definition nfa_lang_def:
   nfa_lang N =
-   {w | w ∈ KSTAR (IMAGE (λa. [a]) N.Sigma) ∧
+   {w | w ∈ KSTAR (IMAGE Symbol_Word N.Sigma) ∧
         ∃qs. LENGTH qs = LENGTH w + 1 ∧
              HD qs ∈ N.initial ∧
-             LAST qs ∈ N.acceptors ∧
+             LAST qs ∈ N.final ∧
          (∀n. n < LENGTH w ⇒ EL (n + 1) qs ∈ N.delta (EL n qs) (EL n w))}
 End
 
 Theorem in_nfa_lang:
  w ∈ nfa_lang N
   <=>
- w ∈ KSTAR (IMAGE (λa. [a]) N.Sigma) ∧
+ w ∈ KSTAR (IMAGE Symbol_Word N.Sigma) ∧
  ∃qs. LENGTH qs = LENGTH w + 1 ∧
           HD qs ∈ N.initial ∧
-        LAST qs ∈ N.acceptors ∧
+        LAST qs ∈ N.final ∧
        (∀n. n < LENGTH w ⇒ EL (n + 1) qs ∈ N.delta (EL n qs) (EL n w))
 Proof
  rw [nfa_lang_def]
-QED
-
-(*---------------------------------------------------------------------------*)
-(* There's a coercion between symbols in the alphabet and the words needed   *)
-(* for application of KSTAR                                                  *)
-(*---------------------------------------------------------------------------*)
-
-Triviality KSTAR_SIGMA[simp]:
-  ∀w. w ∈ KSTAR (IMAGE (λa. [a]) sigma) <=> EVERY (λa. a ∈ sigma) w
-Proof
-  Induct >> simp [Once IN_KSTAR_THM] >> rw [EQ_IMP_THM,PULL_EXISTS]
 QED
 
 (*---------------------------------------------------------------------------*)
@@ -282,54 +504,349 @@ Proof
 QED
 
 (*---------------------------------------------------------------------------*)
+(* Basics for NFAs and DFAs. It's often neater to base the proofs on the     *)
+(* notion of an execution, a generalization of the notion of *accepting      *)
+(* execution* used to characterize NFA languages.                            *)
+(*---------------------------------------------------------------------------*)
+
+Definition is_exec_def :
+ is_exec N qs w ⇔
+   EVERY (λa. a ∈ N.Sigma) w ∧
+   LENGTH qs = LENGTH w + 1 ∧
+   HD qs ∈ N.Q ∧
+   (∀n. n < LENGTH w ⇒ EL (n+1) qs ∈ N.delta (EL n qs) (EL n w))
+End
+
+(* This should be a theorem
+Definition is_exec_rec_def:
+   is_exec_rec N [q] [] = (q ∈ N.Q) ∧
+   is_exec_rec N (q1::q2::t) (a::w) =
+     (q1 ∈ N.Q ∧ q2 ∈ N.Q ∧
+      q2 ∈ N.delta q1 a ∧
+      is_exec_rec N (q2::t) w)
+   ∧
+   is_exec_rec N [] w = F ∧
+   is_exec_rec N [q] (a::w) = F ∧
+   is_exec_rec N (q1::q2::t) [] = F
+End
+*)
+
+Definition is_accepting_exec_def :
+ is_accepting_exec N qs w
+  ⇔
+ is_exec N qs w ∧ HD qs ∈ N.initial ∧ LAST qs ∈ N.final
+End
+
+Theorem in_nfa_lang_is_exec:
+  wf_nfa N ∧ w ∈ nfa_lang N ⇒ ∃qs. is_exec N qs w
+Proof
+ rw [is_exec_def,in_nfa_lang,wf_nfa_def] >> metis_tac [SUBSET_DEF]
+QED
+
+Theorem in_nfa_lang_is_accepting_exec:
+  wf_nfa N ∧ w ∈ nfa_lang N
+  ⇒
+  ∃qs. is_accepting_exec N qs w ∧ ~NULL qs
+Proof
+  rw [is_accepting_exec_def,is_exec_def,in_nfa_lang,wf_nfa_def] >>
+  ‘~NULL qs’ by (Cases_on ‘qs’ >> fs[]) >>
+  metis_tac [SUBSET_DEF]
+QED
+
+Theorem in_nfa_lang_iff_accepting_exec:
+  wf_nfa N ⇒
+  (w ∈ nfa_lang N ⇔ ∃qs. is_accepting_exec N qs w)
+Proof
+  rw [is_accepting_exec_def,is_exec_def,in_nfa_lang,wf_nfa_def,EQ_IMP_THM] >>
+  metis_tac [SUBSET_DEF]
+QED
+
+Theorem epsilon_in_nfa_lang:
+  wf_nfa N ⇒ (ε ∈ nfa_lang N ⇔ N.initial ∩ N.final ≠ ∅)
+Proof
+  rw [wf_nfa_def, in_nfa_lang, LENGTH_EQ_NUM_compute, EQ_IMP_THM] >>
+  fs [EXTENSION,IN_INTER,PULL_EXISTS] >> metis_tac []
+QED
+
+Theorem is_exec_length:
+  is_exec N qs w ⇒ LENGTH qs = LENGTH w + 1
+Proof
+ rw [is_exec_def]
+QED
+
+Theorem is_exec_nonempty:
+  is_exec N qs w ⇒ qs ≠ []
+Proof
+ rw [is_exec_def] >> Cases_on ‘qs’ >> fs[]
+QED
+
+Theorem is_exec_tl_nonempty:
+  w ≠ ε ∧ is_exec N qs w ⇒ TL qs ≠ []
+Proof
+ rw [is_exec_def] >>
+ Cases_on ‘qs’ >> fs[GSYM ADD1] >>
+ Cases_on ‘t’ >> fs[]
+QED
+
+Theorem is_exec_Sigma:
+  is_exec N qs w ⇒ EVERY (λa. a ∈ N.Sigma) w
+Proof
+ rw [is_exec_def]
+QED
+
+Theorem is_exec_hd_state:
+  is_exec N qs w ⇒ HD qs ∈ N.Q
+Proof
+ rw [is_exec_def]
+QED
+
+Theorem is_exec_delta:
+  is_exec N qs w ∧ n < LENGTH w ⇒ EL (n+1) qs ∈ N.delta (EL n qs) (EL n w)
+Proof
+ rw [is_exec_def]
+QED
+
+Theorem is_exec_TL:
+  wf_nfa N ∧ is_exec N qs w ∧ w ≠ ε ⇒ is_exec N (TL qs) (TL w)
+Proof
+  rw [is_exec_def]
+  >- (Cases_on ‘w’ >> fs [])
+  >- (Cases_on ‘qs’ >> Cases_on ‘w’ >> fs[])
+  >- (Cases_on ‘qs’ >> fs[] >> Cases_on ‘t’ >> fs[GSYM ADD1] >>
+      ‘0 < LENGTH w’ by decide_tac >> first_x_assum drule >> rw[] >>
+      Cases_on ‘w’ >> fs[] >> metis_tac [wf_nfa_def,SUBSET_DEF])
+  >- (‘qs ≠ []’ by (Cases_on ‘qs’ >> fs[]) >> rw [] >>
+      ‘0 < LENGTH w’ by (Cases_on ‘w’ >> fs[]) >> fs [LENGTH_TL] >>
+      ‘n+1 < LENGTH w’ by decide_tac >> rw[] >> first_x_assum drule >> rw[])
+QED
+
+Theorem is_exec_TL_alt:
+  wf_nfa N ∧ is_exec N (q::qs) (a::w) ⇒ is_exec N qs w
+Proof
+  rpt strip_tac >> drule is_exec_TL >> rw[] >> res_tac >> fs[]
+QED
+
+Theorem is_exec_states:
+  wf_nfa N ∧ is_exec N qs w ⇒ EVERY (λq. q ∈ N.Q) qs
+Proof
+  rw [is_exec_def,EVERY_EL] >> Induct_on ‘n’ >> rw[] >> fs[] >>
+  ‘n < LENGTH w’ by decide_tac >> last_x_assum drule >>
+  metis_tac [ADD1, wf_nfa_def,SUBSET_DEF]
+QED
+
+Theorem is_exec_extend_left:
+  wf_nfa N ∧
+  a ∈ N.Sigma ∧
+  q1 ∈ N.Q ∧
+  q2 ∈ N.delta q1 a ∧
+  is_exec N (q2::qs) w ⇒ is_exec N (q1::q2::qs) (a::w)
+Proof
+  rw [is_exec_def] >> Cases_on ‘n’ >> gvs[GSYM ADD1]
+QED
+
+Theorem is_exec_step_left:
+  wf_nfa N ∧ is_exec N (q1::q2::qs) (a::w) ⇒ q2 ∈ N.delta q1 a ∧ is_exec N (q2::qs) w
+Proof
+  rw[is_exec_def,wf_nfa_def]
+  >- (‘0 < SUC(LENGTH w)’ by decide_tac >> first_x_assum drule >> rw[])
+  >- (‘0 < SUC(LENGTH w)’ by decide_tac >> first_x_assum drule >>
+      gvs[SUBSET_DEF] >> metis_tac[])
+  >- (‘SUC n < SUC(LENGTH w)’ by decide_tac >>
+      first_x_assum drule >> rw[GSYM ADD1])
+QED
+
+Theorem is_accepting_exec_length:
+ wf_nfa N ∧ w ≠ ε ∧ is_accepting_exec N qs w
+ ⇒
+ TL qs ≠ []
+Proof
+ rw[is_accepting_exec_def,is_exec_def] >>
+ ‘0 < LENGTH w’ by metis_tac[NOT_NIL_EQ_LENGTH_NOT_0] >>
+ Cases_on ‘qs’ >> fs[] >> Cases_on ‘t’ >> fs[]
+QED
+
+Theorem is_accepting_exec_final:
+ is_accepting_exec N qs w ⇒ LAST qs ∈ N.final
+Proof
+ rw[is_accepting_exec_def]
+QED
+
+Theorem accepting_exec_states_not_nil:
+  is_accepting_exec M qs w ⇒ qs ≠ []
+Proof
+  rw [is_accepting_exec_def] >>
+  drule is_exec_length >>
+  rpt strip_tac >> gvs[]
+QED
+
+Theorem accepting_exec_min_lengths:
+  wf_nfa M ∧
+  ε ∉ nfa_lang M ∧
+  is_accepting_exec M qs w
+  ⇒
+  qs ≠ [] ∧ (∀x. qs ≠ [x]) ∧ w ≠ ε
+Proof
+ rw [is_accepting_exec_def] >> strip_tac >>
+ rw[] >> rfs[epsilon_in_nfa_lang,EXTENSION]
+  >- metis_tac [is_exec_nonempty]
+  >- metis_tac[]
+  >- (gvs [is_exec_def] >> Cases_on ‘qs’ >> gvs[] >> metis_tac[])
+QED
+
+Theorem epsilon_free_exec_left_cons:
+  w ≠ ε ∧ is_exec M qs w
+  ⇒
+  ∃q1 q2 qs' a w'. qs = q1::q2::qs' ∧ w = a::w'
+Proof
+  rw [is_exec_def] >>
+  Cases_on ‘w’ >>
+  Cases_on ‘qs’ >> gvs[] >>
+  Cases_on ‘t'’ >> gvs[]
+QED
+
+Theorem nfa_execution_states_closed:
+  wf_nfa N ⇒
+  ∀w Q.
+   EVERY (λa. a ∈ N.Sigma) w ∧
+   LENGTH Q = LENGTH w + 1 ∧
+   HD Q ∈ N.Q ∧
+   (∀n. n < LENGTH w ⇒ EL (n+1) Q ∈ N.delta (EL n Q) (EL n w))
+   ==>
+   EVERY (λq. q ∈ N.Q) Q
+Proof
+  disch_tac >> ho_match_mp_tac SNOC_INDUCT >> rw[]
+  >- (fs[LENGTH_EQ_NUM_compute,wf_nfa_def,SUBSET_DEF] >> gvs[])
+  >- (‘LENGTH Q = LENGTH w + 2’ by decide_tac >> drule snoc2 >> rw[] >>
+      gvs [GSYM SNOC_APPEND,EVERY_SNOC] >>
+      rename [‘a ∈ N.Sigma’, ‘HD qs ∈ N.Q’] >>
+      ‘SUC (LENGTH w) = LENGTH qs’ by decide_tac >> gvs[EL_LENGTH_SNOC] >>
+      ‘EVERY (λq. q ∈ N.Q) qs’ by
+        (first_x_assum irule >> rw[] >> ‘n < LENGTH qs’ by decide_tac >>
+         first_x_assum drule >> rw [EL_SNOC]) >>
+      ‘LENGTH w < LENGTH qs’ by decide_tac >>
+      first_x_assum drule >> fs [ADD1,EL_SNOC,EL_LENGTH_SNOC] >>
+      ‘EL (LENGTH w) qs ∈ N.Q’ by
+        (rw [EL_LENGTH_LAST] >> drule_all EVERY_LAST >> simp[]) >>
+      metis_tac [wf_nfa_def,SUBSET_DEF])
+QED
+
+Theorem nfa_execution_last_state:
+  wf_nfa N ⇒
+  ∀w Q.
+   EVERY (λa. a ∈ N.Sigma) w ∧
+   LENGTH Q = LENGTH w + 1 ∧
+   HD Q ∈ N.initial ∧
+   (∀n. n < LENGTH w ⇒ EL (n+1) Q ∈ N.delta (EL n Q) (EL n w))
+   ==>
+   EL (LENGTH w) Q ∈ N.Q
+Proof
+  rpt strip_tac >>
+  ‘Q ≠ []’ by (Cases_on ‘Q’ >> fs[]) >>
+  ‘HD Q ∈ N.Q’ by metis_tac [wf_nfa_def,SUBSET_DEF] >>
+  drule_all nfa_execution_states_closed >> strip_tac >>
+  drule_all EVERY_LAST >> simp[EL_LENGTH_LAST]
+QED
+
+(*---------------------------------------------------------------------------*)
+(* DFA execution on valid words.                                             *)
+(*---------------------------------------------------------------------------*)
+
+Theorem dfa_execution:
+  is_dfa N ⇒
+  ∀w.
+    EVERY (λa. a ∈ N.Sigma) w
+     ⇒
+    ∃qs. LENGTH qs = LENGTH w + 1 ∧ {HD qs} = N.initial ∧
+         EVERY (λq. q ∈ N.Q) qs ∧
+         (∀n. n<LENGTH w ⇒ {EL (n+1) qs} = N.delta (EL n qs) (EL n w))
+Proof
+  disch_tac >> ho_match_mp_tac SNOC_INDUCT >> rw[EVERY_SNOC]
+  >- gvs [LENGTH_EQ_NUM_compute,is_dfa_def,PULL_EXISTS,wf_nfa_def]
+  >- (first_x_assum drule >> rw[] >> rename1 ‘a ∈ N.Sigma’ >>
+      ‘qs ≠ []’ by (Cases_on ‘qs’ >> fs[]) >>
+      ‘LAST qs ∈ N.Q’ by
+        (‘EL (LENGTH w) qs ∈ N.Q’ by
+           (irule nfa_execution_last_state >> fs [is_dfa_def] >> rw[]
+            >- metis_tac[EXTENSION,IN_INSERT]
+            >- rfs[]) >> metis_tac [EL_LENGTH_LAST]) >>
+      fs [is_dfa_def, wf_nfa_def] >>
+      ‘∃q. {q} = N.delta (LAST qs) a’ by metis_tac[] >>
+      ‘q ∈ N.Q’ by metis_tac [SUBSET_DEF,EXTENSION,IN_INSERT] >>
+      qexists_tac ‘SNOC q qs’ >> rw[EVERY_SNOC]
+      >- rfs[]
+      >- (‘n < LENGTH w ∨ n = LENGTH w’ by decide_tac
+          >- rw [EL_SNOC]
+          >- (rw [EL_SNOC, EL_LENGTH_LAST] >>
+              qpat_x_assum ‘LENGTH qs = LENGTH w + 1’ (SUBST_ALL_TAC o GSYM) >>
+              rw [EL_LENGTH_SNOC]))
+     )
+QED
+
+Theorem dfa_execution_deterministic:
+  is_dfa N ⇒
+  ∀w Q1 Q2.
+    EVERY (λa. a ∈ N.Sigma) w ∧
+    LENGTH Q1 = LENGTH w + 1 ∧
+    HD Q1 ∈ N.initial ∧
+    (∀n. n<LENGTH w ⇒ EL (n+1) Q1 ∈ N.delta (EL n Q1) (EL n w))
+    ∧
+    LENGTH Q2 = LENGTH w + 1 ∧
+    HD Q2 ∈ N.initial ∧
+    (∀n. n<LENGTH w ⇒ EL (n+1) Q2 ∈ N.delta (EL n Q2) (EL n w))
+  ⇒
+  Q1 = Q2
+Proof
+  disch_tac >> ho_match_mp_tac SNOC_INDUCT >> rw[]
+  >- gvs [LENGTH_EQ_NUM_compute,is_dfa_def]
+  >- (rename1 ‘SNOC a w’ >> fs [EVERY_SNOC] >>
+      ‘LENGTH Q1 = LENGTH w + 2 ∧ LENGTH Q2 = LENGTH w + 2’ by decide_tac >>
+      ‘∃qs1 q1. Q1 = SNOC q1 qs1 ∧ qs1 ≠ []’ by metis_tac[snoc2] >>
+      ‘∃qs2 q2. Q2 = SNOC q2 qs2 ∧ qs2 ≠ []’ by metis_tac[snoc2] >> fs[] >>
+      irule (METIS_PROVE [] “(b' ⇒ a=a') ∧ (a' ⇒ b=b') ∧ a' ∧ b' ⇒ a ∧ b”) >>
+      qexists_tac ‘qs1 = qs2’ >> qexists_tac ‘T’ >> simp[] >> conj_tac
+      >- (first_x_assum irule >> rw[LENGTH_FRONT] >> fs[GSYM SNOC_APPEND]
+          >- (‘EL (n+1) (SNOC q1 qs1) ∈
+               N.delta (EL n (SNOC q1 qs1)) (EL n (SNOC a w))’ by rw[] >>
+               rpt (forget_tac is_forall) >> pop_assum mp_tac >> simp [EL_SNOC])
+          >- (‘EL (n+1) (SNOC q2 qs2) ∈
+               N.delta (EL n (SNOC q2 qs2)) (EL n (SNOC a w))’ by rw[] >>
+               rpt(forget_tac is_forall) >> pop_assum mp_tac >> simp[EL_SNOC]))
+      >- (rw[] >> forget_tac is_neg >> forget_tac is_eq >>
+          fs [GSYM SNOC_APPEND] >> ‘LENGTH w < SUC (LENGTH w)’ by decide_tac >>
+          first_x_assum drule >> fs [Once BOUNDED_FORALL_THM] >>
+          ‘LENGTH w + 1 = LENGTH qs1’ by decide_tac >>
+          gvs[EL_LENGTH_SNOC,EL_SNOC] >>
+          ‘EL (LENGTH w) qs1 ∈ N.Q’ by
+            (irule nfa_execution_last_state >> rw[] >> fs [is_dfa_def]) >>
+          fs [is_dfa_def] >>
+          ‘∃qf. N.delta (EL (LENGTH w) qs1) a = {qf}’ by metis_tac[] >> gvs[])
+     )
+QED
+
+(*---------------------------------------------------------------------------*)
 (* Subset construction                                                       *)
 (*---------------------------------------------------------------------------*)
 
 Definition nfa_to_dfa_def:
   nfa_to_dfa N =
-    <|Q := {enc s | s ⊆ N.Q};
-      Sigma := N.Sigma;
-      delta := λq a. {enc (BIGUNION {N.delta qi a | qi ∈ dec q})};
+    <|Q       := {enc s | s ⊆ N.Q};
+      Sigma   := N.Sigma;
+      delta   := λq a. {enc (BIGUNION {N.delta qi a | qi ∈ dec q})};
       initial := {enc N.initial};
-      acceptors := {enc s | s ⊆ N.Q ∧ s ∩ N.acceptors ≠ ∅} |>
+      final   := {enc s | s ⊆ N.Q ∧ s ∩ N.final ≠ ∅} |>
 End
 
-Triviality in_nfa_to_dfa_states[simp]:
-  ∀q. q ∈ (nfa_to_dfa N).Q <=> ∃s. q = enc s ∧ s ⊆ N.Q
+Triviality nfa_to_dfa_builtin_simps[simp]:
+  (nfa_to_dfa N).Sigma = N.Sigma ∧
+  (nfa_to_dfa N).initial = {enc N.initial} ∧
+  (nfa_to_dfa N).final   = {enc s | s ⊆ N.Q ∧ s ∩ N.final ≠ ∅} ∧
+  (∀q. q ∈ (nfa_to_dfa N).Q <=> ∃s. q = enc s ∧ s ⊆ N.Q)
 Proof
   rw[nfa_to_dfa_def]
-QED
-
-Triviality nfa_to_dfa_Sigma[simp]:
-  (nfa_to_dfa N).Sigma = N.Sigma
-Proof
-  rw[nfa_to_dfa_def]
-QED
-
-Triviality nfa_to_dfa_initial[simp]:
-  (nfa_to_dfa N).initial = {enc N.initial}
-Proof
-  rw[nfa_to_dfa_def]
-QED
-
-Triviality nfa_to_dfa_acceptors[simp]:
-  (nfa_to_dfa N).acceptors = {enc s | s ⊆ N.Q ∧ s ∩ N.acceptors ≠ ∅}
-Proof
-  rw[nfa_to_dfa_def]
-QED
-
-Theorem finite_dfa_delta_successors:
- wf_nfa N ⇒
-  ∀eq a. s ⊆ N.Q ∧ a ∈ N.Sigma ==> FINITE (BIGUNION {N.delta q a | q ∈ s})
-Proof
-  rw [] >>
-  ‘FINITE s’ by metis_tac [SUBSET_FINITE,wf_nfa_def]
-  >- (fs[GSPEC_IMAGE,o_DEF,IN_DEF] >> metis_tac [IMAGE_FINITE])
-  >- (fs [wf_nfa_def] >> metis_tac [SUBSET_FINITE,SUBSET_DEF])
 QED
 
 (*---------------------------------------------------------------------------*)
-(* Well-formedness of a constructed DFA                                      *)
+(* Well-formedness of subset DFA                                             *)
 (*---------------------------------------------------------------------------*)
 
 Theorem is_dfa_nfa_to_dfa:
@@ -347,12 +864,7 @@ Proof
 QED
 
 (*---------------------------------------------------------------------------*)
-(* All lemmas about DFA executions go by SNOC induction. The SNOC step       *)
-(* assumes the property for the front of the list and wants to show it for   *)
-(* the last element. The last element is obtained by a Delta step from the   *)
-(* last element of the front of the list. In order to expand the Delta step, *)
-(* the last element of the front of the list has to shown to be in the state *)
-(* set.                                                                      *)
+(* This seems very close to nfa_states_closed above.                         *)
 (*---------------------------------------------------------------------------*)
 
 Theorem dfa_states_closed:
@@ -377,7 +889,7 @@ Proof
           >- (rw[PULL_EXISTS] >>  qexistsl_tac [‘FRONT eqs’, ‘LAST eqs’] >>
               rw [LENGTH_FRONT,APPEND_FRONT_LAST])) >>
       drule_all EVERY_LAST >> rw[] >> fs [Once BOUNDED_FORALL_THM] >>
-      rpt (weaken_tac is_forall) >> qpat_x_assum ‘_ ∈ _’ mp_tac >>
+      rpt (forget_tac is_forall) >> qpat_x_assum ‘_ ∈ _’ mp_tac >>
       fs[EVERY_SNOC,EL_LENGTH_SNOC] >>
       ‘LENGTH w + 1 = LENGTH eqs’ by decide_tac >> pop_subst_tac >>
       simp_tac std_ss [GSYM SNOC_APPEND] >> simp [EL_LENGTH_SNOC,EL_SNOC] >>
@@ -388,6 +900,7 @@ Proof
       rw [nfa_to_dfa_def] >> irule_at Any EQ_REFL >>
       rw[BIGUNION_SUBSET,SUBSET_DEF] >> metis_tac[wf_nfa_def,SUBSET_DEF])
 QED
+
 
 Theorem nfa_to_dfa_execution_states:
   wf_nfa N ⇒
@@ -405,20 +918,10 @@ Proof
   drule_all EVERY_LAST >> rw [nfa_to_dfa_def]
 QED
 
-Triviality snoc2:
- ∀list n. LENGTH list = n+2 ⇒ ∃a b. list = SNOC a b ∧ b ≠ []
-Proof
-  rpt strip_tac >> Cases_on ‘list = []’
-  >- fs[]
-  >- (drule SNOC_LAST_FRONT >> Cases_on ‘FRONT list = []’
-      >- (Cases_on ‘list’ >> fs[])
-      >- metis_tac [])
-QED
-
 (*---------------------------------------------------------------------------*)
 (* Main lemma for the subset construction. The last state in an execution of *)
 (* the DFA on input w, when decoded, is equal to the set of states reachable *)
-(* by NFA executions on w.                                                   *)
+(* by NFA execution on w.                                                    *)
 (*---------------------------------------------------------------------------*)
 
 Theorem nfa_to_dfa_inductive:
@@ -448,7 +951,7 @@ Proof
         by (first_x_assum irule >> rw[] >> fs[] >>
             fs [Once BOUNDED_FORALL_THM] >> first_x_assum drule >>
             full_simp_tac std_ss [GSYM SNOC_APPEND] >> simp[EL_SNOC]) >>
-     qpat_weaken_tac ‘$∀ (M:num list->bool)’ >> rw[] >> fs[] >>
+     qpat_forget_tac ‘$∀ (M:num list->bool)’ >> rw[] >> fs[] >>
      (* LAST eqs' encodes a set of states s *)
      ‘∃s. LAST eqs' = enc s ∧ s ⊆ N.Q’ by
        (‘(LAST eqs') ∈ (nfa_to_dfa N).Q’
@@ -470,9 +973,9 @@ Proof
      drule_then (rewrite_tac o single) MEM_SET_TO_LIST >>
      disch_then (SUBST1_TAC o SYM) >>
      ‘FINITE (BIGUNION {N.delta qi a | qi ∈ s})’
-        by metis_tac[finite_dfa_delta_successors] >> simp[] >>
-     ntac 2 pop_forget_tac >> qpat_weaken_tac ‘s = GSPEC _’ >>
-     (* Finally equality between the two fringe state sets *)
+        by metis_tac[finite_nfa_successors] >> simp[] >>
+     ntac 2 pop_forget_tac >> qpat_forget_tac ‘s = GSPEC _’ >>
+     (* Now show equality between the two fringe state sets *)
      rw [EXTENSION] >> eq_tac >> rpt strip_tac >> fs[] >> rw[PULL_EXISTS] >>
      ‘qs ≠ []’ by (Cases_on ‘qs’ >> gvs[])
      >- (qexists_tac ‘SNOC x qs’ >> rw[EL_SNOC] >>
@@ -530,7 +1033,7 @@ Proof
   rw[EL_LENGTH_SNOC,
      EL_LENGTH_SNOC |> Q.ISPEC ‘SNOC eq eqs: num list’
                     |> SIMP_RULE std_ss [LENGTH_SNOC],EL_SNOC] >>
- rw [nfa_to_dfa_def]
+  rw [nfa_to_dfa_def]
 QED
 
 (*---------------------------------------------------------------------------*)
@@ -544,7 +1047,7 @@ Proof
  >- (rename1 ‘LAST eqs = enc s’ >> drule_all nfa_to_dfa_inductive >> rw[] >>
      ‘FINITE s’ by metis_tac [wf_nfa_def,SUBSET_FINITE] >>
      qpat_x_assum ‘set (SET_TO_LIST _) = _’ mp_tac >> simp [SET_TO_LIST_INV] >>
-     ‘∃qa. qa ∈ s ∧ qa ∈ N.acceptors’ by (fs[EXTENSION] >> metis_tac[]) >>
+     ‘∃qa. qa ∈ s ∧ qa ∈ N.final’ by (fs[EXTENSION] >> metis_tac[]) >>
      rw[EXTENSION] >> metis_tac[])
  >- (drule_all nfa_path_to_dfa_path >> rw[] >> qexists_tac ‘eqs’ >> rw[] >>
      drule_all dfa_states_closed >> disch_tac >>
@@ -561,37 +1064,12 @@ Theorem NFA_LANGS_EQ_DFA_LANGS:
   NFA_LANGS = DFA_LANGS
 Proof
   rw [EXTENSION,IN_NFA_LANGS,IN_DFA_LANGS,EQ_IMP_THM]
-  >- (qexists_tac ‘nfa_to_dfa N’ >>
-      rw [is_dfa_nfa_to_dfa,nfa_to_dfa_correct])
-  >- (fs [is_dfa_def] >> metis_tac[])
+  >- metis_tac [is_dfa_nfa_to_dfa,nfa_to_dfa_correct]
+  >- metis_tac[is_dfa_def]
 QED
 
 (*===========================================================================*)
-(* NFA and DFA languages are Finite_State languages.                         *)
-(*===========================================================================*)
-
-Theorem DFA_Finite_State:
-  DFA_LANGS ⊆ Finite_State
-Proof
- cheat
-QED
-
-Theorem Finite_State_DFA:
-  Finite_State ⊆ DFA_LANGS
-Proof
- cheat
-QED
-
-Theorem NFA_LANGS_EQ_Finite_State:
-  Finite_State = NFA_LANGS
-Proof
-  metis_tac [SET_EQ_SUBSET,NFA_LANGS_EQ_DFA_LANGS,
-             DFA_Finite_State, Finite_State_DFA]
-QED
-
-
-(*===========================================================================*)
-(* Boolean, and other, closure properties via machine constructions          *)
+(* Machine constructions and closure properties                              *)
 (*===========================================================================*)
 
 Definition nfa_compl_def:
@@ -600,1620 +1078,1636 @@ Definition nfa_compl_def:
       Sigma := N.Sigma;
       delta := N.delta;
       initial := N.initial;
-      acceptors := (N.Q DIFF N.acceptors)
+      final   := (N.Q DIFF N.final)
     |>
 End
 
 Definition nfa_inter_def:
   nfa_inter N1 N2 =
     <|Q  := {q1 ⊗ q2 | q1 ∈ N1.Q ∧ q2 ∈ N2.Q};
-      Sigma := N1.Sigma ∪ N2.Sigma;
+      Sigma := N1.Sigma ∩ N2.Sigma;
       delta := λq a. {q1 ⊗ q2 | q1 ∈ N1.delta (nfst q) a ∧ q2 ∈ N2.delta (nsnd q) a};
-      initial   := {q1 ⊗ q2 | q1 ∈ N1.initial ∧ q2 ∈ N2.initial};
-      acceptors := {q1 ⊗ r2 | q1 ∈ N1.acceptors ∧ r2 ∈ N2.acceptors}
+      initial := {q1 ⊗ q2 | q1 ∈ N1.initial ∧ q2 ∈ N2.initial};
+      final   := {q1 ⊗ r2 | q1 ∈ N1.final ∧ r2 ∈ N2.final}
     |>
 End
 
 Definition nfa_union_def:
   nfa_union N1 N2 =
     <|Q  := {q1 ⊗ q2 | q1 ∈ N1.Q ∧ q2 ∈ N2.Q };
-      Sigma := N1.Sigma ∪ N2.Sigma;
+      Sigma := N1.Sigma ∩ N2.Sigma;
       delta := λq a. {q1 ⊗ q2 | q1 ∈ N1.delta (nfst q) a ∧ q2 ∈ N2.delta (nsnd q) a};
-      initial   := {q1 ⊗ q2 | q1 ∈ N1.initial ∧ q2 ∈ N2.initial};
-      acceptors := {q1 ⊗ q2 | (q1 ∈ N1.acceptors ∧ q2 ∈ N2.Q) ∨
-                              (q1 ∈ N1.Q ∧ q2 ∈ N2.acceptors)};
+      initial := {q1 ⊗ q2 | q1 ∈ N1.initial ∧ q2 ∈ N2.initial};
+      final   := {q1 ⊗ q2 | (q1 ∈ N1.final ∧ q2 ∈ N2.Q) ∨
+                            (q1 ∈ N1.Q ∧ q2 ∈ N2.final)};
     |>
 End
 
-Definition nfa_cat_def:
-  nfa_cat N1 N2 =
-    <|Q  := {0 ⊗ q | q ∈ N1.Q} ∪ {1 ⊗ q | q ∈ N2.Q};
-      Sigma := N1.Sigma ∪ N2.Sigma;
+Definition nfa_dot_def:
+  nfa_dot N1 N2 =
+    <|Q  := N1.Q ∪ N2.Q; (* N1.Q and N2.Q are disjoint *)
+      Sigma := N1.Sigma ∩ N2.Sigma;
       delta := λq a.
-              if nfst q = 0 then
-                let
-                  N1kids = {0 ⊗ q1 | q1 ∈ N1.delta (nsnd q) a}
-                in
-                  if nsnd q ∈ N1.acceptors ∧ copt = NONE then frs ∪ {1 ⊗ N2.q_0}
-                  else frs
-              else
-                {1 ⊗ s' | s' ∈ N2.tf (nsnd s) copt};
-      initial   := {0 ⊗ q | q ∈ N1.initial};
-      acceptors := {1 ⊗ q | q ∈ N2.acceptors};
+        if q ∈ N1.Q then
+          (if q ∉ N1.final then N1.delta q a
+           else N1.delta q a ∪
+                BIGUNION {N2.delta q' a |q'| q' ∈ N2.initial})
+        else N2.delta q a;
+      initial := N1.initial;
+      final   := N2.final;
     |>
 End
 
-Definition nfa_star_def:
-  nfa_star N =
-   <| Q :=  IMAGE SUC N.Q ∪ {0} ;
+Definition nfa_plus_def:
+  nfa_plus N =
+   <|Q := N.Q;
      Sigma := N.Sigma ;
-     tf := λs0 copt.
-             case s0 of
-               0 => if copt = NONE then {SUC N.q_0} else ∅
-             | SUC s0' =>
-                if copt = NONE ∧ s0' ∈ N.C then
-                  IMAGE SUC (N.tf s0' copt) ∪ {0}
-                else IMAGE SUC (N.tf s0' copt) ;
-     initia := 0 ;
-     acceptors := {0};
+     delta := λq a.
+       if q ∉ N.final then
+         N.delta q a
+       else
+         N.delta q a ∪
+         BIGUNION {N.delta q' a |q'| q' ∈ N.initial};
+     initial := N.initial ;
+     final   := N.final;
    |>
 End
 
-(* Theorem 1.25 *)
-Theorem wf_dfa_nfa_union :
-  ∀M1 N2. wf_dfa M1 ∧ wf_dfa N2 ⇒ wf_dfa (machine_union M1 N2)
+(*---------------------------------------------------------------------------*)
+(* Wellformedness of constructions                                           *)
+(*---------------------------------------------------------------------------*)
+
+Theorem wf_nfa_compl:
+  wf_nfa N ⇒ wf_nfa (nfa_compl N)
 Proof
-  rw[wf_dfa_def,machine_union_def] (* 11 *) >> simp[]
-  >- (qmatch_abbrev_tac ‘FINITE s’ >>
-      ‘s = IMAGE (UNCURRY npair) (M1.Q CROSS M2.Q)’ suffices_by simp[] >>
-      simp[Abbr‘s’, EXTENSION, pairTheory.EXISTS_PROD])
-  >- (simp[SUBSET_DEF,PULL_EXISTS] >> metis_tac[SUBSET_DEF])
-  >- (Cases_on ‘c ∈ M2.A’ >> simp[])
+  rw[wf_nfa_def, nfa_compl_def]
+QED
+
+Theorem wf_nfa_inter:
+  wf_nfa N1 ∧ wf_nfa N2 ⇒ wf_nfa (nfa_inter N1 N2)
+Proof
+  rw [wf_nfa_def,nfa_inter_def,SUBSET_DEF]
+  >- (rw [GSPEC_IMAGE, o_DEF,pairTheory.LAMBDA_PROD] >>
+      irule IMAGE_FINITE >> irule SUBSET_FINITE >>
+      qexists ‘N1.Q CROSS N2.Q’ >> rw[] >>
+      rw [SUBSET_DEF,CROSS_DEF,pairTheory.LAMBDA_PROD,pairTheory.FORALL_PROD])
   >- metis_tac[]
-QED
-
-(* regular languages closed under union *)
-Theorem thm_1_25:
-  ∀ lA lB. regularLanguage lA ∧
-           regularLanguage lB ⇒
-           regularLanguage (lA ∪ lB)
-Proof
-  rw [regularLanguage_def] >>
-  rename [‘recogLangD M1 ∪ recogLangD M2’] >>
-  qexists_tac ‘machine_union M1 M2’ >>
-  rw [recogLangD_def, EXTENSION,
-      has_Accepting_Execution_Delta_coincide_thm,
-      wf_dfa_machine_union] >>
-  qabbrev_tac ‘MU = machine_union M1 M2’ >>
-  rw[accepts_def] >>
-  ‘(MU.A = M1.A ∪ M2.A) ∧ (MU.q_0 = M1.q_0 ⊗ M2.q_0)’
-    by rw[machine_union_def, Abbr ‘MU’] >>
-  simp[] >>
-  ‘∀ q1 q2. q1 ∈ M1.Q ∧ q2 ∈ M2.Q
-    ⇒ (Delta MU (q1 ⊗ q2) x ∈ MU.C ⇔
-      Delta M1 q1 x ∈ M1.C ∨ Delta M2 q2 x ∈ M2.C)’
-    suffices_by (rpt strip_tac >>
-                 metis_tac[wf_dfa_def]) >>
-  Induct_on ‘x’
-  >- (rw[Abbr ‘MU’, Delta_def,machine_union_def])
-  >- (rw[Delta_def, DISJ_IMP_THM, FORALL_AND_THM] >>
-      ‘MU.tf (q1 ⊗ q2) h = M1.tf q1 h ⊗ M2.tf q2 h’
-        by rw[Abbr ‘MU’, machine_union_def] >>
-      first_x_assum (fn x => SUBST_TAC [x]) >>
-      ‘M1.tf q1 h ∈ M1.Q ∧ M2.tf q2 h ∈ M2.Q’
-        suffices_by metis_tac[] >>
-      metis_tac[wf_dfa_def])
-QED
-
-(*---------------------------------------------------------------------------*)
-(* Closure under concatenation                                               *)
-(*---------------------------------------------------------------------------*)
-
-Definition machine_link_def:
-  machine_link N1 N2 =
-    <|Q  := {0 ⊗ q1 | q1 ∈ N1.Q} ∪ {1 ⊗ r2 | r2 ∈ N2.Q};
-      A  := N1.A ∪ N2.A;
-      tf := λs copt.
-              if nfst s = 0 then
-                let
-                  frs = { 0 ⊗ s' | s' ∈ N1.tf (nsnd s) copt}
-                in
-                  if nsnd s ∈ N1.C ∧ copt = NONE then frs ∪ {1 ⊗ N2.q_0}
-                  else frs
-              else
-                {1 ⊗ s' | s' ∈ N2.tf (nsnd s) copt};
-      q_0 := 0 ⊗ N1.q_0;
-      C  := {1 ⊗ r2 | r2 ∈ N2.C };
-    |>
-End
-
-val _ =
-  set_mapped_fixity
-     {term_name = "machine_link",
-      fixity = Infixl 500,
-      tok = "⌢"}
-
-Theorem machine_link_q_0[simp]:
-  (N1 ⌢ N2).q_0 = 0 ⊗ N1.q_0
-Proof
-  simp[machine_link_def]
-QED
-
-Theorem wfNFA_machine_link:
-  ∀N1 N2.
-    wfNFA N1 ∧ wfNFA N2 ⇒ wfNFA (N1 ⌢ N2)
-Proof
-  rw[wfNFA_def,machine_link_def]
-  >- (qmatch_abbrev_tac ‘FINITE s’ >>
-      ‘s = IMAGE (npair 0) N1.Q’
-        suffices_by metis_tac[IMAGE_FINITE] >>
-      simp[EXTENSION,Abbr ‘s’])
-  >- (qmatch_abbrev_tac ‘FINITE s’ >>
-      ‘s = IMAGE (npair 1) N2.Q’
-        suffices_by metis_tac[IMAGE_FINITE] >>
-      simp[EXTENSION,Abbr ‘s’]) >>
-  simp[SUBSET_DEF,PULL_EXISTS] >> rw[] >>
-  metis_tac[SUBSET_DEF,NOT_IN_EMPTY]
-QED
-
-Theorem machine_link_tf0:
-  (N1 ⌢ N2).tf (0 ⊗ n1) c =
-   if n1 ∈ N1.C ∧ c = NONE then
-      {0 ⊗ n | n ∈ N1.tf n1 NONE} ∪ {1 ⊗ N2.q_0}
-    else {0 ⊗ n | n ∈ N1.tf n1 c}
-Proof
-  simp[machine_link_def]
-QED
-
-Theorem machine_link_A:
-  (N1 ⌢ N2).A = N1.A ∪ N2.A
-Proof
-  simp[machine_link_def]
-QED
-
-Theorem machine_link_C[simp]:
-  (N1 ⌢ N2).C = { 1 ⊗ n | n ∈ N2.C }
-Proof
-  simp[machine_link_def]
-QED
-
-Theorem NF_transition_link2_E:
-  ∀q1 n. NF_transition (N1 ⌢ N2) (1 ⊗ q1) ts n ⇒ ∃q2. n = 1 ⊗ q2
-Proof
-  Induct_on ‘NF_transition’ >> simp[] >> rw[] >> first_x_assum irule >>
-  qpat_x_assum ‘_ ∈ _.tf _ _’ mp_tac >> simp[machine_link_def] >>
-  simp[PULL_EXISTS]
-QED
-
-Theorem NF_transition_link21_impossible[simp]:
-  ¬NF_transition (N1 ⌢ N2) (1 ⊗ q1) ts (0 ⊗ q2)
-Proof
-  strip_tac >> drule NF_transition_link2_E >> simp[]
-QED
-
-Theorem NF_transition_machine_link1[simp]:
-  wfNFA N1 ⇒
-  (NF_transition (N1 ⌢ N2) (0 ⊗ q1) ts (0 ⊗ q2) ⇔ NF_transition N1 q1 ts q2)
-Proof
-  strip_tac >> eq_tac
-  >- (map_every qid_spec_tac [‘q1’, ‘q2’] >> Induct_on ‘NF_transition’ >>
-      rw[] >> fs[NF_transition_rules] >>
-      qpat_x_assum ‘_ ∈ _.tf _ _’ mp_tac >>
-      rw[machine_link_def] >> fs[] >>
-      irule (NF_transition_rules |> SPEC_ALL |> CONJUNCT2) >>
-      fs[machine_link_A] >> fs[wfNFA_def] >>
-      metis_tac[NF_transition_rules, NOT_IN_EMPTY]) >>
-  Induct_on ‘NF_transition’ >> simp[NF_transition_rules] >> rw[] >>
-  irule (NF_transition_rules |> SPEC_ALL |> CONJUNCT2) >>
-  simp[machine_link_A] >> goal_assum (first_assum o mp_then Any mp_tac) >>
-  simp[machine_link_def] >>
-  asm_simp_tac (srw_ss() ++ boolSimps.COND_elim_ss)[] >> metis_tac[]
-QED
-
-Theorem NF_transition_machine_link2[simp]:
-  wfNFA N2 ⇒
-  (NF_transition (N1 ⌢ N2) (1 ⊗ q1) ts (1 ⊗ q2) ⇔ NF_transition N2 q1 ts q2)
-Proof
-  strip_tac >> eq_tac
-  >- (map_every qid_spec_tac [‘q1’, ‘q2’] >> Induct_on ‘NF_transition’ >>
-      rw[] >> fs[NF_transition_rules] >>
-      qpat_x_assum ‘_ ∈ _.tf _ _’ mp_tac >>
-      rw[machine_link_def] >> fs[] >>
-      irule (NF_transition_rules |> SPEC_ALL |> CONJUNCT2) >>
-      fs[machine_link_A] >> fs[wfNFA_def] >>
-      metis_tac[NF_transition_rules, NOT_IN_EMPTY]) >>
-  Induct_on ‘NF_transition’ >> simp[NF_transition_rules] >> rw[] >>
-  irule (NF_transition_rules |> SPEC_ALL |> CONJUNCT2) >>
-  simp[machine_link_A] >> goal_assum (first_assum o mp_then Any mp_tac) >>
-  simp[machine_link_def]
-QED
-
-
-Theorem NF_transition_machine_link_shift12:
-  wfNFA N1 ∧ wfNFA N2 ∧
-  NF_transition (N1 ⌢ N2) q_0 ts q ∧
-  q_0 ∈ { 0 ⊗ n1 | n1 ∈ N1.Q } ∧ q ∈ { 1 ⊗ n2 | n2 ∈ N2.Q }
-⇒
-  ∃q1 ts1 ts2.
-    q1 ∈ N1.C ∧ (* q2 = 1 ⊗ N2.q_0 *)
-    NF_transition N1 (nsnd q_0) ts1 q1 ∧
-    NF_transition N2 N2.q_0 ts2 (nsnd q) ∧
-    ts = ts1 ++ [NONE] ++ ts2
-Proof
-  Induct_on ‘NF_transition’ >> rw[]
-  >- (qspec_then ‘q_0’ strip_assume_tac npair_cases >> simp[] >>
-      rename [‘q_0 = m ⊗ n’] >> Cases_on ‘m = 0’ >> simp[]) >>
-  fs[PULL_EXISTS] >>
-  rename [‘NF_transition _ q1 ts (1 ⊗ n2)’] >>
-  qpat_x_assum ‘_ ∈ _.tf _ _’ mp_tac >>
-  rw[machine_link_def] >> fs[]
-  >- (rename [‘n1' ∈ N1.tf n1 _’] >>
-      ‘n1' ∈ N1.Q’ by metis_tac[wfNFA_def, SUBSET_DEF] >>
-      fs[] >>
-      rename [‘ts = ts1 ++ [NONE] ++ ts2’, ‘NF_transition N1 n1' ts1 q1’,
-              ‘NF_transition N2 N2.q_0 ts2 n2’] >>
-      ‘NF_transition N1 n1 (NONE::ts1) q1’
-         by metis_tac[NF_transition_rules, optionTheory.NOT_SOME_NONE] >>
-      map_every qexists_tac [‘q1’, ‘NONE::ts1’, ‘ts2’] >> simp[])
-  >- (goal_assum drule >> qexists_tac ‘[]’ >> simp[NF_transition_rules])
-  >- (rename [‘n1' ∈ N1.tf n1 _’] >>
-      ‘n1' ∈ N1.Q’ by metis_tac[wfNFA_def, SUBSET_DEF, NOT_IN_EMPTY,
-                                optionTheory.option_CASES] >> fs[] >>
-      goal_assum (first_assum o mp_then (Pos (el 3)) mp_tac) >>
-      rename [‘ts = ts1 ++ [NONE] ++ ts2’, ‘NF_transition N1 n1' ts1 q1’,
-              ‘NF_transition N2 N2.q_0 ts2 n2’] >>
-      ‘NF_transition N1 n1 (c::ts1) q1’
-         by (irule (NF_transition_rules |> SPEC_ALL |> CONJUNCT2) >>
-             reverse conj_tac >- metis_tac[] >> fs[machine_link_A] >>
-             metis_tac[wfNFA_def, NOT_IN_EMPTY]) >>
-      metis_tac[APPEND])
-QED
-
-Theorem munge_exists:
-!ts. ?n xnlist cs.
-  ts = munge n (ZIP (cs,xnlist)) ∧ LENGTH xnlist = LENGTH cs
-Proof
-  Induct_on ‘ts’ >> csimp[ZIP_EQ_NIL] >>
-  strip_tac >> fs[] >> Cases_on ‘h’ (* 2 *)
-  >- (map_every qexists_tac [‘SUC n’,‘xnlist’, ‘cs’] >> simp[munge_SUC]) >>
-  rename [‘SOME c :: munge n (ZIP (cs, xnlist))’] >>
-  map_every qexists_tac [‘0’,‘n::xnlist’, ‘c::cs’] >>
-  simp[]
-QED
-
-Theorem NF_transition_concat:
-  NF_transition m q_0 ts1 q1 ∧ NF_transition m q1 ts2 q2
-  ==>
-  NF_transition m q_0 (ts1 ++ ts2) q2
-Proof
-  Induct_on ‘NF_transition’ >> rw[] >> fs[] >>
-  metis_tac[NF_transition_rules]
-QED
-
-Theorem front_cons_snoc[simp]:
-∀h t x.  FRONT (h::(t++[x])) = h::t
-Proof
-  Induct_on‘t’ >> simp[]
-QED
-
-Theorem replicate_single[simp]:
-  REPLICATE 1 e = [e]
-Proof
-  rw[rich_listTheory.REPLICATE_compute]
-QED
-
-Theorem replicate_snoc[simp]:
-  ∀r.  REPLICATE r NONE ⧺ [NONE] = REPLICATE (r + 1) NONE
-Proof
-  Induct_on ‘r’ >> rw[GSYM arithmeticTheory.ADD1] >> rw[ADD_CLAUSES]
-QED
-
-Theorem munge_middle_none:
-∀ xnlist1 xnlist2 n1 n2.
-  munge n1 xnlist1 ⧺ NONE::munge n2 xnlist2 =
-    if xnlist1 = [] then munge (n1+n2+1) xnlist2
-    else munge n1 (FRONT xnlist1 ++
-                   (FST $ LAST xnlist1, (SND $ LAST xnlist1) + 1 + n2)::xnlist2)
-Proof
-  rw[munge_def,rich_listTheory.REPLICATE_APPEND]
-  >> pop_assum mp_tac
-  >> map_every qid_spec_tac [‘n2’, ‘n1’, ‘xnlist2’, ‘xnlist1’]
-  >> ho_match_mp_tac SNOC_INDUCT >> rw[Excl"APPEND_ASSOC"]
-  >> Cases_on‘xnlist1’ >> fs[]
-  >> rename [‘SOME (FST cn)’] >> Cases_on‘cn’ >>
-  simp[rich_listTheory.REPLICATE_APPEND]
-QED
-
-Theorem WF_IND_I:
-  ∀R P. WF R ∧ (∀x. (∀y. R y x ⇒ P y) ⇒ P x) ⇒ ∀x. P x
-Proof
-  metis_tac[relationTheory.WF_INDUCTION_THM]
-QED
-
-Theorem munge_inj[simp]:
- ∀n1 l1 n2 l2. munge n1 l1 = munge n2 l2 <=> n1 = n2 ∧ l1 = l2
-Proof
-  ‘∀p n2 l2 n1 l1.
-     p = (n1,l1) ⇒ (munge n1 l1 = munge n2 l2 ⇔ n1 = n2 ∧ l1 = l2)’
-     suffices_by simp[] >>
-  ho_match_mp_tac WF_IND_I >> simp[GSYM RIGHT_FORALL_IMP_THM] >>
-  qexists_tac ‘inv_image ($< LEX $<) (λ(n,l). (LENGTH l, n))’ >>
-  conj_tac
-  >- simp[relationTheory.WF_inv_image, pairTheory.WF_LEX] >>
-  simp[pairTheory.LEX_DEF] >> rw[] >>
-  Cases_on ‘n1’ >> simp[]
-  >- (reverse (Cases_on ‘n2’) >> simp[munge_SUC]
-      >- (Cases_on ‘l1’ >> simp[] >> Cases_on ‘h’ >> simp[munge0CONS]) >>
-      map_every Cases_on [‘l1’, ‘l2’] >> simp[] >>
-      rename [‘munge 0 (h1::t1) = munge 0 (h2::t2)’] >>
-      map_every Cases_on [‘h1’, ‘h2’] >> simp[munge0CONS] >> metis_tac[]) >>
-  Cases_on ‘n2’ >> simp[munge_SUC] >>
-  Cases_on ‘l2’ >> simp[] >> Cases_on ‘h’ >> simp[munge0CONS]
-QED
-
-Theorem NON_NIL_FRONT:
-  t ≠ [] ⇒ FRONT(h::t) = h::FRONT t
-Proof
-  Cases_on ‘t’ >> simp[]
-QED
-
-Theorem FRONT_ZIP:
-  ∀l1 l2. l1 ≠ [] ∧ LENGTH l1 = LENGTH l2 ⇒
-          FRONT (ZIP (l1,l2)) = ZIP (FRONT l1, FRONT l2)
-Proof
-  Induct >> simp[] >> Cases_on ‘l2’ >> simp[] >>
-  Cases_on ‘l1 = []’ >> simp[] >> fs[] >>
-  rename [‘LENGTH l1 = LENGTH l2’] >> rw[] >>
-  ‘l2 ≠ []’ by (strip_tac >> fs[]) >>
-  simp[NON_NIL_FRONT, ZIP_EQ_NIL]
-QED
-
-Theorem LAST_ZIP:
-  ∀l1 l2. l1 ≠ [] ∧ LENGTH l1 = LENGTH l2 ⇒
-          LAST (ZIP (l1, l2)) = (LAST l1, LAST l2)
-Proof
-  Induct >> simp[] >> Cases_on ‘l2’ >> simp[] >>
-  Cases_on ‘l1 = []’ >> simp[] >> fs[] >> rw[] >>
-  rename [‘LENGTH l1 = LENGTH l2’] >> ‘l2 ≠ []’ by (strip_tac >> fs[]) >>
-  simp[LAST_CONS_cond, ZIP_EQ_NIL]
-QED
-
-(*---------------------------------------------------------------------------*)
-(* Finally, regular languages are closed under concatenation                 *)
-(*---------------------------------------------------------------------------*)
-
-Theorem thm_1_47:
-  ∀L1 L2.
-    regularLanguage L1 ∧ regularLanguage L2 ⇒ regularLanguage (L1 dot L2)
-Proof
-  rw[corollary_1_40] >>
-  rename1 ‘recogLangN _ = (_ N1) dot (_ N2)’ >>
-  qexists_tac ‘N1 ⌢ N2’ >>
-  rw[wfNFA_machine_link,EXTENSION,dot_def, recogLangN_def,
-     Sipser_ND_Accepts_NF_transition, EQ_IMP_THM]
-  >- (rename [‘LENGTH epslist = LENGTH s’,
-              ‘NF_transition (N1 ⌢ N2) _ (munge eps0 _)’] >>
-      drule_then (drule_then drule) NF_transition_machine_link_shift12 >>
-      simp[] >> impl_tac >- metis_tac[wfNFA_def, SUBSET_DEF] >>
-      strip_tac >>
-      rename [‘munge _ _ = ts1 ⧺ [NONE] ⧺ ts2’,
-              ‘NF_transition _ _ _ (1 *, n)’] >>
-      simp[PULL_EXISTS] >>
-      qspec_then ‘ts1’
-         (qx_choosel_then [‘n1’,‘s1’,‘nlist1’] strip_assume_tac) munge_exists >>
-      qspec_then ‘ts2’
-         (qx_choosel_then [‘n2’,‘s2’,‘nlist2’] strip_assume_tac) munge_exists >>
-      rw[] >>
-      goal_assum (first_assum o mp_then (Pos (el 3)) mp_tac) >>
-      simp[] >>
-      goal_assum (first_assum o mp_then (Pos (el 3)) mp_tac) >>
-      simp[] >>
-      first_x_assum
-        (mp_tac o AP_TERM “drop_epsilon: num option list -> num list”) >>
-      simp[drop_epsilon_munge]) >>
-  rename [‘machine_link N1 N2’,
-          ‘NF_transition N1 _ (munge n1 (ZIP (s1,nlist1))) q1’,
-          ‘NF_transition N2 _ (munge n2 (ZIP (s2,nlist2))) q2’] >>
-  ‘NF_transition (N1 ⌢ N2) (0 ⊗ N1.q_0) (munge n1 (ZIP (s1,nlist1))) (0 ⊗ q1)’
-     by simp[] >>
-  ‘NF_transition (N1 ⌢ N2) (1 ⊗ N2.q_0) (munge n2 (ZIP (s2,nlist2))) (1 ⊗ q2)’
-     by simp[] >>
-  ‘NF_transition (N1 ⌢ N2) (0 ⊗ q1) (NONE::munge n2 (ZIP (s2,nlist2))) (1 ⊗ q2)’
-     by (irule (NF_transition_rules |> SPEC_ALL |> CONJUNCT2) >> simp[] >>
-         qexists_tac ‘1 ⊗ N2.q_0’ >> simp[] >> simp[machine_link_def]) >>
-  drule_all NF_transition_concat >> rw[munge_middle_none]
-  >- (‘s1 = [] ∧ nlist1 = []’ by metis_tac[ZIP_EQ_NIL] >> rw[] >> metis_tac[])>>
-  simp[PULL_EXISTS] >>
-  map_every qexists_tac [
-    ‘n1’, ‘FRONT nlist1 ++ (n2 + LAST nlist1 + 1) :: nlist2’, ‘q2’
-  ] >> rw[]
-  >- (Cases_on‘nlist1 = []’
-      >- (fs[] >> rw[] >> fs[])
-      >> rw[rich_listTheory.LENGTH_FRONT]
-      >> Cases_on ‘LENGTH s1’ >> simp[] >> fs[]) >> pop_assum mp_tac >>
-  qmatch_abbrev_tac‘NF_transition _ _ l1 _ ==> NF_transition _ _ l2 _’ >>
-  ‘l1 = l2’ suffices_by fs[] >> simp[Abbr‘l1’,Abbr‘l2’] >>
-  ‘s1 ≠ [] ∧ nlist1 ≠ []’ by (rfs[ZIP_EQ_NIL] >> rpt strip_tac >> fs[]) >>
-  ‘0 < LENGTH nlist1’ by (Cases_on ‘nlist1’ >> fs[]) >>
-  simp[FRONT_ZIP, LAST_ZIP, GSYM ZIP_APPEND, LENGTH_FRONT] >>
-  simp[GSYM ZIP_SNOC, Excl "LIST_EQ_SIMP_CONV",LENGTH_FRONT,GSYM SNOC_APPEND] >>
-  simp[SNOC_APPEND, APPEND_FRONT_LAST]
-QED
-
-(*---------------------------------------------------------------------------*)
-(* Closure under Kleene star                                                 *)
-(*---------------------------------------------------------------------------*)
-
-Definition machine_star_def:
-  machine_star N =
-   <|
-     Q :=  IMAGE SUC N.Q ∪ {0} ;
-     A :=  N.A ;
-     q_0 := 0 ;
-     tf := λs0 copt.
-             case s0 of
-               0 => if copt = NONE then {SUC N.q_0} else ∅
-             | SUC s0' =>
-                if copt = NONE ∧ s0' ∈ N.C then
-                  IMAGE SUC (N.tf s0' copt) ∪ {0}
-                else IMAGE SUC (N.tf s0' copt) ;
-     C := {0};
-   |>
-End
-
-Theorem wfNFA_machine_star:
-  wfNFA N ⇒ wfNFA (machine_star N)
-Proof
-  simp[wfNFA_def, machine_star_def, DISJ_IMP_THM, PULL_EXISTS,
-       AllCaseEqs()] >>
-  rw[] >> simp[]
-  >- (simp[] >> fs[SUBSET_DEF, PULL_EXISTS] >> metis_tac[])
-  >- (rw[] >> fs[SUBSET_DEF, PULL_EXISTS] >> metis_tac[])
-  >- metis_tac[TypeBase.nchotomy_of “:num”]
-QED
-
-Theorem machine_star_accepting_states[simp]:
-  (machine_star N).C = {0}
-Proof
-  simp[machine_star_def]
-QED
-
-Theorem machine_star_alphabet[simp]:
-  (machine_star N).A = N.A
-Proof
-  simp[machine_star_def]
-QED
-
-Theorem machine_star_tf0[simp]:
-  (machine_star N).tf 0 NONE = {SUC N.q_0} ∧
-  (machine_star N).tf 0 (SOME c) = ∅ ∧
-  ((q ∈ (machine_star N).tf 0 cO) ⇔ (cO = NONE ∧ q = SUC N.q_0))
-Proof
-  rw[machine_star_def]
-QED
-
-Theorem machine_star_q_0[simp]:
-  (machine_star N).q_0 = 0
-Proof
-  simp[machine_star_def]
-QED
-
-Theorem machine_star_tfSUC:
-  (machine_star N).tf (SUC q_0) (SOME c) =
-    {SUC q | q ∈ N.tf q_0 (SOME c)} ∧
-  (machine_star N).tf (SUC q_0) NONE =
-    {SUC q | q ∈ N.tf q_0 NONE} ∪
-    (if q_0 ∈ N.C then {0} else ∅) ∧
-  (SUC q ∈ (machine_star N).tf (SUC q_0) cO ⇔
-    q ∈ N.tf q_0 cO)
-Proof
-  simp[machine_star_def, EXTENSION] >> rw[]
-QED
-
-Theorem NF_transition_machine_star_SUC:
-∀q cs. NF_transition (machine_star N) (SUC q) cs 0 ⇒
-  ∃s1 s2 nc. cs = s1++[NONE]++s2 ∧ nc ∈ N.C ∧ NF_transition N q s1 nc ∧
-             NF_transition (machine_star N) 0 s2 0
-Proof
-  Induct_on ‘NF_transition’ >> rw[] >>
-  rename [‘qI ∈ _ _ _’] >> Cases_on ‘qI’
-  >- (Cases_on ‘c’ >> fs[machine_star_tfSUC] >>
-      rw[] >> Cases_on ‘q ∈ N.C’ >> fs[] >>
-      rw[] >> MAP_EVERY qexists_tac [‘[]’,‘cs’,‘q’] >>
-      simp[NF_transition_rules])
-  >- (fs[] >> MAP_EVERY qexists_tac [‘c::s1’,‘s2’,‘nc’] >> simp[] >>
-      fs[machine_star_tfSUC] >> metis_tac[NF_transition_rules])
-QED
-
-Theorem NF_transition_machine_star:
-  NF_transition (machine_star N) 0 cs 0 ⇒
-  cs = [] ∨
-  ∃s1 s2 nc. cs = NONE::s1++[NONE]++s2 ∧ nc ∈ N.C ∧ NF_transition N N.q_0 s1 nc ∧
-             NF_transition (machine_star N) 0 s2 0
-Proof
-  Cases_on ‘cs’ >> simp[] >>
-  simp[SimpL“$==>”, Once NF_transition_cases] >>
-  csimp[] >> metis_tac[NF_transition_machine_star_SUC]
-QED
-
-Theorem LENGTH_mungeNIL[simp]:
-  LENGTH (munge n []) = n
-Proof
-  Induct_on ‘n’ >> simp[munge_SUC]
-QED
-
-Theorem mungeNIL_IFF:
-  (munge n [] = s ⇔ s = REPLICATE n NONE) ∧
-  (s = munge n [] ⇔ s = REPLICATE n NONE)
-Proof
-  simp[munge_def, EQ_SYM_EQ]
-QED
-
-(*---------------------------------------------------------------------------*)
-(* Already in numLib somewhere                                               *)
-(*---------------------------------------------------------------------------*)
-
-Triviality EXISTS_NUM:
-  (∃n. P n) ⇔ P 0 ∨ (∃n. P (SUC n))
-Proof
-  rw[EQ_IMP_THM] >- (Cases_on ‘n’ >> metis_tac[]) >>
-  metis_tac[]
-QED
-
-Triviality FORALL_NUM:
-  (∀n. P n) ⇔ P 0 ∧ ∀n. P (SUC n)
-Proof
-  rw[EQ_IMP_THM] >> Cases_on ‘n’ >> simp[]
-QED
-
-Theorem drop_epsilon_EQ_NIL:
-  drop_epsilon l = [] ⇔ ∃n. l = REPLICATE n NONE
-Proof
-  Induct_on ‘l’ >> simp[] >>
-  Cases >> simp[] >- simp[Once EXISTS_NUM, SimpRHS] >>
-  Cases >> simp[]
-QED
-
-Triviality REPLICATE_NIL'[simp]:
-  [] = REPLICATE n e ⇔ n = 0
-Proof
-  metis_tac[REPLICATE_NIL]
-QED
-
-Theorem REPLICATE_EQ_APPEND:
-  ∀n e l1 l2.
-     REPLICATE n e = l1 ++ l2 ⇔
-     ∃n1 n2. n1 + n2 = n ∧ l1 = REPLICATE n1 e ∧ l2 = REPLICATE n2 e
-Proof
-  Induct_on ‘n’ >> simp[APPEND_EQ_CONS, PULL_EXISTS] >>
-  rw[EQ_IMP_THM] >> simp[]
-  >- (simp[Once EXISTS_NUM, arithmeticTheory.ADD_CLAUSES] >> metis_tac[]) >>
-  Cases_on ‘n1’ >> simp[] >> fs[arithmeticTheory.ADD_CLAUSES] >>
-  metis_tac[]
-QED
-
-Definition munge'_def[simp]:
-  munge' 0 [] = [] ∧
-  munge' 0 ((c,n)::t) = SOME c :: munge' n t ∧
-  munge' (SUC n) cs = NONE :: munge' n cs
-End
-
-Theorem munge_alt_def:
-  ∀n l. munge n l = munge' n l
-Proof
-  ho_match_mp_tac munge'_ind >>
-  rw[munge_SUC,munge_eq_nil]
-QED
-
-Theorem munge'_split:
-  ∀n l str nlist s1 s2.
-   munge' n l = s1 ⧺ [NONE] ⧺ s2 ∧
-   ZIP (str,nlist) = l ∧
-   LENGTH str = LENGTH nlist ⇒
-   ∃nR strR nlistR.
-    s2 = munge' nR (ZIP (strR,nlistR)) ∧
-    LENGTH strR = LENGTH nlistR ∧
-    str = drop_epsilon s1 ++ strR
-Proof
-  ho_match_mp_tac munge'_ind >>
-  simp[] >> rw[] >> Cases_on ‘n’ >> fs[] >>
-  Cases_on ‘s1’ >> fs[] >> rw[]
-  >- (Cases_on ‘str’ >> Cases_on ‘nlist’ >> fs[] >>
-      last_x_assum irule >> metis_tac[])
-  >- (Cases_on ‘str’ >> Cases_on ‘nlist’ >> fs[] >>
-      rw[] >> last_x_assum irule >> metis_tac[])
   >- metis_tac[]
-  >- (last_x_assum irule >> metis_tac[])
-  >- metis_tac[munge'_def]
-  >- (last_x_assum irule >> metis_tac[])
+  >- (fs[] >> metis_tac[])
 QED
 
-Theorem munge_split:
- ∀str n nlist s1 s2.
-   munge n (ZIP (str,nlist)) = (s1 ⧺ [NONE] ⧺ s2) ∧
-   LENGTH str = LENGTH nlist ⇒
-   ∃nR strR nlistR.
-    s2 = munge nR (ZIP (strR,nlistR)) ∧
-    LENGTH strR = LENGTH nlistR ∧
-    str = drop_epsilon s1 ++ strR
+Theorem wf_nfa_union:
+  wf_nfa N1 ∧ wf_nfa N2 ⇒ wf_nfa (nfa_union N1 N2)
 Proof
- metis_tac[munge_alt_def,munge'_split]
+  rw [wf_nfa_def,nfa_union_def,SUBSET_DEF]
+  >- (rw [GSPEC_IMAGE, o_DEF,pairTheory.LAMBDA_PROD] >>
+      irule IMAGE_FINITE >> irule SUBSET_FINITE >>
+      qexists ‘N1.Q CROSS N2.Q’ >> rw[] >>
+      rw [SUBSET_DEF,CROSS_DEF,pairTheory.LAMBDA_PROD,pairTheory.FORALL_PROD])
+  >- metis_tac[]
+  >- metis_tac[]
+  >- metis_tac[]
+  >- (fs[] >> metis_tac[])
 QED
 
-Theorem munge_drop_epsilon_exists:
-  ∀s.
-    ∃n nlist.
-      munge n (ZIP (drop_epsilon s, nlist)) = s ∧
-      LENGTH nlist = LENGTH (drop_epsilon s)
+Triviality nfa_dot_builtin_simps[simp]:
+  (∀q. q ∈ (nfa_dot N1 N2).Q <=> q ∈ N1.Q ∨ q ∈ N2.Q) ∧
+  (∀a. a ∈ (nfa_dot N1 N2).Sigma ⇔ a ∈ N1.Sigma ∧ a ∈ N2.Sigma) ∧
+  (nfa_dot N1 N2).initial = N1.initial ∧
+  (nfa_dot N1 N2).final = N2.final
 Proof
-  metis_tac[munge_exists,drop_epsilon_munge]
+  rw[nfa_dot_def]
 QED
 
-Theorem NF_transition_machine_star_i:
-  NF_transition M q_0 cs q ⇒ NF_transition (machine_star M) (SUC q_0) cs (SUC q)
+Triviality nfa_plus_builtin_simps[simp]:
+  (nfa_plus N).Sigma = N.Sigma ∧
+  (nfa_plus N).Q = N.Q ∧
+  (nfa_plus N).initial = N.initial ∧
+  (nfa_plus N).final = N.final
 Proof
-  Induct_on ‘NF_transition’ >> simp[NF_transition_rules] >> rw[] >>
-  irule (NF_transition_rules |> SPEC_ALL |> CONJUNCT2) >>
-  rw[] >> qexists_tac ‘SUC q_0'’ >> rw[] >> rw[machine_star_def] >> rw[]
+  rw[nfa_plus_def]
 QED
 
-Theorem NF_transition_cons =
-        NF_transition_rules |> SPEC_ALL |> CONJUNCT2 |> Q.GEN‘a’;
-
-Theorem machine_star_single:
-  x ∈ recogLangN M0 ⇒ x ∈ recogLangN (machine_star M0)
+Theorem wf_nfa_dot:
+  wf_nfa N1 ∧ wf_nfa N2 ∧ N1.Q ∩ N2.Q = {} ==> wf_nfa (nfa_dot N1 N2)
 Proof
-  simp[recogLangN_def, Sipser_ND_Accepts_NF_transition_l] >>
-  rw[] >> drule NF_transition_machine_star_i >> rw[] >>
-  qexists_tac ‘NONE::l ++ [NONE]’ >> simp[] >> irule NF_transition_cons >>
-  rw[] >> irule NF_transition_concat >> rw[] >> qexists_tac ‘SUC q’ >> rw[] >>
-  irule NF_transition_cons >> rw[] >> qexists_tac ‘0’ >>
-  rw[NF_transition_rules] >> rw[machine_star_def]
+  fs [wf_nfa_def, nfa_dot_def] >> rw[]
+  >- metis_tac [SUBSET_UNION_RIGHT]
+  >- metis_tac [SUBSET_UNION_RIGHT,UNION_COMM]
+  >- (rw[]
+       >- metis_tac [SUBSET_UNION_RIGHT,UNION_COMM]
+       >- metis_tac [SUBSET_UNION_RIGHT,UNION_COMM]
+       >- (simp [Once UNION_COMM] >> irule SUBSET_UNION_RIGHT >>
+           rw [SUBSET_DEF] >> metis_tac [SUBSET_DEF]))
+  >- (rw[] >> fs[EXTENSION] >> rw[]
+       >- metis_tac [SUBSET_UNION_RIGHT,UNION_COMM]
+       >- (gvs [SUBSET_DEF] >> metis_tac[])
+       >- (gvs [SUBSET_DEF] >> metis_tac[])
+       >- (simp [Once UNION_COMM] >> irule SUBSET_UNION_RIGHT >> metis_tac[]))
 QED
 
-Theorem thm_1_50:
-  regularLanguage L ⇒ regularLanguage (KSTAR L)
+Theorem wf_nfa_plus:
+  wf_nfa N ==> wf_nfa (nfa_plus N)
 Proof
-  simp[corollary_1_40] >>
-  disch_then (qx_choose_then ‘M0’ strip_assume_tac) >>
-  qexists_tac ‘machine_star M0’ >>
-  simp[wfNFA_machine_star, KSTAR_DEF_ALT, Once EXTENSION, PULL_EXISTS,EQ_IMP_THM] >>
-  qx_gen_tac ‘str’ >> conj_tac
-  >- (simp[recogLangN_def, Sipser_ND_Accepts_NF_transition] >>
-      rw[] >> pop_assum mp_tac >>
-      completeInduct_on ‘LENGTH (munge n (ZIP (str,nlist)))’ >>
-      fs[PULL_FORALL] >> rw[] >> drule NF_transition_machine_star >>
-      rw[]
-      >- (rfs[ZIP_EQ_NIL] >> qexists_tac ‘0’ >> rw[DOTn_def]) >>
-      rename1 ‘NONE::(s1 ++ [NONE] ++ s2)’ >>
-      ‘NONE::(s1 ++ [NONE] ++ s2) = (NONE::s1 ++ [NONE] ++ s2)’
-        by rw[] >>
-      pop_assum SUBST_ALL_TAC >>
-      drule_then strip_assume_tac munge_split >> rw[] >>
-      rfs[] >> rw[] >>
-      first_x_assum (first_assum o mp_then.mp_then (mp_then.Pos last) mp_tac) >>
-      simp[] >> disch_then (qx_choose_then ‘N’ strip_assume_tac) >>
-      qexists_tac ‘SUC N’ >>
-      simp[DOTn_def] >>
-      simp[dot_def] >>
-      qexistsl_tac [‘drop_epsilon s1’,‘strR’] >>
-      simp[recogLangN_def,Sipser_ND_Accepts_NF_transition] >>
-      metis_tac[munge_drop_epsilon_exists]) >>
-  qx_gen_tac ‘n’ >> MAP_EVERY qid_spec_tac [‘str’,‘n’] >>
-  fs[recogLangN_def, Sipser_ND_Accepts_NF_transition_l] >>
-  rw[] >> pop_assum mp_tac >> qid_spec_tac ‘str’ >>
-  Induct_on ‘n’
-  >- (simp[DOTn_def] >> qexists_tac ‘[]’ >> rw[NF_transition_rules])
-  >> simp[DOTn_def, dot_def, PULL_EXISTS] >> rw[] >>
-  first_x_assum (drule_then strip_assume_tac) >>
-  qexists_tac ‘NONE::l++[NONE]++l'’ >>
-  rw[] >> irule NF_transition_cons >> rw[] >> irule NF_transition_concat >>
-  qexists_tac ‘0’ >> rw[] >> irule NF_transition_concat >>
-  qexists_tac ‘SUC q’ >> rw[]
-  >- rw[NF_transition_machine_star_i]
-  >> irule NF_transition_cons >> rw[] >> qexists_tac ‘0’ >>
-  rw[NF_transition_rules] >> rw[machine_star_def]
+  rw [wf_nfa_def, nfa_plus_def,SUBSET_DEF] >>
+  pop_keep_tac >> rw[] >> metis_tac []
 QED
 
-(* TODO: Closure under complement, reversal *)
-
-(*===========================================================================*)
-(* Regular expressions. A more elaborate version is in regexpScript, need to *)
-(* reconcile.                                                                *)
-(*===========================================================================*)
-
-Datatype:
-regexp = Concat regexp regexp |
-         Star regexp |
-         Alt regexp regexp |
-         Single num |
-         Epsilon |
-         Empty
-End
-
-Definition regexp_lang[simp]:
-  regexp_lang (Concat r1 r2) = regexp_lang r1 dot regexp_lang r2 ∧
-  regexp_lang (Star r) = KSTAR (regexp_lang r) ∧
-  regexp_lang (Alt r1 r2) = regexp_lang r1 ∪ regexp_lang r2 ∧
-  regexp_lang (Single c) = { [c] } ∧
-  regexp_lang Epsilon = { [] } ∧
-  regexp_lang Empty = {}
-End
-
-Theorem lemma_1_55:
-  ∀r. regularLanguage (regexp_lang r)
+Theorem is_dfa_compl:
+  is_dfa N ⇒ is_dfa (nfa_compl N)
 Proof
-  Induct >> simp[]
-  >- metis_tac[thm_1_47]
-  >- metis_tac[thm_1_50]
-  >- metis_tac[thm_1_25]
-  >- (rw[regularLanguage_def] >>
-      qexists_tac ‘<| Q := {0;1;2};
-                      A := {n};
-                      tf := (λs0 c. if c = n ∧ s0 = 1 then 2 else 0);
-                      q_0 := 1;
-                      C := {2};|>’ >>
-      conj_asm1_tac >>
-      rw[wf_dfa_def, recogLangD_def] >>
-      rw[EXTENSION, has_Accepting_Execution_Delta_coincide] >>
-      rw[accepts_def] >> eq_tac
-      >- (Cases_on ‘x’ >> rw[]
-          >- (Cases_on ‘t’ >> fs[Delta_def] >> Induct_on‘t'’ >> fs[])
-          >> Induct_on ‘t’ >> fs[])
-      >> simp[])
-  >- (rw[regularLanguage_def] >>
-      qexists_tac ‘<| Q := {0;1};
-                      A := {};
-                      tf := (λs0 c. 0);
-                      q_0 := 1;
-                      C := {1};|>’ >>
-      conj_asm1_tac >>
-      rw[wf_dfa_def, recogLangD_def] >>
-      rw[EXTENSION, has_Accepting_Execution_Delta_coincide] >>
-      rw[accepts_def] >> eq_tac
-      >- (Cases_on ‘x’ >> rw[] >> Induct_on ‘t’ >> simp[])
-      >> simp[])
-  >> rw[regularLanguage_def] >>
-     qexists_tac ‘<| Q := {0;1;2};
-                      A := {};
-                      tf := (λs0 c. 0);
-                      q_0 := 1;
-                      C := {2};|>’ >>
-     conj_asm1_tac >>
-     rw[wf_dfa_def, recogLangD_def] >>
-     rw[EXTENSION, has_Accepting_Execution_Delta_coincide] >>
-     rw[accepts_def] >>
-     Cases_on ‘x’ >> rw[] >> Induct_on ‘t’ >> rw[]
+  rw [is_dfa_def]
+  >- metis_tac [wf_nfa_compl]
+  >- simp[nfa_compl_def]
+  >- fs[nfa_compl_def]
+QED
+
+Theorem is_dfa_inter:
+ is_dfa N1 ∧ is_dfa N2 ⇒ is_dfa (nfa_inter N1 N2)
+Proof
+ rw [is_dfa_def]
+ >- metis_tac [wf_nfa_inter]
+ >- (rw [nfa_inter_def,EXTENSION] >> metis_tac[])
+ >- (ntac 2 pop_keep_tac >> rw [nfa_inter_def,EXTENSION,PULL_EXISTS] >>
+     ‘∃qa qb. {qa} = N1.delta q1 a ∧
+              {qb} = N2.delta q2 a’ by metis_tac[] >>
+     qexists_tac ‘qa ⊗ qb’ >> rw[EQ_IMP_THM]
+     >- (RULE_ASSUM_TAC GSYM >> rfs[])
+     >- metis_tac [EXTENSION,IN_INSERT]
+     >- metis_tac [EXTENSION,IN_INSERT])
+QED
+
+Theorem is_dfa_union:
+ is_dfa N1 ∧ is_dfa N2 ⇒ is_dfa (nfa_union N1 N2)
+Proof
+ rw [is_dfa_def]
+ >- metis_tac [wf_nfa_union]
+ >- (rw [nfa_union_def,EXTENSION] >> metis_tac[])
+ >- (ntac 2 pop_keep_tac >> rw [nfa_union_def,EXTENSION,PULL_EXISTS] >>
+     ‘∃qa qb. {qa} = N1.delta q1 a ∧
+              {qb} = N2.delta q2 a’ by metis_tac[] >>
+     qexists_tac ‘qa ⊗ qb’ >> rw[EQ_IMP_THM]
+     >- (RULE_ASSUM_TAC GSYM >> rfs[])
+     >- metis_tac [EXTENSION,IN_INSERT]
+     >- metis_tac [EXTENSION,IN_INSERT])
 QED
 
 (*---------------------------------------------------------------------------*)
-(* Every FSA has a corresponding regexp, via GNFAs                           *)
+(* Correctness of constructions                                              *)
 (*---------------------------------------------------------------------------*)
 
-(* Definition 1.64 *)
-Datatype:
-  gnfa = <|
-    Q : state set;
-    A : symbol set;
-    tf : state -> state -> regexp;
-    q_0 : state;
-    C : state;
-  |>
-End
-
-Definition wfm_gnfa_def:
-  wfm_gnfa G ⇔ FINITE G.Q ∧ G.q_0 ∈ G.Q ∧ G.C ∈ G.Q ∧ G.q_0 ≠ G.C ∧
-               (∀s. G.tf s G.q_0 = Empty) ∧
-               (∀s. G.tf G.C  s = Empty)
-End
-
-Inductive gnfa_accepts:
-[~nil:]
-  ∀q_0. q_0 IN G.Q ⇒ gnfa_accepts G q_0 [] q_0
-[~step:]
-  ∀q' q. q_0 IN G.Q ∧ q' IN G.Q ∧ c1 ∈ regexp_lang (G.tf q_0 q') ∧
-         gnfa_accepts G q' c2 q ⇒
-         gnfa_accepts G q_0 (c1++c2) q
-End
-
-Inductive charset_reR:
-  charset_reR ∅ Empty ∧
-  (e ∉ s ∧ charset_reR s re ⇒ charset_reR (e INSERT s) (Alt (Single e) re))
-End
-
-Theorem charset_reR_correct:
-  charset_reR cs re ⇒ regexp_lang re = {[c] | c ∈ cs}
+Theorem dfa_compl_correct :
+  is_dfa N ⇒
+  ∀w. w ∈ nfa_lang (nfa_compl N) <=>
+      w ∈ (KSTAR (IMAGE Symbol_Word N.Sigma) DIFF (nfa_lang N))
 Proof
-  Induct_on ‘charset_reR’ >> rw[EXTENSION] >> metis_tac[]
+  rw [in_nfa_lang, nfa_compl_def, EQ_IMP_THM]
+  >- (rw_tac std_ss [GSYM IMP_DISJ_THM] >> spose_not_then assume_tac >>
+      ‘qs = qs'’ by
+        (irule dfa_execution_deterministic >> rw [] >> metis_tac[]) >>
+      rw[] >> metis_tac[])
+  >- metis_tac [NOT_EVERY]
+  >- (drule_all dfa_execution >> rw[] >> first_x_assum drule >> rw[]
+      >- metis_tac [EXTENSION,IN_INSERT]
+      >- (qexists_tac ‘qs’ >> rw[]
+          >- metis_tac [EXTENSION,IN_INSERT]
+          >- (fs [EVERY_EL] >>
+              drule_then (fn th => SUBST_TAC [SYM th]) EL_LENGTH_LAST >>
+              first_x_assum irule >> decide_tac)
+          >- (first_x_assum drule >> disch_then (SUBST_ALL_TAC o SYM) >>
+              metis_tac [IN_INSERT]))
+      >- (first_x_assum drule >> disch_then (SUBST_ALL_TAC o SYM) >>
+          metis_tac [IN_INSERT]))
 QED
 
-Theorem charset_reR_exists:
-  ∀cs. FINITE cs ⇒ ∃re. charset_reR cs re
-Proof
-  Induct_on ‘FINITE’ >> metis_tac[charset_reR_rules]
-QED
-
-Definition charset_re_def:
-  charset_re cs = @re. charset_reR cs re
-End
-
-Theorem regexp_lang_charset_re:
-  ∀cs. FINITE cs ⇒ regexp_lang (charset_re cs) = {[c] | c ∈ cs}
-Proof
-  rw[charset_re_def] >> SELECT_ELIM_TAC >>
-  simp[charset_reR_correct, charset_reR_exists]
-QED
-
-Definition dfa_to_gnfa_def:
-  dfa_to_gnfa d = <| Q := {0; 1} ∪ IMAGE ($+2) d.Q;
-                          A := d.A;
-                          tf := (λs1 s2. if s1 = 0 ∧ s2 = d.q_0+2 then Epsilon
-                                         else if s1 ∈ IMAGE ($+2) d.C ∧ s2 = 1
-                                         then
-                                           Epsilon
-                                         else if 1 < s1 ∧ 1 < s2 then
-                                         let s = {cs | d.tf (s1-2) cs = s2-2}
-                                         in
-                                            charset_re s
-                                         else Empty);
-                          q_0 := 0;
-                          C := 1; |>
-End
-
-Theorem dfa_to_gnfa_wfm:
-  wf_dfa d ⇒ wfm_gnfa (dfa_to_gnfa d)
-Proof
-  rw[wf_dfa_def, wfm_gnfa_def, dfa_to_gnfa_def]
-QED
-
-Theorem dfa_to_gnfa_q_0[simp]:
-  ∀d. (dfa_to_gnfa d).q_0 = 0
-Proof
-  rw[dfa_to_gnfa_def]
-QED
-
-Theorem dfa_to_gnfa_tf_0[simp]:
-  ∀d x. ((dfa_to_gnfa d).tf 0 x = if x = d.q_0 + 2 then Epsilon else Empty) ∧
-        ((dfa_to_gnfa d).tf x 0 = Empty)
-Proof
-  rw[dfa_to_gnfa_def]
-QED
-
-Theorem dfa_to_gnfa_Q[simp]:
-  ∀d. (dfa_to_gnfa d).Q = {0;1} ∪ {q+2 | q ∈ d.Q}
-Proof
-  rw[EXTENSION ,dfa_to_gnfa_def]
-QED
-
-Theorem dfa_to_gnfa_never_looks_back:
-  ∀d s. gnfa_accepts (dfa_to_gnfa d) s cs 0 ⇒ (s = 0 ∧ cs = [])
-Proof
-  rpt gen_tac >> Induct_on ‘gnfa_accepts’ >>
-  rw[] >> fs[]
-QED
-
-Theorem dfa_prod_gnfa_shuffle_start:
-  ∀d cs es. gnfa_accepts (dfa_to_gnfa d) (d.q_0 + 2) cs es
-              ⇔ es ≠ 0 ∧ gnfa_accepts (dfa_to_gnfa d) (dfa_to_gnfa d).q_0 cs es
-Proof
-  rw[SimpRHS, Once gnfa_accepts_cases] >>
-  simp_tac (srw_ss () ++ boolSimps.COND_elim_ss) [] >>
-  rw[EQ_IMP_THM] >>
-  fs[Once gnfa_accepts_cases]
-  >- (strip_tac >>
-      fs[] >>
-      drule_all_then strip_assume_tac dfa_to_gnfa_never_looks_back >>
-      fs[] >> rw[] >> fs[])
-  >- (rpt strip_tac >> rw[] >> fs[] >>
-      metis_tac[dfa_to_gnfa_never_looks_back, DECIDE “1≠0”]) >>
-  rpt strip_tac >> rw[] >> fs[] >>
-  metis_tac[dfa_to_gnfa_never_looks_back, DECIDE “q+2≠0”]
-QED
-
-Theorem dfa_to_gnfa_c[simp]:
-  (dfa_to_gnfa d).C = 1
-Proof
-  rw[dfa_to_gnfa_def]
-QED
-
-Theorem dfa_to_gnfa_final_state_no_op:
-∀d s.
-  wf_dfa d ∧ s ∈ d.Q ∧ s ∈ d.C
+Theorem dfa_inter_correct :
+  is_dfa N1 ∧ is_dfa N2 ∧ N1.Sigma = N2.Sigma
   ⇒
-  gnfa_accepts (dfa_to_gnfa d) (s + 2) [] 1
+  ∀w. w ∈ nfa_lang (nfa_inter N1 N2) <=>
+      w ∈ nfa_lang N1 ∧ w ∈ nfa_lang N2
 Proof
-  rw[] >>
-  ‘[] ∈ regexp_lang ((dfa_to_gnfa d).tf (s+2) 1)’ by rw[dfa_to_gnfa_def] >>
-  ‘1 ∈ (dfa_to_gnfa d).Q ∧ s+2 ∈ (dfa_to_gnfa d).Q’ by simp[] >>
-  dxrule_then (drule_then (drule_then strip_assume_tac)) gnfa_accepts_step >>
-  fs[] >> simp[gnfa_accepts_rules]
+  strip_tac >> rw [in_nfa_lang, nfa_inter_def, EQ_IMP_THM]
+  >- (qexists_tac ‘MAP nfst qs’ >> rw[]
+      >- (Cases_on ‘qs’ >> fs[])
+      >- (Cases_on ‘qs’ >> fs[])
+      >- (first_x_assum drule >> rw[EL_MAP] >> rw[]))
+  >- (qexists_tac ‘MAP nsnd qs’ >> rw[]
+      >- (Cases_on ‘qs’ >> fs[])
+      >- (Cases_on ‘qs’ >> fs[])
+      >- (first_x_assum drule >> rw[EL_MAP] >> rw[]))
+  >- (qexists_tac ‘MAP2 npair qs qs'’ >> rw[]
+      >- (Cases_on ‘qs’ >> Cases_on ‘qs'’ >> fs[])
+      >- (‘qs ≠ [] ∧ qs' ≠ []’ by (Cases_on ‘qs’ >> Cases_on ‘qs'’ >> fs[]) >>
+          rw[LAST_MAP2])
+      >- (ntac 2 (first_x_assum drule) >> ntac 2 disch_tac >>
+          qexists_tac ‘EL (n+1) qs’ >> qexists_tac ‘EL (n+1) qs'’ >> rw[EL_MAP2]))
 QED
 
-Theorem Delta_c_in_A:
-  ∀d s c cs. Delta d (d.tf s c) cs ∈ d.C ∧ wf_dfa d ⇒ c ∈ d.A
+Theorem dfa_union_correct :
+  is_dfa N1 ∧ is_dfa N2 ∧ N1.Sigma = N2.Sigma
+  ⇒
+  ∀w. w ∈ nfa_lang (nfa_union N1 N2) <=>
+      w ∈ nfa_lang N1 ∨ w ∈ nfa_lang N2
 Proof
-  CCONTR_TAC >> fs[] >> ‘d.tf s c = 0’ by fs[wf_dfa_def] >> fs[] >>
-  drule_then strip_assume_tac Delta_0_Sink >> metis_tac[wf_dfa_def]
+  strip_tac >> rw [in_nfa_lang, nfa_union_def, EQ_IMP_THM]
+  >- (disj1_tac >> qexists_tac ‘MAP nfst qs’ >> rw[]
+      >- (Cases_on ‘qs’ >> fs[])
+      >- (Cases_on ‘qs’ >> fs[])
+      >- (first_x_assum drule >> rw[EL_MAP] >> rw[]))
+  >- (disj2_tac >> qexists_tac ‘MAP nsnd qs’ >> rw[]
+      >- (Cases_on ‘qs’ >> fs[])
+      >- (Cases_on ‘qs’ >> fs[])
+      >- (first_x_assum drule >> rw[EL_MAP] >> rw[]))
+  >- metis_tac[]
+  >- (qpat_forget_tac ‘N1.Sigma = N2.Sigma’ >> qpat_forget_tac ‘is_dfa N1’ >>
+      drule_all dfa_execution >> rw[] >>
+      qexists_tac ‘MAP2 npair qs qs'’ >> rw[]
+      >- (Cases_on‘qs’ >> Cases_on‘qs'’ >> fs[] >> metis_tac[EXTENSION,IN_INSERT])
+      >- (‘qs ≠ [] ∧ qs' ≠ []’ by (Cases_on ‘qs’ >> Cases_on ‘qs'’ >> fs[]) >>
+          rw[LAST_MAP2] >> disj1_tac >> drule_all EVERY_LAST >> rw[])
+      >- (ntac 2 (first_x_assum drule) >> ntac 2 disch_tac >>
+          qexists_tac ‘EL (n+1) qs’ >> qexists_tac ‘EL (n+1) qs'’ >> rw[EL_MAP2] >>
+          metis_tac [EXTENSION,IN_INSERT]))
+  >- metis_tac[]
+  >- (qpat_x_assum ‘N1.Sigma = N2.Sigma’ (SUBST_ALL_TAC o GSYM) >>
+      qpat_forget_tac ‘is_dfa N2’ >> drule_all dfa_execution >> rw[] >>
+      qexists_tac ‘MAP2 npair qs' qs’ >> rw[]
+      >- (Cases_on‘qs’ >> Cases_on‘qs'’ >> fs[] >> metis_tac[EXTENSION,IN_INSERT])
+      >- (‘qs ≠ [] ∧ qs' ≠ []’ by (Cases_on ‘qs’ >> Cases_on ‘qs'’ >> fs[]) >>
+          rw[LAST_MAP2] >> disj2_tac >> drule_all EVERY_LAST >> rw[])
+      >- (ntac 2 (first_x_assum drule) >> ntac 2 disch_tac >>
+          qexists_tac ‘EL (n+1) qs'’ >> qexists_tac ‘EL (n+1) qs’ >>
+          rw[EL_MAP2] >> metis_tac [EXTENSION,IN_INSERT]))
 QED
 
-Theorem gnfa_error_sink:
-  ∀d. (wf_dfa d ⇒ ∀q cs. gnfa_accepts (dfa_to_gnfa d) 2 cs q ⇒ (q = 2))
+Theorem dfa_union_closed:
+  is_dfa N1 ∧ is_dfa N2 ∧ N1.Sigma = N2.Sigma
+  ⇒
+  nfa_lang N1 ∪ nfa_lang N2 ∈ NFA_LANGS
 Proof
-  ntac 2 strip_tac >>
-  Induct_on ‘gnfa_accepts’ >>
-  rw[] >> fs[]
-  >- (rw[] >> fs[dfa_to_gnfa_def] >> rfs[wf_dfa_def]) >>
-  rw[] >>
-  pop_assum irule >>
-  pop_assum kall_tac >>
-  fs[dfa_to_gnfa_def] >>
-  rfs[wf_dfa_def] >> rw[] >> CCONTR_TAC >> fs[] >>
-  fs[regexp_lang_charset_re]
+  rw [NFA_LANGS_def] >> qexists_tac ‘nfa_union N1 N2’ >>
+  ‘wf_nfa N1 ∧ wf_nfa N2’ by metis_tac [is_dfa_def] >>
+  rw [wf_nfa_union,EXTENSION,dfa_union_correct]
 QED
 
-Theorem Delta_append[simp]:
-  ∀d s c1 c2. Delta d s (c1++c2) = Delta d (Delta d s c1) c2
-Proof
-  Induct_on ‘c1’ >> rw[]
-QED
+(*---------------------------------------------------------------------------*)
+(* A regular language L is a subset of A*, where A is a finite alphabet. The *)
+(* languages is defined by the strings accepting by an NFA.                  *)
+(*---------------------------------------------------------------------------*)
 
-Theorem gnfa_accepts_1_to_1:
-  ∀d cs. wf_dfa d ∧ gnfa_accepts (dfa_to_gnfa d) 1 cs 1 ⇒ cs = []
-Proof
-  rw[Once gnfa_accepts_cases] >> qpat_x_assum ‘c1 ∈ _’ mp_tac >>
-  rw[dfa_to_gnfa_def]
-QED
-
-Theorem gnfa_accepts_2_to_1:
-  ∀d cs. wf_dfa d ⇒ ¬gnfa_accepts (dfa_to_gnfa d) 2 cs 1
-Proof
-  ‘∀d x cs y. gnfa_accepts (dfa_to_gnfa d) x cs y ⇒ x = 2 ⇒ y = 1 ⇒ wf_dfa d ⇒ F’
-    suffices_by metis_tac[] >> gen_tac >>
-  ho_match_mp_tac gnfa_accepts_ind >> rw[] >>
-  fs[dfa_to_gnfa_def] >> strip_tac >> fs[] >> fs[wf_dfa_def] >>
-  Cases_on ‘1 < x'’ >> fs[regexp_lang_charset_re]
-QED
-
-Theorem dfa_to_gnfa_correct:
-  ∀d. wf_dfa d ⇒
-      ∃g. wfm_gnfa g ∧ ∀cs. has_Accepting_Execution d cs ⇔ gnfa_accepts g g.q_0 cs g.C
-Proof
-  rw[] >> qexists_tac ‘dfa_to_gnfa d’ >> rw[dfa_to_gnfa_wfm] >>
-  rw[has_Accepting_Execution_Delta_coincide_thm,accepts_def] >>
-  ‘∀s. s ∈ d.Q ⇒
-    (Delta d s cs ∈ d.C ⇔
-    gnfa_accepts (dfa_to_gnfa d) (s + 2) cs (dfa_to_gnfa d).C)’
-    suffices_by (fs[dfa_prod_gnfa_shuffle_start,wf_dfa_def] >>
-                 simp[dfa_to_gnfa_def]) >>
-  simp[EQ_IMP_THM, IMP_CONJ_THM, FORALL_AND_THM] >> conj_tac
-  >- (Induct_on ‘cs’
-      >- rw[dfa_to_gnfa_final_state_no_op]
-      >> rw[] >> ‘h::cs = [h]++cs’ by simp[] >> pop_assum SUBST_ALL_TAC >>
-      irule $ CONJUNCT2 $ SPEC_ALL gnfa_accepts_rules >> simp[] >>
-      qexists_tac ‘(d.tf s h)+2’ >> rw[]
-      >- (rw[dfa_to_gnfa_def] >>
-         ‘FINITE {cs | d.tf s cs = d.tf s h}’
-            by (irule SUBSET_FINITE_I >> qexists_tac ‘d.A’ >> conj_tac
-                >- fs[wf_dfa_def]
-                >> rw[SUBSET_DEF] >> metis_tac[Delta_c_in_A]) >>
-          simp[regexp_lang_charset_re])
-      >- (fs[wf_dfa_def] >> metis_tac[]) >>
-      first_x_assum irule >> rw[] >> metis_tac[wf_dfa_def, Delta_c_in_A]) >>
-  Induct_on ‘gnfa_accepts’ >> rw[] >> qpat_x_assum ‘c1 ∈ _’ mp_tac >>
-  rw[dfa_to_gnfa_def] >> fs[]
-  >- (drule gnfa_accepts_1_to_1 >> rw[]) >>
-  rfs[] >> rw[] >> ‘Delta d q c1 = q'’ suffices_by simp[] >>
-  ‘FINITE {cs | d.tf q cs = q'}’
-        by (irule SUBSET_FINITE_I >> qexists_tac ‘d.A’ >> fs[wf_dfa_def] >>
-            rw[SUBSET_DEF] >> metis_tac[Delta_c_in_A, wf_dfa_def]) >>
-  fs[regexp_lang_charset_re] >> rw[] >> fs[wf_dfa_def]
-QED
-
-Definition rip_def:
-  rip G q = if q IN G.Q ∧ q ≠ G.q_0 ∧ q <> G.C then
-            G with
-            <| Q := G.Q DELETE q ;
-               tf := \i j. if i = G.C then Empty
-                           else if j = G.q_0 then Empty
-                           else
-                             Alt (Concat (G.tf i q)
-                                  (Concat (Star (G.tf q q)) (G.tf q j)))
-                                 (G.tf i j)
-             |>
-            else G
+Definition REGULAR_def:
+  REGULAR = {(L,A) | ∃N. N.Sigma = A ∧ wf_nfa N ∧ L = nfa_lang N}
 End
 
-Theorem wfm_rip_wfm:
-  wfm_gnfa G ⇒ wfm_gnfa (rip G q)
+(* Possible alternative: pulls alphabet constraint out of the NFA
+Definition REGULAR_def:
+  REGULAR = {(L,A) | L ⊆ KSTAR (IMAGE Symbol_Word A) ∧ ∃N. wf_nfa N ∧ L = nfa_lang N}
+End
+*)
+
+Theorem IN_REGULAR:
+  (L,A) ∈ REGULAR ⇔ ∃N. N.Sigma = A ∧ wf_nfa N ∧ L = nfa_lang N
 Proof
-  rw[rip_def,wfm_gnfa_def]
+ rw [REGULAR_def,pairTheory.LAMBDA_PROD]
 QED
 
-Theorem gnfa_accepts_q_in_Q:
-  ∀G q_0 l q. gnfa_accepts G q_0 l q ⇒ q_0 ∈ G.Q ∧ q ∈ G.Q
+Theorem IN_REGULAR_AS_DFA:
+  (L,A) ∈ REGULAR ⇔ ∃M. M.Sigma = A ∧ is_dfa M ∧ L = nfa_lang M
 Proof
-  gen_tac >> Induct_on ‘gnfa_accepts’ >> simp[]
+  rw [IN_REGULAR,EQ_IMP_THM]
+  >- (qexists_tac ‘nfa_to_dfa N’ >> rw[is_dfa_nfa_to_dfa] >>
+      metis_tac [nfa_to_dfa_correct,EXTENSION])
+  >- (fs [is_dfa_def] >> metis_tac[])
 QED
 
-Theorem gnfa_accepts_star:
- ∀x G q_0 l q.
-   x IN KSTAR (regexp_lang (G.tf q_0 q_0)) ∧
-   gnfa_accepts G q_0 l q ⇒ gnfa_accepts G q_0 (x ⧺ l) q
+Theorem REGULAR_BOUNDED:
+  (L,A) ∈ REGULAR ⇒ L ⊆ KSTAR (IMAGE Symbol_Word A)
 Proof
- simp[KSTAR_DEF_ALT, PULL_EXISTS] >>
- CONV_TAC (RENAME_VARS_CONV ["s","G","q_0","l","q","n"]) >>
- Induct_on ‘n’ >> simp[DOTn_def,dot_def,PULL_EXISTS] >> rw[] >>
- metis_tac[APPEND_ASSOC,gnfa_accepts_step,gnfa_accepts_q_in_Q]
+  rw [IN_REGULAR,SUBSET_DEF] >>
+  fs [in_nfa_lang,wf_nfa_def]
 QED
 
-Theorem G_rip_Q:
-q ∈ G.Q ∧ q ≠ G.q_0 ∧ q ≠ G.C ⇒ (rip G q).Q = G.Q DELETE q
+Theorem REGULAR_SIGMA_FINITE:
+  (L,A) ∈ REGULAR ⇒ FINITE A
 Proof
-rw[rip_def]
+  rw [IN_REGULAR,SUBSET_DEF] >> metis_tac [wf_nfa_def]
 QED
 
-
-Theorem G_rip_back_sim:
-  ∀q_0 s. wfm_gnfa G ∧ q_0 ≠ q ∧ q ≠ G.q_0 ∧ q ≠ G.C ∧ q IN G.Q ∧
-         gnfa_accepts (rip G q) q_0 s G.C ⇒ gnfa_accepts G q_0 s G.C
+Theorem EMPTYSET_IN_REGULAR:
+  FINITE A ⇒ ({},A) ∈ REGULAR
 Proof
-  Induct_on ‘gnfa_accepts’ >>
-  reverse (rw[rip_def,gnfa_accepts_rules])
-  >- metis_tac[gnfa_accepts_rules]
-  >> Cases_on ‘q_0 = G.C’ >> fs[] >>
-  Cases_on ‘q_0' = G.q_0’ >> reverse (fs[])
-  >- (reverse (Cases_on ‘q_0' = q’)
-      >- metis_tac[gnfa_accepts_rules]
-      >> fs[])
-  >> fs[dot_def] >> REWRITE_TAC [GSYM APPEND_ASSOC] >>
-  irule gnfa_accepts_step >> simp[] >>
-  qexists_tac ‘q’ >>
-  ASM_REWRITE_TAC [GSYM APPEND_ASSOC] >> irule gnfa_accepts_star >> simp[] >>
-  metis_tac[gnfa_accepts_step,gnfa_accepts_q_in_Q]
+  rw [IN_REGULAR] >>
+  qexists_tac
+    ‘<| Q := {}; Sigma := A;
+        initial := {}; final := {};
+        delta := λq a. {} |>’ >>
+  rw [wf_nfa_def,EXTENSION,in_nfa_lang]
 QED
 
-Inductive gnfaA':
-  (∀q_0. q_0 ∈ G.Q ⇒ gnfaA' G q_0 [] [q_0] q_0) ∧
-  (∀q_0 q1 q2 s1 s2 states.
-     q_0 ∈ G.Q ∧ q1 ∈ G.Q ∧
-     s1 ∈ regexp_lang (G.tf q_0 q1) ∧
-     gnfaA' G q1 s2 states q2
-     ⇒
-     gnfaA' G q_0 (s1 ++ s2) (q_0::states) q2)
+Theorem EPSILON_LANG_IN_REGULAR:
+  FINITE A ⇒ ({ε},A) ∈ REGULAR
+Proof
+  rw [IN_REGULAR] >>
+  qexists_tac
+    ‘<| Q := {0}; Sigma := A;
+        initial := {0}; final := {0};
+        delta := λq a. {} |>’ >>
+  rw [wf_nfa_def,EXTENSION,in_nfa_lang,EQ_IMP_THM]
+  >- (fs [NOT_LESS] >> Cases_on ‘x’ >> fs[] >>
+      first_x_assum (mp_tac o Q.SPEC ‘0’) >> rw[])
+  >- (qexists_tac ‘[0]’ >> rw[])
+QED
+
+Theorem REGULAR_CLOSED_UNDER_COMPL:
+  (L,A) ∈ REGULAR ⇒ (KSTAR (IMAGE Symbol_Word A) DIFF L, A) ∈ REGULAR
+Proof
+  rw [IN_REGULAR_AS_DFA] >>
+  qexists_tac ‘nfa_compl M’ >> rw[]
+  >- simp[nfa_compl_def]
+  >- metis_tac [is_dfa_compl]
+  >- (drule dfa_compl_correct >> simp [EXTENSION])
+QED
+
+Theorem REGULAR_CLOSED_UNDER_UNION:
+  (L1,A) ∈ REGULAR ∧ (L2,A) ∈ REGULAR ⇒ (L1 ∪ L2, A) ∈ REGULAR
+Proof
+  rw [IN_REGULAR_AS_DFA] >> rename1 ‘M1.Sigma = M2.Sigma’ >>
+  qexists_tac ‘nfa_union M1 M2’ >> rw[]
+  >- simp[nfa_union_def]
+  >- metis_tac [is_dfa_union]
+  >- (drule_all dfa_union_correct >> simp [EXTENSION])
+QED
+
+Theorem REGULAR_CLOSED_UNDER_INTER:
+  (L1,A) ∈ REGULAR ∧ (L2,A) ∈ REGULAR ⇒ (L1 ∩ L2, A) ∈ REGULAR
+Proof
+  rw [IN_REGULAR_AS_DFA] >> rename1 ‘M1.Sigma = M2.Sigma’ >>
+  qexists_tac ‘nfa_inter M1 M2’ >> rw[]
+  >- simp[nfa_inter_def]
+  >- metis_tac [is_dfa_inter]
+  >- (drule_all dfa_inter_correct >> simp [EXTENSION])
+QED
+
+(*  TODO: need to under stand where A* and complement comes into play
+Theorem REGULAR_CLOSED_UNDER_DIFF:
+  (L1,A) ∈ REGULAR ∧ (L2,A) ∈ REGULAR ⇒ (L1 DIFF L2, A) ∈ REGULAR
+Proof
+  rw [DIFF_INTER_COMPL] >> irule REGULAR_CLOSED_UNDER_INTER >> rw[] >>
+  drule REGULAR_CLOSED_UNDER_COMPL >>
+  drule REGULAR_BOUNDED
+QED
+*)
+
+(*---------------------------------------------------------------------------*)
+(* Support for proving closure under concatenation. Adding a new start state *)
+(* with arrows to all targets of the original start state(s) gives a machine *)
+(* that accepts the original language less ε.                                *)
+(*---------------------------------------------------------------------------*)
+
+Definition new_state_def:
+  new_state N = MAX_SET N.Q + 1
 End
 
-Theorem gnfaA'_states_nonempty:
-  gnfaA' G q_0 str sts q ⇒ sts ≠ [] ∧ HD sts = q_0 ∧ LAST sts = q
+Theorem new_state_thm:
+  FINITE N.Q ⇒ new_state N ∉ N.Q
 Proof
-  Induct_on ‘gnfaA'’ >> simp[LAST_CONS_cond]
+  rw[new_state_def] >> strip_tac >>
+  ‘MAX_SET N.Q + 1 <= MAX_SET N.Q’ by metis_tac[X_LE_MAX_SET] >>
+  decide_tac
 QED
 
-Theorem gnfa_accepts_gnfaA':
-  gnfa_accepts G q_0 str q ⇒ ∃sts. gnfaA' G q_0 str sts q
+Definition new_start_state_def:
+ new_start_state N =
+   let start' = new_state N
+   in
+     N with <|Q := N.Q ∪ {start'};
+              initial := {start'};
+              delta := (λq a.
+                 if q = start' then
+                    BIGUNION {N.delta q a |q| q ∈ N.initial}
+                  else N.delta q a) |>
+End
+
+Theorem new_start_state_builtin_simps[simp]:
+ (new_start_state N).Sigma = N.Sigma ∧
+ (new_start_state N).Q = N.Q ∪ {new_state N} ∧
+ (new_start_state N).initial = {new_state N} ∧
+ (new_start_state N).final = N.final
 Proof
-  Induct_on ‘gnfa_accepts’ >> simp[] >> metis_tac[gnfaA'_rules]
+  rw[new_start_state_def]
 QED
 
-Theorem gnfaA'_gnfa_accepts:
-  gnfaA' G q_0 str sts q ⇒ gnfa_accepts G q_0 str q
+Theorem new_start_state_delta:
+  is_dfa N ∧ q ∈ N.Q ∧ a ∈ N.Sigma
+   ⇒
+ (new_start_state N).delta q a = N.delta q a
 Proof
-  Induct_on ‘gnfaA'’ >> simp[gnfa_accepts_rules] >>
-  metis_tac[gnfa_accepts_rules]
+  rw [new_start_state_def,is_dfa_def, wf_nfa_def] >>
+  metis_tac [new_state_thm]
 QED
 
-Theorem IN_ripQ:
-  x ≠ r ∧ x IN G.Q ⇒ x IN (rip G r).Q
+Theorem wf_new_start_state:
+  wf_nfa N ==> wf_nfa (new_start_state N)
 Proof
-  rw[rip_def]
+  fs [wf_nfa_def, new_start_state_def] >> rw[]
+  >- metis_tac [SUBSET_UNION_RIGHT]
+  >- (rw [] >> metis_tac [new_state_thm,SUBSET_UNION_RIGHT])
+  >- (irule SUBSET_UNION_RIGHT >> rw [SUBSET_DEF] >> metis_tac [SUBSET_DEF])
 QED
 
-Theorem repeated_head_elements:
-  ∀l e. ∃n sfx. l = REPLICATE n e ++ sfx ∧ (sfx ≠ [] ⇒ HD sfx ≠ e)
+Theorem is_dfa_new_start_state:
+  is_dfa N ⇒ is_dfa (new_start_state N)
 Proof
-  rpt gen_tac >> Induct_on ‘l’ >> simp[] >> fs[] >>
-  qx_gen_tac ‘h’ >> Cases_on ‘h = e’
-  >- (rw[] >> qexistsl_tac [‘SUC n’, ‘sfx’] >> simp[]) >>
-  qexistsl_tac [‘0’, ‘h::REPLICATE n e ++ sfx’] >> simp[]
+  rw [is_dfa_def,wf_new_start_state] >>
+  fs [new_start_state_def] >> rw[]
+  >- metis_tac [new_state_thm,wf_nfa_def]
+  >- (‘∃qa. N.delta q_0 a = {qa}’
+            by metis_tac [wf_nfa_def,EXTENSION,IN_INSERT,SUBSET_DEF] >>
+      qexists_tac ‘qa’ >> rw [EXTENSION,EQ_IMP_THM]
+      >- metis_tac[]
+      >- (qexists_tac ‘{qa}’ >> rw[]))
 QED
 
-Theorem gnfaA'_APPEND_states:
-  ∀G q_0 str sts1 sts2 q.
-    gnfaA' G q_0 str (sts1 ++ sts2) q ∧ sts1 ≠ [] ∧ sts2 ≠ [] ⇒
-    ∃str1 str2 q1. str = str1 ++ str2 ∧
-                   q1 ∈ G.Q ∧
-                   gnfaA' G q_0 str1 (sts1 ++ [HD sts2]) q1 ∧
-                   gnfaA' G q1 str2 sts2 q
+Theorem epsilon_not_in_new_start_state_lang:
+  wf_nfa N ⇒ ε ∉ nfa_lang (new_start_state N)
 Proof
-  Induct_on ‘sts1’ >> rw[] >> qpat_x_assum (‘gnfaA' _ _ _ _ _’) mp_tac >>
-  simp[Once gnfaA'_cases, SimpL “$==>”] >> rw[] >>
-  Cases_on ‘sts1 = []’
-  >- (rw[] >> fs[] >>
-      first_assum (goal_assum o resolve_then (Pos last) mp_tac) >>
-      simp[] >> drule gnfaA'_states_nonempty >> rw[] >>
-      drule_at (Pos $ el 3) (cj 2 gnfaA'_rules) >> rw[] >>
-      first_x_assum (resolve_then (Pos hd) mp_tac (cj 1 gnfaA'_rules)) >>
-      rw[]) >>
-  first_x_assum (drule_all_then strip_assume_tac) >>
-  first_assum (goal_assum o resolve_then (Pos last) mp_tac) >> rw[] >>
-  drule_at (Pos $ el 3) (cj 2 gnfaA'_rules) >> rw[]
+  rpt strip_tac >> drule_then assume_tac wf_new_start_state >>
+  drule epsilon_in_nfa_lang >> rw[] >>
+  rw [new_start_state_def] >> ntac 2 pop_forget_tac >>
+  fs [wf_nfa_def,EXTENSION] >> metis_tac [new_state_thm,SUBSET_DEF]
 QED
 
-Theorem gnfaA'_q_to_q_0:
-  wfm_gnfa G ⇒ gnfaA' G q str sts G.q_0 ⇒ q = G.q_0 ∧ sts = [G.q_0]
+Theorem new_start_state_closed:
+  wf_nfa N ∧
+  is_exec (new_start_state N) qs w ⇒
+  ∀n. 0 < n ∧ n < LENGTH qs ⇒ EL n qs ∈ N.Q
 Proof
-  Induct_on ‘gnfaA'’ >> rw[] >> Cases_on ‘wfm_gnfa G’ >> fs[] >> rw[] >>
-  fs[wfm_gnfa_def]
+  strip_tac >> Induct >> rw[] >>
+  ‘n < LENGTH qs’ by decide_tac >>
+  fs [is_exec_def,EVERY_EL,wf_nfa_def,SUBSET_DEF] >>
+  ‘n < LENGTH w’ by decide_tac >>
+  first_x_assum drule >> rw [new_start_state_def,ADD1] >>
+  ‘EL n w ∈ N.Sigma’ by metis_tac[]
+  >- metis_tac[]
+  >- (Cases_on ‘n=0’ >> fs[] >> rw[] >> metis_tac[])
+  >- metis_tac[]
+  >- (Cases_on ‘n=0’ >> fs[] >> rw[] >> metis_tac[])
 QED
 
-Theorem gnfaA'_in_G:
-∀s l q_0 q. gnfaA' G q_0 s l q ⇒ ∀st. MEM st l ⇒ st IN G.Q
+Theorem new_start_state_subset:
+  is_dfa N ⇒ nfa_lang (new_start_state N) ⊆ nfa_lang N
 Proof
-Induct_on ‘gnfaA'’ >> simp[DISJ_IMP_THM]
+  rw[SUBSET_DEF] >> rename1 ‘w ∈ nfa_lang N’ >>
+  ‘w ≠ ε’ by metis_tac [is_dfa_def,epsilon_not_in_new_start_state_lang] >>
+  fs [in_nfa_lang] >> rw[] >>
+  ‘qs ≠ []’ by (Cases_on ‘qs’ >> fs[]) >>
+  ‘∃q_0. N.initial = {q_0}’ by metis_tac [is_dfa_def] >>
+  qexists_tac ‘q_0 :: TL qs’ >>
+  fs [NOT_NIL_EQ_LENGTH_NOT_0, LENGTH_TL] >> rw[]
+  >- (‘TL qs ≠ []’ by (Cases_on ‘qs’ >> fs[] >> Cases_on ‘t’ >> gvs[]) >>
+      rw [LAST_DEF])
+  >- (rw [GSYM ADD1] >> Cases_on ‘n’ >> fs[]
+      >- (first_x_assum drule >> rw[] >>
+          rfs [new_start_state_def,PULL_EXISTS] >>
+          Cases_on ‘qs’ >> fs [] >> Cases_on ‘t’ >> fs[])
+      >- (rename1 ‘SUC m < LENGTH w’ >>
+          ‘qs ≠ []’ by (Cases_on ‘qs’ >> fs[]) >> rw[GSYM ADD1] >>
+          ‘EL (SUC m) w ∈ N.Sigma’ by fs [EVERY_EL] >>
+          ‘EL (SUC m) qs ∈ N.Q’ by
+             (fs [is_dfa_def] >> drule new_start_state_closed >> disch_then irule >>
+              rw[is_exec_def] >> metis_tac[]) >>
+          metis_tac [new_start_state_delta, ADD1]))
 QED
 
-Theorem gnfaA'_APPEND_states2:
-  ∀G q_0 str sts1 sts2 q.
-         gnfaA' G q_0 str (sts1 ⧺ sts2) q ∧ sts1 ≠ [] ∧ sts2 ≠ [] ⇒
-         ∃str1 str2 q1.
-             str = str1 ⧺ str2 ∧ q1 ∈ G.Q ∧
-             gnfaA' G q_0 str1 sts1 q1 ∧ gnfaA' G q1 str2 (LAST sts1 :: sts2) q
+Theorem new_start_state_diff_epsilon:
+  is_dfa N ⇒ nfa_lang N DIFF {ε} ⊆ nfa_lang (new_start_state N)
 Proof
- rw[] >> Cases_on ‘sts1’ >> fs[] >> rename [‘q1 :: (sts1 ++ sts2)’] >>
- ‘q_0 = q1’ by (drule gnfaA'_states_nonempty >> simp[]) >> rw[] >>
- Cases_on ‘sts1 = []’ >> fs[] (* 2 *)
- >- (first_assum (goal_assum o resolve_then (Pos last) mp_tac) >>
-     csimp[gnfaA'_rules] >>
-     metis_tac[gnfaA'_in_G,MEM]) >>
- ‘q_0::(sts1 ⧺ sts2) = FRONT (q_0::sts1) ++ LAST (q_0::sts1) :: sts2’
-   by (‘LAST (q_0::sts1)::sts2 = [LAST (q_0::sts1)] ++ sts2’ by simp[] >>
-      simp[APPEND_FRONT_LAST]) >>
- qpat_x_assum ‘gnfaA' _ _ _ _ _’ mp_tac >> simp[] >>
- strip_tac >> drule gnfaA'_APPEND_states >> simp[APPEND_FRONT_LAST]
+  rw [EXTENSION,in_nfa_lang,SUBSET_DEF] >> rename1 ‘LENGTH w + 1’ >>
+  qexists_tac ‘new_state N :: TL qs’ >>
+  fs [NOT_NIL_EQ_LENGTH_NOT_0, LENGTH_TL] >> rw[]
+  >- (‘TL qs ≠ []’
+       by (Cases_on ‘qs’ >> fs[] >> Cases_on ‘t’ >> gvs[]) >>
+      rw [LAST_DEF])
+  >- (‘qs ≠ []’ by (Cases_on ‘qs’ >> fs[]) >>
+      Cases_on ‘n’ >> fs[]
+      >- (first_x_assum drule >> rw[] >>
+          rw [new_start_state_def,PULL_EXISTS] >> metis_tac[])
+      >- (fs [is_dfa_def] >>
+          ‘EL (SUC n') qs ∈ N.Q’ by
+            (‘HD qs ∈ N.Q’
+               by metis_tac [wf_nfa_def,SUBSET_DEF] >>
+             drule_all nfa_execution_states_closed >>
+             rw [EVERY_EL]) >>
+          ‘EL (SUC n') w ∈ N.Sigma’ by fs [EVERY_EL] >> rw[GSYM ADD1] >>
+          metis_tac[new_start_state_delta,ADD1,is_dfa_def]))
 QED
 
-Theorem gnfaA'_REPLICATE:
-  ∀G q s n.
-    gnfaA' G q s (REPLICATE n q) q ⇒
-    s ∈ KSTAR (regexp_lang (G.tf q q))
+Theorem nfa_lang_new_start_state:
+  is_dfa N ⇒ nfa_lang (new_start_state N) = nfa_lang N DIFF {ε}
 Proof
-  Induct_on ‘n’ >> rw[]
-  >- fs[Once gnfaA'_cases]  >>
-  pop_assum mp_tac >> simp[Once gnfaA'_cases] >>
-  rw[] >- fs[EMPTY_IN_KSTAR] >>
-  Cases_on ‘n = 0’
-  >- (qpat_x_assum ‘gnfaA' _ _ _ _ _ ’ mp_tac >> simp[Once gnfaA'_cases]) >>
-  rename [‘s1 ∈ regexp_lang (G.tf q q1)’] >>
-  ‘q1 = q’
-    by (drule gnfaA'_states_nonempty >>
-        simp[HD_REPLICATE]) >>
-  gvs[] >> first_x_assum $ drule_all_then assume_tac >>
-  gvs[KSTAR_FLAT] >> rename1 ‘s1 ++ FLAT ls’ >> qexists_tac ‘s1::ls’ >>
-  rw[] >> rw[]
+  rw[EXTENSION,EQ_IMP_THM]
+   >- metis_tac [new_start_state_subset,SUBSET_DEF]
+   >- metis_tac [epsilon_not_in_new_start_state_lang,is_dfa_def]
+   >- metis_tac [new_start_state_diff_epsilon |> SRULE [SUBSET_DEF]]
 QED
 
-Theorem gnfaA'_rip_filter:
-  ∀sts q_0 str q r.
-    wfm_gnfa G ∧ gnfaA' G q_0 str sts q ∧ q_0 ≠ r ∧ q ≠ r ∧ r ∈ G.Q ∧ r ≠ G.q_0 ∧
-    r ≠ G.C ⇒
-    gnfaA' (rip G r) q_0 str (FILTER (λq. q ≠ r) sts) q
+Theorem is_dfa_final_union:
+  is_dfa N ∧ qs ⊆ N.Q ⇒ is_dfa (N with final := N.final ∪ qs)
 Proof
-  gen_tac >>
-  completeInduct_on ‘LENGTH sts’ >> fs[PULL_FORALL] >> rpt gen_tac >>
-  strip_tac >>
-  simp[Once gnfaA'_cases, SimpL “$==>”] >> rw[]
-  >- simp[IN_ripQ, gnfaA'_rules] >>
-  simp[] >>
-  qspecl_then [‘states’, ‘r’] (qx_choosel_then [‘n’, ‘sfx’] strip_assume_tac)
-              repeated_head_elements >>
-  rw[FILTER_APPEND, FILTER_REPLICATE] >>
-  drule gnfaA'_APPEND_states >> simp[] >> Cases_on ‘sfx = []’ >> rw[]
-  >- (fs[] >> drule gnfaA'_states_nonempty >> rw[] >> fs[LAST_REPLICATE]) >>
-  Cases_on ‘n = 0’ >> fs[] >> rw[]
-  >- (irule (cj 2 gnfaA'_rules) >> rw[IN_ripQ] >> qexists_tac ‘q1’ >> rw[]
-      >- (rw[rip_def] >> fs[wfm_gnfa_def] >> rfs[])
-      >- (drule gnfaA'_states_nonempty >> rw[] >> rw[IN_ripQ]) >>
-      first_x_assum irule >> rw[] >> drule gnfaA'_states_nonempty >> rw[]) >>
-  ‘q1 = r’ by (rev_drule gnfaA'_states_nonempty >> rw[] >>
-               simp[HD_APPEND, HD_REPLICATE]) >>
-  rw[] >> rename [‘gnfaA' G q1 str1 (REPLICATE n q1 ⧺ [HD sfx]) q2’] >>
-  ‘q2 = HD sfx’ by (drule gnfaA'_states_nonempty >> rw[]) >> rw[] >>
-  irule (cj 2 gnfaA'_rules) >> rw[IN_ripQ] >> qexists_tac ‘HD sfx’ >>
-  rw[] (* 2 *)
-  >- (simp[rip_def] >> rw[]
-      >- rfs[wfm_gnfa_def]
-      >- (fs[] >> rw[] >> drule_all gnfaA'_q_to_q_0 >> rw[]) >>
-      DISJ1_TAC >> simp[Once dot_def] >> goal_assum (drule_at (Pos $ el 2))>>
-      simp[] >>
-      drule gnfaA'_APPEND_states2 >> simp[] >> strip_tac >>
-      drule gnfaA'_states_nonempty >> simp[] >> rw[] >> rfs[LAST_REPLICATE] >>
-      simp[dot_def] >> simp[] >>
-      rename [‘s1 ++ s2 = _ ++ _’] >> qexistsl_tac [‘s1’,‘s2’] >> simp[] >>
-      reverse conj_tac (* 2 *)
-      >- (pop_assum mp_tac >> simp[Ntimes gnfaA'_cases 3]) >>
-      metis_tac[gnfaA'_REPLICATE]) >>
-  rw[rip_def]
+ rw [is_dfa_def,wf_nfa_def]
 QED
 
-Theorem G_rip_forw_sim:
-  ∀q_0 s q1 q. wfm_gnfa G ∧ q_0 ∈ G.Q ∧ q ≠ q_0 ∧ q1 ∈ G.Q ∧ q ≠ q1 ∧ q ∈ G.Q ∧
-         gnfa_accepts G q_0 s q1 ⇒ gnfa_accepts (rip G q) q_0 s q1
+Theorem nfa_lang_final_union:
+  nfa_lang (N with final := N.final ∪ qs) =
+  nfa_lang N ∪ nfa_lang (N with final := qs)
+Proof
+ rw [EXTENSION,in_nfa_lang] >> metis_tac[]
+QED
+
+(*---------------------------------------------------------------------------*)
+(* Given a machine that accepts ε, obtain a machine that recognizes the same *)
+(* language, except ε is rejected. And vice-versa.                           *)
+(*---------------------------------------------------------------------------*)
+
+Theorem REGULAR_CLOSED_UNDER_EPSILON_ADDITION_OR_DELETION:
+ (L ∪ {ε},A) ∈ REGULAR ⇔ (L DIFF {ε},A) ∈ REGULAR
+Proof
+  rw [IN_REGULAR_AS_DFA,EQ_IMP_THM] THENL
+  [qexists_tac ‘new_start_state M’,
+   qexists_tac ‘let M' = new_start_state M
+                in M' with <| final := M'.final ∪ {new_state M} |>’]
+  >> rw[]
+  >- metis_tac [is_dfa_new_start_state]
+  >- (drule_then subst_all_tac UNION_EQ_DIFF >> pop_forget_tac >>
+      metis_tac [nfa_lang_new_start_state])
+  >- (drule is_dfa_new_start_state >> rpt pop_forget_tac >> disch_tac >>
+      ‘M.final = (new_start_state M).final’ by rw[] >> pop_subst_tac >>
+      irule is_dfa_final_union >> rw[])
+  >- (drule_then subst_all_tac DIFF_EQ_UNION >> pop_forget_tac >>
+     ‘M.final = (new_start_state M).final’ by rw[] >> pop_subst_tac >>
+      rw [EXTENSION,nfa_lang_final_union,nfa_lang_new_start_state] >>
+      rw [EQ_IMP_THM]
+      >- rw[in_nfa_lang,new_start_state_def,LENGTH_EQ_NUM_compute,PULL_EXISTS]
+      >- rw[in_nfa_lang,new_start_state_def,LENGTH_EQ_NUM_compute,PULL_EXISTS]
+      >- rw[]
+      >- (disj2_tac >> rename1 ‘w = ε’ >> CCONTR_TAC >>
+          fs [in_nfa_lang,NOT_NIL_EQ_LENGTH_NOT_0] >>
+          ‘EL (LENGTH w) qs ∈ M.Q’
+             by (fs [is_dfa_def] >> drule new_start_state_closed >>
+                 disch_then irule >> rw[is_exec_def] >> metis_tac[]) >>
+          gvs [EL_LENGTH_LAST] >>
+          metis_tac [new_state_thm, is_dfa_def, wf_nfa_def]))
+QED
+
+(* Better to have this as an instance of closure under difference? *)
+Theorem REGULAR_CLOSED_UNDER_EPSILON_DELETION:
+ (L,A) ∈ REGULAR ⇒ (L DIFF {ε},A) ∈ REGULAR
+Proof
+  disch_tac >> Cases_on ‘ε ∈ L’
+  >- (‘L = L ∪ {ε}’ by (rw [EXTENSION,EQ_IMP_THM] >> metis_tac[]) >>
+      metis_tac [REGULAR_CLOSED_UNDER_EPSILON_ADDITION_OR_DELETION])
+  >- (‘L DIFF {ε} = L’ by (rw [EXTENSION,EQ_IMP_THM] >> metis_tac[]) >>
+      metis_tac [])
+QED
+
+Theorem isolate_corner_cases:
+ ∀L. ∃L0. L0 ⊆ {ε} ∧ L = L0 ∪ (L DIFF {ε})
+Proof
+  rw [SUBSET_DEF,EXTENSION] >>
+  qexists_tac ‘if ε ∈ L then {ε} else {}’ >>
+  rw[EQ_IMP_THM] >> metis_tac[]
+QED
+
+Theorem TRIVIAL_DOT_TRIVIAL_IN_REGULAR:
+ L1 ⊆ {ε} ∧ L2 ⊆ {ε} ∧ FINITE A ⇒ (L1 dot L2,A) ∈ REGULAR
+Proof
+  rw [SUBSET_SING] >> simp [DOT_EMPTYSET, DOT_EMPTYSTRING] >>
+  metis_tac [EMPTYSET_IN_REGULAR,EPSILON_LANG_IN_REGULAR]
+QED
+
+Triviality TRIVIAL_DOT_EPSILON_FREE_IN_REGULAR:
+  (L,A) ∈ REGULAR ∧
+  s1 ⊆ {ε} ∧ s2 ⊆ {ε}
+  ⇒
+  (L = s2 ∪ (L DIFF {ε}) ⇒ (s1 dot (L DIFF {ε}),A) ∈ REGULAR) ∧
+  (L = s1 ∪ (L DIFF {ε}) ⇒ ((L DIFF {ε}) dot s2,A) ∈ REGULAR)
+Proof
+  rw [SUBSET_SING] >>
+  fs [DOT_EMPTYSET, DOT_EMPTYSTRING] >>
+  metis_tac [EMPTYSET_IN_REGULAR, REGULAR_CLOSED_UNDER_EPSILON_DELETION,
+             UNION_COMM,REGULAR_SIGMA_FINITE]
+QED
+
+(*---------------------------------------------------------------------------*)
+(* Mechanism for renaming states apart when combining machines, used in, eg, *)
+(* the nfa_dot machine. Without renaming, the composed transition function   *)
+(* could be confused when given a state that happened to occur in both       *)
+(* components. NB: we could also prevent confusion via the encode/decode     *)
+(* functions used elsewhere in this theory.                                  *)
+(*---------------------------------------------------------------------------*)
+
+Definition newFn_def:
+  newFn base n = base + n
+End
+
+Theorem INJ_newFn:
+  INJ (newFn base) 𝕌(:num) 𝕌(:num)
+Proof
+  rw [newFn_def,INJ_DEF]
+QED
+
+Theorem newFn_eq[simp]:
+  newFn base q1 = newFn base q2 ⇔ q1 = q2
+Proof
+  assume_tac INJ_newFn >> fs [INJ_DEF] >> metis_tac[]
+QED
+
+Theorem BIJ_newFn:
+  BIJ (newFn base) N.Q (IMAGE (newFn base) N.Q)
+Proof
+ irule INJ_BIJ_SUBSET >> qexists_tac ‘𝕌(:num)’ >>
+ rw [SUBSET_DEF] >> metis_tac [INJ_newFn]
+QED
+
+Theorem oldFn_newFn:
+  q ∈ N.Q ⇒ LINV (newFn base) N.Q (newFn base q) = q
+Proof
+  rw [] >> assume_tac BIJ_newFn >> drule BIJ_LINV_INV >>
+  rw[PULL_EXISTS] >> fs [newFn_def]
+QED
+
+Definition rename_states_def:
+  rename_states N base =
+    let newq = newFn base in
+    let oldq = LINV newq N.Q in
+    N with <| Q       := IMAGE newq N.Q;
+              initial := IMAGE newq N.initial;
+              final   := IMAGE newq N.final;
+              delta   := λnq a. IMAGE newq (N.delta (oldq nq) a)
+            |>
+End
+
+Theorem rename_states_builtin_simps[simp]:
+ (rename_states N base).Sigma = N.Sigma
+Proof
+ simp [rename_states_def]
+QED
+
+Theorem wf_nfa_rename_states:
+  wf_nfa N ⇒ wf_nfa (rename_states N base)
+Proof
+  rw[wf_nfa_def,rename_states_def,SUBSET_DEF] >> metis_tac[oldFn_newFn]
+QED
+
+Theorem rename_states_delta_commutes:
+ wf_nfa N ∧ q ∈ N.Q ∧ a ∈ N.Sigma
+  ⇒
+ N.delta q a = IMAGE (LINV (newFn base) N.Q)
+                     ((rename_states N base).delta (newFn base q) a)
+Proof
+  rw[EXTENSION,EQ_IMP_THM,rename_states_def] >>
+  qabbrev_tac ‘oldFn = LINV (newFn base) N.Q’ >>
+  metis_tac [wf_nfa_def,SUBSET_DEF,oldFn_newFn]
+QED
+
+Theorem is_dfa_rename_states:
+  wf_nfa N ⇒ (is_dfa (rename_states N base) ⇔ is_dfa N)
+Proof
+  rw [is_dfa_def,EQ_IMP_THM,wf_nfa_rename_states]
+  >- (pop_forget_tac >> pop_keep_tac >> simp [rename_states_def] >>
+      ‘BIJ (newFn base) N.initial (IMAGE (newFn base) N.initial)’ by
+         (irule INJ_BIJ_SUBSET >> qexists_tac ‘𝕌(:num)’ >>
+          rw [SUBSET_DEF] >> metis_tac [INJ_newFn]) >>
+      ‘FINITE N.initial’ by metis_tac [wf_nfa_def,SUBSET_FINITE] >>
+      drule_all FINITE_BIJ_CARD >> rw[] >> fs[] >>
+      ‘SING N.initial’ by metis_tac [SING_IFF_CARD1] >> fs [SING_DEF])
+  >- (‘newFn base q ∈ (rename_states N base).Q’ by rw [rename_states_def] >>
+      first_x_assum drule_all >> rw[] >>
+      qabbrev_tac ‘oldFn = LINV (newFn base) N.Q’ >>
+      qexists_tac ‘oldFn q''’ >>
+      drule_all_then (qspec_then ‘base’ assume_tac)
+        rename_states_delta_commutes >>  rw[])
+  >- rw [rename_states_def]
+  >- (rule_assum_tac (SRULE[rename_states_def]) >> fs[] >> rw[] >>
+      first_x_assum drule_all >> rw[] >>
+      qexists_tac ‘newFn base q'’ >> rw [rename_states_def,oldFn_newFn])
+QED
+
+Theorem nfa_lang_rename_states:
+  wf_nfa N ⇒ nfa_lang (rename_states N base) = nfa_lang N
+Proof
+  rw [EXTENSION,EQ_IMP_THM]
+  >- (drule_then (qspec_then ‘base’ assume_tac) wf_nfa_rename_states >>
+      drule_all in_nfa_lang_is_accepting_exec >>
+      rw[NULL_EQ,is_accepting_exec_def,in_nfa_lang]
+      >- (drule is_exec_Sigma >> rw[])
+      >- (qpat_forget_tac ‘_ ∈ nfa_lang _’ >>
+          qpat_keep_tac ‘HD qs ∈ _’ >> qpat_keep_tac ‘LAST qs ∈ _’ >>
+          rw [rename_states_def] >> rename [‘qi ∈ N.initial’, ‘qf ∈ N.final’] >>
+          qabbrev_tac ‘oldFn = LINV (newFn base) N.Q’ >>
+          qexists_tac ‘MAP oldFn qs’ >> rw[]
+          >- (drule is_exec_length >> rw[])
+          >- metis_tac [oldFn_newFn,wf_nfa_def,SUBSET_DEF]
+          >- metis_tac [oldFn_newFn,wf_nfa_def,SUBSET_DEF]
+          >- (drule is_exec_length >> rename1 ‘n < LENGTH w’ >> disch_tac >>
+              ‘n < LENGTH qs’ by decide_tac >> rw[EL_MAP] >>
+              drule_all is_exec_states >>
+              rw [rename_states_def,EVERY_EL,PULL_EXISTS] >>
+              ‘n < LENGTH w + 1’ by metis_tac [] >> first_x_assum drule >> rw[] >>
+              rw[Abbr ‘oldFn’,oldFn_newFn] >>
+              qabbrev_tac ‘oldFn = LINV (newFn base) N.Q’ >>
+              drule_all is_exec_delta >> rw [rename_states_def] >> rw[] >>
+              pop_keep_tac >> rw [Abbr‘oldFn’, oldFn_newFn] >>
+              ‘EL n w ∈ N.Sigma’ by (drule is_exec_Sigma >> rw [EVERY_EL]) >>
+              metis_tac [wf_nfa_def, SUBSET_DEF,oldFn_newFn])))
+  >- (drule_all in_nfa_lang_is_accepting_exec >>
+      rw[NULL_EQ,in_nfa_lang,is_accepting_exec_def]
+      >- metis_tac[is_exec_Sigma]
+      >- (rename1 ‘is_exec N qs w’ >>
+          qexists_tac ‘MAP (newFn base) qs’ >> rw[]
+          >- metis_tac [is_exec_length]
+          >- rw [rename_states_def]
+          >- rw [rename_states_def]
+          >- (rw [rename_states_def] >> drule is_exec_length >> disch_tac >>
+              ‘n < LENGTH qs’ by decide_tac >> rw[EL_MAP] >>
+              drule_all is_exec_states >> rw [EVERY_EL] >>
+              ‘n < LENGTH w + 1’ by metis_tac [] >> first_x_assum drule >> rw[] >>
+              ‘EL n w ∈ N.Sigma’ by (drule is_exec_Sigma >> rw [EVERY_EL]) >>
+              rw [oldFn_newFn] >> metis_tac [is_exec_delta])))
+QED
+
+Theorem RENAME_STATES_APART:
+  FINITE Q ∧ wf_nfa N
+  ⇒
+  ∃N'. N'.Sigma = N.Sigma ∧
+       Q ∩ N'.Q = ∅ ∧
+       wf_nfa N' ∧
+       (is_dfa N' ⇔ is_dfa N) ∧
+       nfa_lang N' = nfa_lang N
+Proof
+ strip_tac >>
+ qexists_tac ‘rename_states N (MAX_SET (Q ∪ N.Q) + 1)’ >> rw[]
+ >- (rw [rename_states_def,EXTENSION, Once (GSYM IMP_DISJ_THM),newFn_def] >>
+     CCONTR_TAC >> pop_forget_tac >>
+     ‘FINITE N.Q’ by metis_tac [wf_nfa_def] >> qpat_keep_tac ‘_ ∈ _’ >>
+     rw [MAX_SET_UNION,MAX_DEF] >> irule MAX_SET_BOUNDED >> rw[])
+ >- metis_tac [wf_nfa_rename_states]
+ >- metis_tac [is_dfa_rename_states]
+ >- metis_tac [nfa_lang_rename_states]
+QED
+
+(*---------------------------------------------------------------------------*)
+(* Correctness of nfa_dot construction for epsilon-free machines is based on *)
+(* two lemmas: one for pasting together component executions, and one for    *)
+(* breaking an nfa-dot execution into two component executions.              *)
+(*---------------------------------------------------------------------------*)
+
+Theorem is_accepting_exec_paste:
+  is_dfa M1 ∧ is_dfa M2 ∧
+  M1.Sigma = M2.Sigma ∧ M1.Q ∩ M2.Q = ∅ ∧
+  w1 ≠ ε ∧ w2 ≠ ε ∧
+  is_accepting_exec M1 qs1 w1 ∧
+  is_accepting_exec M2 qs2 w2
+  ⇒
+  is_accepting_exec (nfa_dot M1 M2) (qs1 ++ TL qs2) (w1 ++ w2)
+Proof
+  rw [is_accepting_exec_def] >>
+  ‘EVERY (λq. q ∈ M1.Q) qs1 ∧ EVERY (λq. q ∈ M2.Q) qs2’ by
+      metis_tac [is_dfa_def,is_exec_states] >>
+  ‘qs1 ≠ [] ∧ qs2 ≠ []’ by metis_tac [is_exec_nonempty] >>
+  ‘TL qs2 ≠ []’ by
+     metis_tac [is_accepting_exec_length,is_accepting_exec_def,is_dfa_def] >>
+  rw [is_exec_def]
+  >- metis_tac [is_exec_Sigma]
+  >- metis_tac [is_exec_Sigma]
+  >- (imp_res_tac is_exec_length >> rw[LENGTH_TL])
+  >- metis_tac [is_dfa_def,wf_nfa_def,SUBSET_DEF]
+  >- (‘n < LENGTH w1 ∨ n = LENGTH w1 ∨ LENGTH w1 < n’ by decide_tac
+      >- (rev_drule is_exec_Sigma >> rw[EVERY_EL] >>
+          rev_drule is_exec_length >> strip_tac >>
+          ‘n < LENGTH qs1’ by decide_tac >> ‘n+1 < LENGTH qs1’ by decide_tac >>
+          rw[EL_APPEND1] >> rw [nfa_dot_def]
+          >- metis_tac [is_exec_delta,is_dfa_def]
+          >- metis_tac [is_exec_delta,is_dfa_def]
+          >- (qpat_keep_tac ‘EVERY _ qs1’ >> rw[EVERY_EL] >> metis_tac[]))
+      >- (rw[] >> rfs[] >> rev_drule is_exec_length >>
+          disch_then(assume_tac o SYM) >> ONCE_ASM_REWRITE_TAC[] >>
+          rw[SRULE [NULL_EQ] EL_LENGTH_APPEND] >>
+          ‘LENGTH w1 < LENGTH qs1’ by decide_tac >> rw [EL_APPEND1] >>
+          ‘LENGTH w1 = PRE (LENGTH qs1)’ by decide_tac >> pop_subst_tac >>
+          rw [EL_PRE_LENGTH] >> rw [nfa_dot_def,PULL_EXISTS]
+          >- (disj2_tac >> rfs [is_dfa_def,NOT_NIL_EQ_LENGTH_NOT_0] >> rw[] >>
+              ‘0 < LENGTH w1’ by decide_tac >> PURE_REWRITE_TAC[GSYM EL] >>
+              drule is_exec_delta >> disch_then drule >> simp[] >> rfs[])
+          >- metis_tac[is_dfa_def,wf_nfa_def,SUBSET_DEF])
+      >- (‘∃k. 0 < k ∧ k < LENGTH w2 ∧ n = LENGTH w1 + k’
+            by (qexists_tac ‘n - LENGTH w1’ >> fs[]) >> rw[EL_APPEND2_ALT] >>
+          rev_drule is_exec_length >> disch_tac >>
+          ‘k + (LENGTH w1 + 1) = LENGTH qs1 + k’ by decide_tac >> pop_subst_tac >>
+          drule is_exec_length >> disch_tac >>
+          ‘k < LENGTH (TL qs2)’
+            by (‘k + 1 < LENGTH qs2’ by decide_tac >>
+                drule LENGTH_TL_ALT >> rw[]) >>
+          ‘k < LENGTH qs2’ by decide_tac >>
+          rw [EL_APPEND2_ALT] >> rw [EL_APPEND_EQN] >> rw [nfa_dot_def]
+          >- (fs [EVERY_EL,EXTENSION] >> metis_tac[])
+          >- (fs [EVERY_EL,EXTENSION] >> metis_tac[])
+          >- metis_tac [is_exec_delta])
+     )
+  >- rw[LAST_APPEND_NOT_NIL]
+QED
+
+Theorem nfa_dot_paste:
+  is_dfa M1 ∧ is_dfa M2 ∧
+  M1.Sigma = M2.Sigma ∧ M1.Q ∩ M2.Q = ∅ ∧
+  ε ∉ nfa_lang M1 ∧ ε ∉ nfa_lang M2
+  ⇒
+  nfa_lang M1 dot nfa_lang M2 ⊆ nfa_lang (nfa_dot M1 M2)
+Proof
+  rw [SUBSET_DEF, IN_dot] >>
+  ‘u ≠ ε ∧ v ≠ ε’ by metis_tac[] >>
+  ntac 2 (qpat_forget_tac ‘ε ∉ _’) >>
+  ‘wf_nfa M1 ∧ wf_nfa M2 ∧ wf_nfa (nfa_dot M1 M2)’ by
+    metis_tac [is_dfa_def,wf_nfa_dot] >>
+  fs [in_nfa_lang_iff_accepting_exec] >>
+  metis_tac[is_accepting_exec_paste]
+QED
+
+Triviality nfa_dot_delta_states:
+  wf_nfa M1 ∧ wf_nfa M2 ∧
+  M1.Sigma = M2.Sigma ∧ a ∈ M1.Sigma ∧ q ∈ M1.Q ∪ M2.Q
+  ⇒
+  (nfa_dot M1 M2).delta q a ⊆ M1.Q ∪ M2.Q
+Proof
+  rw [wf_nfa_def, nfa_dot_def,SUBSET_DEF] >> metis_tac[]
+QED
+
+Triviality nfa_dot_delta_second_states:
+  wf_nfa M1 ∧ wf_nfa M2 ∧ M1.Q ∩ M2.Q = ∅ ∧
+  M1.Sigma = M2.Sigma ∧ a ∈ M1.Sigma ∧ q ∈ M2.Q ∧
+  q' ∈ (nfa_dot M1 M2).delta q a
+  ⇒
+  q' ∈ M2.Q
+Proof
+  rw [wf_nfa_def, nfa_dot_def,EXTENSION,SUBSET_DEF] >> metis_tac[]
+QED
+
+Triviality nfa_dot_states:
+   wf_nfa M1 ∧ wf_nfa M2 ∧ M1.Sigma = M2.Sigma ∧
+   is_exec (nfa_dot M1 M2) qs w
+   ⇒
+   EVERY (λq. q ∈ M1.Q ∪ M2.Q) qs
+Proof
+  simp[EVERY_EL] >> disch_tac >> Induct >> rw[] >>
+  imp_res_tac POS_LENGTH_NOT_NIL >> fs [is_exec_def,EVERY_EL] >>
+  ‘n < LENGTH w’ by decide_tac >>
+  first_x_assum drule >> first_x_assum drule >> rw[] >>
+  metis_tac[nfa_dot_delta_states, IN_UNION, ADD1, SUBSET_DEF]
+QED
+
+(*---------------------------------------------------------------------------*)
+(* Lemma about nfa_dot executions being split into component executions.     *)
+(*                                                                           *)
+(*   Let qs be an nfa_dot execution accepting word w. The first state        *)
+(*   of qs is in M1.Q and the last state is in M2.Q. Therefore there is      *)
+(*   a first state of qs that is in M2.Q; say it occurs at index j. Since    *)
+(*   M1 and M2 do not accept epsilon, 1 < j < length(qs). Thus               *)
+(*   qs[0 .. j-1] is a sequence of M1.Q states, and                          *)
+(*   qs[j .. length(qs)-1] is a sequence of M2.Q states. Moreover            *)
+(*                                                                           *)
+(*    * qs[j-1] ∈ M1.final                                                   *)
+(*    * qs[j] = M2.delta M2.initial (w[j-1])                                 *)
+(*    * (nfa_dot M1 M2).delta behaves the same as M1.delta below j-1,        *)
+(*      and the same as M2.delta at j and above.                             *)
+(*---------------------------------------------------------------------------*)
+
+Theorem nfa_dot_snip_lemma:
+   is_dfa M1 ∧
+   is_dfa M2 ∧
+   M1.Sigma = M2.Sigma ∧
+   M1.Q ∩ M2.Q = ∅ ∧
+   ε ∉ nfa_lang M1 ∧
+   ε ∉ nfa_lang M2 ∧
+   is_exec (nfa_dot M1 M2) qs w ∧
+   HD qs ∈ M1.initial ∧
+   LAST qs ∈ M2.final
+  ⇒
+  ∃q0 j.
+    M2.initial = {q0} ∧
+    1 < j ∧ j < LENGTH qs ∧
+    (∀i. i < j-1 ⇒ EL (i+1) qs ∈ M1.delta (EL i qs) (EL i w)) ∧
+    EL (j-1) qs ∈ M1.final ∧
+    EL j qs ∈ M2.delta q0 (EL (j-1) w) ∧
+    (∀k. j + k < LENGTH w ⇒
+         EL (j+k+1) qs ∈ M2.delta (EL (j+k) qs) (EL (j+k) w))
 Proof
   rw[] >>
-  Cases_on ‘q = G.q_0’ >- gvs[rip_def] >>
-  Cases_on ‘q = G.C’  >- gvs[rip_def] >>
-  metis_tac[gnfaA'_gnfa_accepts,gnfa_accepts_gnfaA',gnfaA'_rip_filter]
+  ‘∃q0. M2.initial = {q0}’ by
+    metis_tac [is_dfa_def] >> qexists_tac ‘q0’ >> simp[] >>
+  ‘∃j. j < LENGTH qs ∧ EL j qs ∈ M2.Q ∧ ∀m. m < j ⇒ EL m qs ∈ M1.Q’ by
+     (qexists_tac ‘LEAST i. i < LENGTH qs ∧ EL i qs ∈ M2.Q’ >>
+      numLib.LEAST_ELIM_TAC >> rw[]
+      >- (‘qs ≠ []’ by metis_tac [is_exec_nonempty] >>
+          fs [LAST_EL,NOT_NIL_EQ_LENGTH_NOT_0] >>
+          qexists_tac ‘PRE (LENGTH qs)’ >> rw[] >>
+          metis_tac [is_dfa_def,wf_nfa_def,SUBSET_DEF])
+      >- (first_x_assum drule >> rw[] >>
+          ‘EVERY (λq. q ∈ M1.Q ∪ M2.Q) qs’ by
+             (irule nfa_dot_states >> metis_tac [is_dfa_def]) >>
+          fs [EVERY_EL] >> metis_tac [LESS_TRANS])) >>
+  qexists_tac ‘j’ >> rpt conj_asm1_tac
+  >- (spose_not_then assume_tac >> ‘j= 0 ∨ j = 1’ by decide_tac >> rw[]
+      >- (fs[EXTENSION] >> metis_tac [is_dfa_def,wf_nfa_def,SUBSET_DEF])
+      >- (pop_forget_tac >>
+          ‘EL 0 qs ∈ M1.Q’ by metis_tac [DECIDE “0 < 1”] >>
+          forget_tac is_forall >>
+          ‘M1.initial ∩ M1.final = ∅’ by
+             metis_tac[is_dfa_def, epsilon_in_nfa_lang] >>
+          ‘HD qs ∉ M1.final’ by
+             (fs[EXTENSION] >> metis_tac []) >>
+          drule is_exec_length >> strip_tac >>
+          ‘0 < LENGTH w’ by decide_tac >>
+          drule is_exec_Sigma >> disch_tac >> fs [EVERY_EL] >>
+          first_x_assum drule >> strip_tac >>
+          drule is_exec_delta >> rw[] >>
+          qexists_tac ‘0’ >> rw [nfa_dot_def] >> fs[EXTENSION] >>
+          metis_tac [is_dfa_def,wf_nfa_def,SUBSET_DEF]))
+  >- asm_rewrite_tac[]
+  >- (rw[] >> ‘EL i qs ∈ M1.Q ∧ EL (i+1) qs ∈ M1.Q’ by rw[] >>
+      drule is_exec_length >> rw [] >> fs[] >>
+      ‘i < LENGTH w’ by decide_tac >>
+      drule is_exec_Sigma >> strip_tac >> fs [EVERY_EL] >>
+      first_x_assum drule >> rw[] >>
+      drule is_exec_delta >> rw[] >> first_x_assum drule >>
+      rw [nfa_dot_def] >> fs[EXTENSION] >>
+      metis_tac [is_dfa_def,wf_nfa_def,SUBSET_DEF])
+  >- (drule is_exec_length >> rw [] >> fs[] >>
+      ‘EL (j-1) qs ∈ M1.Q ∧ j-1 < LENGTH w’ by rw[] >>
+      drule is_exec_delta >> rw[] >> first_x_assum drule >>
+      rw [nfa_dot_def] >> fs[] >> strip_tac >>
+      drule is_exec_Sigma >> strip_tac >> fs [EVERY_EL] >>
+      fs [EXTENSION] >>
+      ‘j-1 < LENGTH w’ by rw[] >>
+      metis_tac [is_dfa_def,wf_nfa_def,SUBSET_DEF])
+  >- (drule is_exec_length >> rw [] >> fs[] >>
+       ‘EL (j-1) qs ∈ M1.Q ∧ j-1 < LENGTH w’ by rw[] >>
+       drule is_exec_delta >> rw[] >> first_x_assum drule >>
+       rw [nfa_dot_def] >> fs[] >>
+       drule is_exec_Sigma >> strip_tac >> fs [EVERY_EL] >>
+       fs [EXTENSION] >>
+       ‘j-1 < LENGTH w’ by rw[] >>
+      metis_tac [is_dfa_def,wf_nfa_def,SUBSET_DEF])
+  >- (rw [] >> rpt (forget_tac is_forall) >>
+      drule is_exec_length >> rw [] >> fs[] >> rw[] >>
+      ‘EL (j+k) qs ∈ M2.Q’ by
+         (Induct_on ‘k’ >> rw[] >>
+          irule nfa_dot_delta_second_states >> rw []
+          >- metis_tac [is_dfa_def]
+          >- (qexistsl_tac [‘M1’, ‘EL (j+k) w’,‘EL (j+k) qs’] >>
+              simp[] >> rpt conj_asm1_tac
+              >- metis_tac [is_dfa_def]
+              >- (drule is_exec_Sigma >> strip_tac >> fs [EVERY_EL])
+              >- (‘EL (j + k) qs ∈ M2.Q’ by rw[] >>
+                  ‘j+k < LENGTH w’ by rw[] >>
+                  drule_all is_exec_delta >>
+                  metis_tac [DECIDE “j + k + 1 = j + SUC k”]))) >>
+      drule is_exec_Sigma >> strip_tac >> fs [EVERY_EL] >>
+      drule is_exec_delta >> rw[] >> first_x_assum drule >>
+      rw [nfa_dot_def] >> fs[EXTENSION] >> metis_tac[])
 QED
 
-Theorem G_rip_sim:
-  ∀s q. wfm_gnfa G ∧ q ≠ G.q_0 ∧ q ≠ G.C ∧ q ∈ G.Q ⇒
-         (gnfa_accepts (rip G q) G.q_0 s G.C ⇔ gnfa_accepts G G.q_0 s G.C)
+Theorem nfa_dot_snip:
+  is_dfa M1 ∧ is_dfa M2 ∧
+  M1.Sigma = M2.Sigma ∧ M1.Q ∩ M2.Q = ∅ ∧
+  ε ∉ nfa_lang M1 ∧ ε ∉ nfa_lang M2
+  ⇒
+   nfa_lang (nfa_dot M1 M2) ⊆ nfa_lang M1 dot nfa_lang M2
 Proof
-  metis_tac[G_rip_back_sim,G_rip_forw_sim,wfm_gnfa_def]
+  rw [SUBSET_DEF] >> rename1 ‘w ∈ _’ >>
+  ‘wf_nfa (nfa_dot M1 M2)’ by
+    metis_tac [is_dfa_def,wf_nfa_dot] >>
+  drule_all in_nfa_lang_is_accepting_exec >> rw[is_accepting_exec_def] >>
+  qpat_forget_tac ‘w ∈ nfa_lang _’ >> qpat_forget_tac ‘~NULL qs’ >>
+  drule_all nfa_dot_snip_lemma >> rw [IN_dot] >>
+  qexistsl_tac [‘TAKE (j-1) w’, ‘DROP (j-1) w’] >> rw[in_nfa_lang] >>
+  TRY (drule is_exec_Sigma >> rw [nfa_dot_def,EVERY_TAKE,EVERY_DROP])
+  >- (qexists_tac ‘TAKE j qs’ >> rw[]
+      >- (drule is_exec_length >> rw[LENGTH_TAKE])
+      >- rw [HD_TAKE]
+      >- (‘LAST (TAKE j qs) = EL (j − 1) qs’ suffices_by metis_tac[] >>
+          ‘TAKE j qs ≠ []’ by rw [NOT_NIL_EQ_LENGTH_NOT_0] >>
+          rw [LAST_EL,EL_TAKE])
+      >- (drule is_exec_length >> disch_tac >>
+          ‘j - 1 < LENGTH w’ by decide_tac >>
+          fs [LENGTH_TAKE,EL_TAKE]))
+  >- (qexists_tac ‘q0::DROP j qs’ >> rw[]
+      >- (drule is_exec_length >> rw[])
+      >- (‘DROP j qs ≠ []’ by rw [NOT_NIL_EQ_LENGTH_NOT_0] >>
+          rw [LAST_DEF,last_drop])
+      >- (rename1 ‘k < LENGTH w + 1 − j’ >>
+          Cases_on ‘k’ >> rw[]
+          >- rw [HD_DROP]
+          >- (rw [Once (GSYM ADD1),EL_restricted] >>
+              drule is_exec_length >> rw [EL_DROP] >>
+              ‘j + SUC n - 1 = j + n’ by decide_tac >> pop_subst_tac >>
+              ‘j + SUC n = j + (n + 1)’ by decide_tac >> pop_subst_tac >>
+              first_x_assum irule >> decide_tac)))
 QED
 
-Definition reduced_gnfa_def:
-  reduced_gnfa G =
-    if FINITE G.Q ∧ 2 < CARD G.Q then
-      reduced_gnfa (rip G (MAX_SET (G.Q DIFF {G.q_0; G.C})))
-    else
-      G
+Theorem REGULAR_CLOSED_UNDER_EPSILON_FREE_DOT:
+  ε ∉ L1 ∧ ε ∉ L2 ∧
+  (L1,A) ∈ REGULAR ∧
+  (L2,A) ∈ REGULAR
+  ⇒
+  (L1 dot L2, A) ∈ REGULAR
+Proof
+  disch_then (strip_assume_tac o SRULE [IN_REGULAR_AS_DFA]) >> rw[] >>
+  rename1 ‘M1.Sigma = M2.Sigma’ >>
+  ‘∃M2a. is_dfa M2a ∧ nfa_lang M2a = nfa_lang M2 ∧
+         M1.Q ∩ M2a.Q = ∅ ∧ M2a.Sigma = M2.Sigma’ by
+    (‘FINITE M1.Q ∧ wf_nfa M2’ by metis_tac [is_dfa_def, wf_nfa_def] >>
+     drule_all RENAME_STATES_APART >> metis_tac []) >>
+  rw [IN_REGULAR] >> pop_sym_subst_tac >> qpat_forget_tac ‘is_dfa M2’ >>
+  qpat_x_assum ‘nfa_lang M2a = nfa_lang M2’ sym_subst_all_tac >>
+  rename1 ‘M1.Sigma = M2.Sigma’ >>
+  qexists_tac ‘nfa_dot M1 M2’ >> rpt conj_tac
+  >- rw [nfa_dot_def]
+  >- metis_tac [is_dfa_def,wf_nfa_dot]
+  >- metis_tac [nfa_dot_paste, nfa_dot_snip, SET_EQ_SUBSET]
+QED
+
+(*---------------------------------------------------------------------------*)
+(* Closure under concatenation, at last. There's some case analysis on       *)
+(* whether the component languages include the empty string before getting   *)
+(* to the main argument, in which both languages do not include ε.           *)
+(*---------------------------------------------------------------------------*)
+
+Theorem REGULAR_CLOSED_UNDER_DOT:
+  (L1,A) ∈ REGULAR ∧ (L2,A) ∈ REGULAR ⇒ (L1 dot L2,A) ∈ REGULAR
+Proof
+  strip_tac >> imp_res_tac REGULAR_SIGMA_FINITE >>
+  strip_assume_tac (Q.ISPEC ‘L1 : num list -> bool’ isolate_corner_cases) >>
+  rename1 ‘s1 ⊆ {ε}’ >>
+  strip_assume_tac (Q.ISPEC ‘L2 : num list -> bool’ isolate_corner_cases) >>
+  rename1 ‘s2 ⊆ {ε}’ >>
+  ONCE_ASM_REWRITE_TAC[] >>
+  simp [DOT_UNION_LDISTRIB,DOT_UNION_RDISTRIB,PUSH_EXISTS,GSYM UNION_ASSOC] >>
+  rpt (irule REGULAR_CLOSED_UNDER_UNION ORELSE conj_tac)
+  >- metis_tac [TRIVIAL_DOT_TRIVIAL_IN_REGULAR]
+  >- metis_tac [TRIVIAL_DOT_EPSILON_FREE_IN_REGULAR]
+  >- metis_tac [TRIVIAL_DOT_EPSILON_FREE_IN_REGULAR]
+  >- (irule REGULAR_CLOSED_UNDER_EPSILON_FREE_DOT >> rw[] >>
+      metis_tac [REGULAR_CLOSED_UNDER_EPSILON_DELETION])
+QED
+
+(*---------------------------------------------------------------------------*)
+(*---------------------------------------------------------------------------*)
+
+(*
+  From
+
+    wlist = [w1 ; ... ; wn]
+
+  obtain
+
+    qslist = [qs1 ; ... ; qsn]
+
+  where
+
+    is_accepting_exec qsi wi holds, for i < LENGTH wlist
+
+  To then build the execution for the nfa_plus machine, we basically want
+  to build the full nfa_plus state list as "FLAT qslist". But, as for the
+  nfa_dot pasting lemma, we have to arrange for the branching back from
+  accept states to skip over the initial state. Thus for every qsi, i > 1,
+  drop the HD:
+
+        nfa_plus_qs = qs1 ++ TL qs2 ++ ... ++ TL qsn
+*)
+
+Triviality qslist_length:
+  ∀wlist qslist.
+  LIST_REL (is_accepting_exec M) qslist wlist
+  ⇒
+  LENGTH (FLAT qslist) = LENGTH (FLAT wlist) + LENGTH wlist
+Proof
+ Induct_on ‘wlist’ >> rw[] >> fs[] >>
+ rename1 ‘is_accepting_exec M qs w’ >>
+ ‘LENGTH qs = LENGTH w + 1’ suffices_by decide_tac >>
+ metis_tac [is_accepting_exec_def,is_exec_length]
+QED
+
+Triviality length_flat_tl_lem:
+  EVERY (λlist. list ≠ []) ll
+  ⇒
+  LENGTH (FLAT (MAP TL ll)) + LENGTH ll = LENGTH (FLAT ll)
+Proof
+  Induct_on ‘ll’ >> rw[] >> fs[] >>
+  rw [DECIDE“a + (b + SUC c) = (a + c) + b + 1”] >>
+  qpat_x_assum ‘_ = _’ (subst_all_tac o SYM) >> rw[] >>
+  ‘LENGTH (TL h) + 1 = LENGTH h’ suffices_by decide_tac >>
+  fs[NOT_NIL_EQ_LENGTH_NOT_0,LENGTH_TL]
+QED
+
+Triviality LAST_APPEND_FLAT:
+  ll ≠ [] ∧ LAST ll ≠ []
+  ⇒
+  LAST (list ++ FLAT ll) = LAST (LAST ll)
+Proof
+  rw[] >> drule_all LAST_FLAT >> disch_tac >>
+  drule FLAT_NOT_NIL >> rw[LAST_APPEND_NOT_NIL]
+QED
+
+Theorem nfa_plus_delta_subset:
+ M.delta q a ⊆ (nfa_plus M).delta q a
+Proof
+ rw [nfa_plus_def]
+QED
+
+Theorem is_accepting_exec_nfa_plus:
+  is_accepting_exec M qs w ⇒ is_accepting_exec (nfa_plus M) qs w
+Proof
+  rw [is_accepting_exec_def, nfa_plus_def,is_exec_def] >> rw[]
+QED
+
+(*---------------------------------------------------------------------------*)
+(* Similar to the pasting theorem for nfa_dot. The difference is that, for   *)
+(* nfa_kplus, there's only one machine, which loops back from final states   *)
+(* to the successors of the start state.                                     *)
+(*---------------------------------------------------------------------------*)
+
+Theorem is_accepting_exec_nfa_plus_paste:
+  is_dfa M ∧
+  w1 ≠ ε ∧ w2 ≠ ε ∧
+  is_accepting_exec (nfa_plus M) qs1 w1 ∧
+  is_accepting_exec M qs2 w2
+  ⇒
+  is_accepting_exec (nfa_plus M) (qs1 ++ TL qs2) (w1 ++ w2)
+Proof
+  rw [is_accepting_exec_def] >>
+  ‘wf_nfa M ∧ wf_nfa (nfa_plus M)’ by
+     metis_tac [is_dfa_def,wf_nfa_plus] >>
+  ‘EVERY (λq. q ∈ (nfa_plus M).Q) qs1 ∧ EVERY (λq. q ∈ M.Q) qs2’ by
+     metis_tac [is_dfa_def,is_exec_states] >>
+  ‘qs1 ≠ [] ∧ qs2 ≠ []’ by
+     metis_tac [is_exec_nonempty] >>
+  ‘TL qs2 ≠ []’ by
+     metis_tac [is_accepting_exec_length,is_accepting_exec_def,is_dfa_def] >>
+  rw [is_exec_def]
+  >- fs [is_exec_def]
+  >- fs [is_exec_def]
+  >- (imp_res_tac is_exec_length >> rw[LENGTH_TL])
+  >- metis_tac [is_dfa_def,wf_nfa_def,SUBSET_DEF]
+  >- (‘n < LENGTH w1 ∨ n = LENGTH w1 ∨ LENGTH w1 < n’ by decide_tac
+      >- (rev_drule is_exec_Sigma >> simp[] >> rw[EVERY_EL] >>
+          rev_drule is_exec_length >> strip_tac >>
+          ‘n < LENGTH qs1’ by decide_tac >> ‘n+1 < LENGTH qs1’ by decide_tac >>
+          rw[EL_APPEND1] >>metis_tac [is_exec_delta,is_dfa_def])
+      >- (rw[] >> rfs[] >> rev_drule is_exec_length >>
+          disch_then(assume_tac o SYM) >> ONCE_ASM_REWRITE_TAC[] >>
+          rw[SRULE [NULL_EQ] EL_LENGTH_APPEND] >>
+          ‘LENGTH w1 < LENGTH qs1’ by decide_tac >> rw [EL_APPEND1] >>
+          ‘LENGTH w1 = PRE (LENGTH qs1)’ by decide_tac >> pop_subst_tac >>
+          rw [EL_PRE_LENGTH] >> rw [nfa_plus_def,PULL_EXISTS] >>
+          disj2_tac >> rfs [is_dfa_def,NOT_NIL_EQ_LENGTH_NOT_0] >> rw[] >>
+          ‘0 < LENGTH w1’ by decide_tac >> PURE_REWRITE_TAC[GSYM EL] >>
+          drule is_exec_delta >> disch_then drule >> simp[] >> rfs[])
+      >- (‘∃k. 0 < k ∧ k < LENGTH w2 ∧ n = LENGTH w1 + k’
+            by (qexists_tac ‘n - LENGTH w1’ >> fs[]) >> rw[EL_APPEND2_ALT] >>
+          rev_drule is_exec_length >> disch_tac >>
+          ‘k + (LENGTH w1 + 1) = LENGTH qs1 + k’ by decide_tac >> pop_subst_tac >>
+          drule is_exec_length >> disch_tac >>
+          ‘k < LENGTH (TL qs2)’ by
+             (‘k + 1 < LENGTH qs2’ by decide_tac >>
+              drule LENGTH_TL_ALT >> rw[]) >>
+          ‘k < LENGTH qs2’ by decide_tac >>
+          rw[EL_APPEND2_ALT] >> rw[EL_APPEND_EQN] >> rw [nfa_plus_def,PULL_EXISTS]
+          >- metis_tac [is_exec_delta]
+          >- (disj1_tac >>
+             ‘EL k qs2 ∈ M.Q’ by
+                metis_tac[is_dfa_def,wf_nfa_def, SUBSET_DEF] >>
+             drule is_exec_delta >> disch_then drule >> metis_tac[]))
+     )
+  >- rw[LAST_APPEND_NOT_NIL]
+QED
+
+Theorem is_accepting_exec_nfa_plus_paste_list:
+  ∀f qs qslist wlist w.
+    (f = λa b c. a ⧺ TL b) ∧
+    is_dfa M ∧ w ≠ ε ∧
+    EVERY (λw. w ≠ ε) wlist ∧
+    is_accepting_exec (nfa_plus M) qs w ∧
+    LIST_REL (is_accepting_exec M) qslist wlist
+    ⇒
+    is_accepting_exec (nfa_plus M)
+      (FOLDL2 f qs qslist wlist)
+      (FLAT (w::wlist))
+Proof
+  ho_match_mp_tac FOLDL2_ind >> rw[] >>
+  first_x_assum irule >> rw[] >>
+  irule is_accepting_exec_nfa_plus_paste >> rw[]
+QED
+
+Theorem KPLUS_SUBSET_NFA_PLUS:
+  is_dfa M ∧ ε ∉ nfa_lang M
+  ⇒
+  KPLUS (nfa_lang M) ⊆ nfa_lang (nfa_plus M)
+Proof
+  rw [SUBSET_DEF] >>
+  drule_all (iffLR IN_KPLUS_LIST_EPSILON_FREE) >> rw[] >>
+  ‘wf_nfa M ∧ wf_nfa (nfa_plus M)’ by
+     metis_tac [is_dfa_def,wf_nfa_plus] >>
+  ‘∃qslist. LIST_REL (is_accepting_exec M) qslist wlist’ by
+     (fs [in_nfa_lang_iff_accepting_exec,EVERY_EL,SUBSET_SKOLEM_THM] >>
+      qexists_tac ‘GENLIST f (LENGTH wlist)’ >> rw[LIST_REL_EL_EQN]) >>
+  ‘qslist ≠ []’ by
+     (Cases_on ‘qslist’ >> fs[]) >>
+  ‘EVERY (λqs. qs ≠ []) qslist’ by
+     (rw [EVERY_EL] >> fs[LIST_REL_EL_EQN,is_accepting_exec_def] >>
+      metis_tac [is_exec_nonempty]) >>
+  ‘EVERY (λqs. TL qs ≠ []) qslist’ by
+     (fs [EVERY_EL,LIST_REL_EL_EQN,is_accepting_exec_def] >>
+      metis_tac [is_exec_tl_nonempty]) >>
+  ‘EVERY (λw. w ≠ ε) wlist’ by
+     (fs [EVERY_EL] >> rw[] >> metis_tac[]) >>
+  ‘LENGTH qslist = LENGTH wlist’ by
+     metis_tac [LIST_REL_LENGTH] >>
+  rw [in_nfa_lang_iff_accepting_exec] >>
+  qexists_tac
+    ‘FOLDL2 (λa b c. a ++ TL b)
+       (HD qslist) (TL qslist) (TL wlist)’ >>
+  ‘∃qs qslist'. qslist = qs::qslist'’ by (Cases_on‘qslist’ >> fs[]) >>
+  ‘∃w wlist'. wlist = w::wlist'’ by (Cases_on ‘wlist’ >> fs[]) >> rw[] >> fs[] >>
+  drule is_accepting_exec_nfa_plus >> rw_tac bool_ss [Once (GSYM FLAT)] >>
+  irule is_accepting_exec_nfa_plus_paste_list >> rw[]
+QED
+
+(*
+Triviality SPLITP_EXISTS:
+  EXISTS P list ⇒ ∃prefix h t. SPLITP P list = (prefix,h::t)
+Proof
+  Induct_on ‘list’ >> rw[SPLITP] >> gvs[]
+QED
+
+Theorem zip_expand_id:
+ ZIP (MAP FST plist, MAP SND plist) = plist
+Proof
+ Induct_on ‘plist’ >> rw[]
+QED
+
+Theorem pair_list_as_zip:
+  ∀plist:('a # 'b) list. ∃l1 l2. LENGTH l1 = LENGTH l2 ∧ plist = ZIP (l1,l2)
+Proof
+ Induct_on ‘plist’ >> rw[]
+ >- (ntac 2 (qexists_tac ‘[]’) >> rw[])
+ >- (namedCases_on ‘h’ ["a b"] >>
+     qexists_tac ‘a::l1’ >> qexists_tac ‘b::l2’ >> rw[])
+QED
+
+Triviality UNZIP_APPEND:
+ ∀L1 L2. UNZIP (L1 ++ L2) = (FST (UNZIP L1) ++ FST (UNZIP L2),
+                             SND (UNZIP L1) ++ SND (UNZIP L2))
+Proof
+ Induct >> rw[]
+QED
+
+Theorem ZIP_EQ_NIL_OR:
+ ZIP(l1,l2) = [] ⇔ l1 = [] ∨ l2 = []
+Proof
+ Induct_on ‘l1’ >> Induct_on ‘l2’ >> rw[ZIP_def]
+QED
+
+
+*)
+
+Triviality nfa_plus_diff:
+  is_dfa M ∧
+  a ∈ M.Sigma ∧
+  q2 ∈ (nfa_plus M).delta q1 a ∧
+  q2 ∉ M.delta q1 a ⇒
+  q1 ∈ M.final ∧ BIGUNION {M.delta q0 a | q0 | q0 ∈ M.initial} = {q2}
+Proof
+  rw [is_dfa_def,nfa_plus_def] >> rfs[] >> rw[] >>
+  rename1 ‘q2 ∈ M.delta q0 a’ >>
+  rw [EXTENSION,EQ_IMP_THM]
+  >- (‘∃q'. M.delta q0 a = {q'}’ by
+        metis_tac [wf_nfa_def,SUBSET_DEF,IN_INSERT] >> gvs[])
+  >- metis_tac []
+QED
+
+(*---------------------------------------------------------------------------*)
+(* One step of splitting an "nfa_plus(M)" execution into a leading "M"       *)
+(* execution followed by either (A) an empty execution, or, (B) by another   *)
+(* nfa_plus(M) execution. Note the start state has to be attached before the *)
+(* tail nfa_plus(M) execution becomes well-formed.                           *)
+(*                                                                           *)
+(* Subtlety: cronch splits off the longest M-execution it can.               *)
+(*---------------------------------------------------------------------------*)
+
+Definition cronch_def:
+  cronch M [] [] = ([],[],[],[]) ∧
+  cronch M [a] [q] = ([a],[],[q],[]) ∧
+  cronch M (a::b::w) (q1::q2::qs) =
+     if q2 ∈ M.delta q1 b then
+       (case cronch M (b::w) (q2::qs)
+         of (wpref,wsuff,qpref,qsuff) =>
+            (a::wpref, wsuff, q1::qpref, qsuff))
+     else ([a], b::w, [q1], q2::qs)
+End
+
+Triviality cronch_splits_input:
+ ∀M w qs wpref wsuff qpref qsuff.
+   LENGTH qs = LENGTH w ∧
+   cronch M w qs = (wpref,wsuff,qpref,qsuff)
+   ⇒
+   wpref ++ wsuff = w ∧
+   qpref ++ qsuff = qs ∧
+   LENGTH wpref = LENGTH qpref ∧
+   LENGTH wsuff = LENGTH qsuff
+Proof
+  recInduct cronch_ind >>
+  rw [cronch_def,AllCaseEqs()] >> simp[]
+QED
+
+Triviality cronch_consumes_lem:
+ ∀M w qs wpref wsuff qpref qsuff a q w' qs'.
+   LENGTH qs = LENGTH w ∧
+   w = a::w' ∧ qs = q::qs' ∧
+   cronch M w qs = (wpref,wsuff,qpref,qsuff)
+   ⇒
+   ∃wpref' qpref'.  wpref = a::wpref' ∧ qpref = q::qpref'
+Proof
+  recInduct cronch_ind >> rw [cronch_def,AllCaseEqs()]
+QED
+
+Theorem cronch_consumes = cronch_consumes_lem |> SRULE[];
+
+(*---------------------------------------------------------------------------*)
+(* Given |- ∀xs. P ⇒ Q1 ∧ Q2, return |- ∀xs. P ⇒ Q1 and |- ∀xs. P ⇒ Q2       *)
+(*---------------------------------------------------------------------------*)
+
+fun fst_conj th =
+ let val (xs,t) = strip_forall(concl th)
+     val ant = fst(dest_imp t)
+     val th1 = CONJUNCT1(UNDISCH(SPEC_ALL th))
+ in
+   GENL xs (DISCH ant th1)
+ end
+
+fun snd_conj th =
+ let val (xs,t) = strip_forall(concl th)
+     val ant = fst(dest_imp t)
+     val th1 = CONJUNCT2(UNDISCH(SPEC_ALL th))
+ in
+   GENL xs (DISCH ant th1)
+ end
+
+Triviality ELT_SUBSET:
+  a ∈ s ⇔ {a} ⊆ s
+Proof
+ rw[EQ_IMP_THM]
+QED
+
+Theorem cronch_exec:
+ ∀M w qs q0 wpref wsuff qpref qsuff.
+   is_dfa M ∧
+   M.initial = {q0} ∧
+   w ≠ ε ∧
+   LAST qs ∈ M.final ∧
+   is_exec (nfa_plus M) qs (TL w) ∧
+   cronch M w qs = (wpref,wsuff,qpref,qsuff)
+   ⇒
+     is_exec M qpref (TL wpref) ∧
+     LAST qpref ∈ M.final ∧
+     (qsuff = [] ∨ is_exec (nfa_plus M) (q0::qsuff) wsuff)
+Proof
+  recInduct cronch_ind >> simp [] >>
+  rpt conj_tac >> rpt (gen_tac ORELSE disch_tac)
+  >~ [‘cronch M (a::b::w) (q1::q2::qs) = (wpref,wsuff,qpref,qsuff)’]
+  >- (pop_keep_tac >> simp [cronch_def,AllCaseEqs(),PULL_EXISTS] >>
+      rw[] >> gvs[]
+      >- (‘LENGTH qs = LENGTH w’ by gvs[is_exec_def] >>
+          imp_res_tac cronch_consumes >> rw[] >> gvs[] >>
+          irule is_exec_extend_left >> gvs [is_dfa_def] >>
+          drule is_exec_Sigma >> rw[]
+          >- gvs [is_exec_def]
+          >- (first_x_assum (irule_at Any o fst_conj) >>
+              irule (snd_conj is_exec_step_left) >> metis_tac [wf_nfa_plus]))
+      >- (‘LENGTH qs = LENGTH w’ by gvs[is_exec_def] >>
+          imp_res_tac cronch_consumes >> rw[] >> gvs[] >>
+          first_x_assum (irule_at Any o fst_conj o snd_conj) >>
+          irule (snd_conj is_exec_step_left) >>
+          metis_tac [is_dfa_def,wf_nfa_plus])
+      >- (first_x_assum (irule_at Any o snd_conj o snd_conj) >>
+          irule (snd_conj is_exec_step_left) >>
+          metis_tac [is_dfa_def,wf_nfa_plus])
+      >- gvs [is_exec_def]
+      >- (gvs [is_exec_def,nfa_plus_def] >>
+          ‘0 < SUC (LENGTH w)’ by decide_tac >>
+          first_x_assum drule >> simp[] >> rw[])
+      >- (‘LENGTH w = LENGTH qs’ by gvs[is_exec_def] >>
+          ‘wf_nfa (nfa_plus M)’ by metis_tac [wf_nfa_plus,is_dfa_def] >>
+          imp_res_tac is_exec_step_left >>
+          ‘b ∈ M.Sigma’ by gvs [is_exec_def] >>
+          irule is_exec_extend_left >> rw[]
+          >- metis_tac [IN_INSERT,SUBSET_DEF,wf_nfa_def,is_dfa_def]
+          >- (‘b ∈ M.Sigma’ by gvs [is_exec_def] >>
+              drule_all nfa_plus_diff >> rw[nfa_plus_def] >>
+              irule (iffRL ELT_SUBSET) >> pop_sym_subst_tac >>
+              simp[SUBSET_DEF])))
+  >> gvs[cronch_def, is_exec_def]
+QED
+
+Theorem cronch_accepting_exec:
+   is_dfa M ∧ M.initial = {q0} ∧ w ≠ ε ∧
+   is_accepting_exec (nfa_plus M) qs (TL w) ∧
+   cronch M w qs = (wprefix,wsuffix,qprefix,qsuffix)
+   ⇒
+   is_accepting_exec M qprefix (TL wprefix) ∧
+   (qsuffix = [] ∨ is_accepting_exec (nfa_plus M) (q0::qsuffix) wsuffix)
+Proof
+ rw[is_accepting_exec_def] >>
+ ‘LENGTH qs = LENGTH w’ by
+   (Cases_on ‘w’ >> Cases_on ‘qs’ >> gvs[is_exec_def]) >>
+ drule_all cronch_exec >>
+ rpt CASE_TAC >> rw[]
+ >- (Cases_on ‘qs’ >> Cases_on ‘w’ >> gvs[is_exec_def] >>
+     drule_all cronch_consumes >> rw[] >> gvs[])
+ >- (Cases_on ‘qs’ >> Cases_on ‘w’ >> gvs[is_exec_def] >>
+     drule_all cronch_consumes >> rw[] >> gvs[])
+ >- (Cases_on ‘qsuffix’ >> simp[] >>
+     drule_all cronch_splits_input >> rw[] >>
+     metis_tac [NOT_CONS_NIL,LAST_APPEND_NOT_NIL,APPEND_ASSOC,APPEND])
+QED
+
+Triviality cronch_accepting_exec_alt:
+  is_dfa M ∧ M.initial = {q0} ∧ is_accepting_exec (nfa_plus M) qs w ∧
+  cronch M (ARB::w) qs = (wprefix,wsuffix,qprefix,qsuffix)
+  ⇒
+  is_accepting_exec M qprefix (TL wprefix) ∧
+  (qsuffix = [] ∨ is_accepting_exec (nfa_plus M) (q0::qsuffix) wsuffix)
+Proof
+ ACCEPT_TAC
+    (cronch_accepting_exec |> Q.INST [‘w’ |-> ‘ARB::w’] |> SRULE[])
+QED
+
+(*---------------------------------------------------------------------------*)
+(* Termination: the input gets smaller since an M-execution (which must have *)
+(* at least two states) is removed each time.                                *)
+(*---------------------------------------------------------------------------*)
+
+Theorem epsilon_free_accepting_exec_length:
+   wf_nfa N ∧ ε ∉ nfa_lang N ∧
+   is_accepting_exec N qs w
+   ⇒
+   ∃q1 q2 qs'. qs = q1::q2::qs'
+Proof
+  rw[] >> gvs [in_nfa_lang_iff_accepting_exec] >>
+  ‘w ≠ ε’ by metis_tac[] >>
+  metis_tac[epsilon_free_exec_left_cons,is_accepting_exec_def]
+QED
+
+Definition cronch_all_def:
+  cronch_all M q0 w qs =
+    if is_dfa M ∧ ε ∉ nfa_lang M ∧
+       is_accepting_exec (nfa_plus M) qs w
+   then
+    (case cronch M (ARB::w) qs of (wprefix,wsuffix,qprefix,qsuffix)
+      => if qsuffix = [] then
+           ([TL wprefix],[qprefix])
+         else
+          case cronch_all M q0 wsuffix (q0::qsuffix)
+           of (wprefixes,qprefixes) => (TL wprefix::wprefixes, qprefix::qprefixes))
+  else
+    ARB
 Termination
-  WF_REL_TAC ‘measure (λG. CARD G.Q)’ >>
-  rw[rip_def] >> Cases_on ‘FINITE G.Q’ >> simp[] >> strip_tac >>
-  ‘G.Q DIFF {G.q_0; G.C} ≠ ∅’
-    by (simp[SUBSET_DIFF_EMPTY] >> strip_tac >>
-        drule_at (Pos last) CARD_SUBSET >>
-        gvs[]) >>
-  ‘FINITE (G.Q DIFF {G.q_0; G.C})’
-    by simp[] >>
-  drule_all (cj 1 MAX_SET_DEF) >> gvs[]
+  WF_REL_TAC ‘measure (λ(a,b,c,d). LENGTH d)’ >> rw[] >>
+  rename1 ‘cronch M (ARB::w) qs = (wprefix,wsuffix,qprefix,qsuffix)’ >>
+  ‘∃q0. M.initial = {q0}’ by metis_tac [is_dfa_def] >>
+  imp_res_tac (cronch_accepting_exec |> Q.INST [‘w’ |-> ‘ARB::w’] |> SRULE[] |> fst_conj) >>
+  ‘∃q1 q2 qs'. qprefix = q1::q2::qs'’ by
+     metis_tac [epsilon_free_accepting_exec_length,is_dfa_def] >>
+  ‘LENGTH qs = LENGTH (ARB::w)’ by gvs [is_accepting_exec_def,is_exec_def] >>
+  drule_all cronch_splits_input >> rw[] >> gvs[]
 End
 
-Theorem reduced_gnfa_same:
-  wfm_gnfa G ⇒
-    (gnfa_accepts G G.q_0 s G.C ⇔
-    gnfa_accepts (reduced_gnfa G) (reduced_gnfa G).q_0 s (reduced_gnfa G).C)
+Theorem cronch_all_thm:
+  ∀M q0 w qs wslist qslist.
+  is_dfa M ∧ M.initial = {q0} ∧
+  ε ∉ nfa_lang M ∧
+  is_accepting_exec (nfa_plus M) qs w ∧
+  cronch_all M q0 w qs = (wslist,qslist)
+  ⇒
+  LIST_REL (is_accepting_exec M) qslist wslist ∧
+  w = FLAT wslist ∧
+  wslist ≠ []
 Proof
-  reverse (Cases_on ‘FINITE G.Q’)
-  >- (ntac 3 (rw[Once reduced_gnfa_def])) >>
-  pop_assum mp_tac >> qid_spec_tac ‘G’ >>
-  ho_match_mp_tac reduced_gnfa_ind  >> rw[] >>
-  qabbrev_tac ‘ms = MAX_SET (G.Q DIFF {G.q_0; G.C})’ >>
-  gvs[] >> reverse (Cases_on ‘2 < CARD G.Q’)
-  >- (ntac 3 (rw[Once reduced_gnfa_def])) >>
-  gvs[] >>
-  ‘FINITE (rip G ms).Q’
-    by rw[rip_def] >>
-  gvs[wfm_rip_wfm] >>
-  ONCE_REWRITE_TAC [reduced_gnfa_def] >>
-  simp[] >>
-  last_x_assum (SUBST1_TAC o SYM) >>
-  simp[Once EQ_SYM_EQ] >>
-  ‘(rip G ms).q_0 = G.q_0 ∧ (rip G ms).C = G.C’
-    by rw[rip_def] >>
-  simp[] >> irule G_rip_sim >>
-  qunabbrev_tac ‘ms’ >>
-  ‘G.Q DIFF {G.q_0; G.C} ≠ ∅’
-    by (simp[SUBSET_DIFF_EMPTY] >> strip_tac >>
-        drule_at (Pos last) CARD_SUBSET >>
-        gvs[]) >>
-  ‘FINITE (G.Q DIFF {G.q_0; G.C})’
-    by simp[] >>
-  drule_all (cj 1 MAX_SET_DEF) >> gvs[]
+  recInduct cronch_all_ind >> rw[] >> fs[] >> pop_keep_tac >>
+  rw [Once cronch_all_def,AllCaseEqs(),PULL_EXISTS] >> fs[]
+  >- metis_tac [cronch_accepting_exec_alt]
+  >- (drule_all cronch_accepting_exec_alt >> rw[])
+  >- (drule_all cronch_accepting_exec_alt >> rw[] >>
+      ‘LENGTH qs = LENGTH (ARB::w)’ by
+         gvs [is_accepting_exec_def,is_exec_def] >>
+      imp_res_tac cronch_splits_input >> gvs[] >> rw[])
+  >- (drule_all cronch_accepting_exec_alt >> rw[] >> gvs[] >>
+      ‘LENGTH qs = LENGTH (ARB::w)’ by
+         gvs [is_accepting_exec_def,is_exec_def] >>
+      imp_res_tac cronch_splits_input >> gvs[] >>
+      qpat_x_assum ‘wprefix ⧺ FLAT wprefixes = ARB::w’
+        (SUBST1_TAC o SYM o SRULE[] o Q.AP_TERM ‘TL’) >> rw[] >>
+      irule TL_APPEND >>
+      ‘∃q1 q2 qs'. qprefix = q1::q2::qs'’ by
+        metis_tac[epsilon_free_accepting_exec_length,is_dfa_def] >> rw[] >>
+      Cases_on ‘wprefix’ >> gvs[])
 QED
 
-Theorem reduced_gnfa_facts[simp]:
-  ∀GN. (reduced_gnfa GN).q_0 = GN.q_0 ∧ (reduced_gnfa GN).C = GN.C
+Theorem nfa_plus_exec_to_nfa_execs:
+  is_dfa M ∧
+  ε ∉ nfa_lang M ∧
+  is_accepting_exec (nfa_plus M) qs w
+  ⇒
+  ∃qslist wlist.
+    LIST_REL (is_accepting_exec M) qslist wlist ∧
+    w = FLAT wlist ∧
+    wlist ≠ []
 Proof
-  ho_match_mp_tac reduced_gnfa_ind >> simp[] >> qx_gen_tac ‘GN’ >> strip_tac >>
-  ONCE_REWRITE_TAC[reduced_gnfa_def] >>
-  Cases_on ‘FINITE GN.Q ∧ 2 < CARD GN.Q’ >> simp[] >>
-  qmatch_abbrev_tac ‘(rip GN s).q_0 = GN.q_0 ∧ _’ >>
-  rw[rip_def]
+ metis_tac [cronch_all_thm,ABS_PAIR_THM,is_dfa_def]
 QED
 
-Theorem reduced_gnfas_have_two_states:
-  ∀GN. wfm_gnfa GN ⇒
-       (reduced_gnfa GN).Q = {GN.q_0 ; GN.C }
+Triviality LIST_REL_EVERY:
+  LIST_REL R l1 l2 ⇒ EVERY (λx. ∃y. R x y) l1
 Proof
-  ho_match_mp_tac reduced_gnfa_ind >> qx_gen_tac ‘GN’ >> rpt strip_tac >>
-  ONCE_REWRITE_TAC [reduced_gnfa_def] >> reverse (rw[])
-  >- (gvs[wfm_gnfa_def, arithmeticTheory.NOT_LESS] >>
-      simp[EXTENSION, EQ_IMP_THM, DISJ_IMP_THM] >> CCONTR_TAC >> gvs[] >>
-      rename [‘s ≠ GN.C’, ‘s ≠ GN.q_0’] >>
-      ‘{s; GN.C; GN.q_0} ⊆ GN.Q’ by simp[SUBSET_DEF] >>
-      ‘CARD {s;GN.C;GN.q_0} ≤ CARD GN.Q’ by metis_tac[CARD_SUBSET] >>
-      gvs[]) >>
-  gvs[wfm_rip_wfm] >> rw[rip_def]
+  rw[EVERY_MEM] >> drule_all LIST_REL_MEM_IMP >> metis_tac[]
 QED
 
-Theorem wfm_gnfa_reduced:
-  ∀GN. wfm_gnfa GN ⇒ wfm_gnfa (reduced_gnfa GN)
+Triviality LIST_REL_EVERY_R:
+  LIST_REL R l1 l2 ⇒ EVERY (λy. ∃x. R x y) l2
 Proof
-  ho_match_mp_tac reduced_gnfa_ind >> rw[] >>
-  ONCE_REWRITE_TAC [reduced_gnfa_def] >> rw[] >> gvs[] >>
-  simp[wfm_rip_wfm]
+  rw[EVERY_MEM] >> drule_all LIST_REL_MEM_IMP_R >> metis_tac[]
 QED
 
-Theorem thm_1_54_ltr:
-  ∀l. regularLanguage l ⇒ ∃r. regexp_lang r = l
+Theorem NFA_PLUS_SUBSET_KPLUS:
+  is_dfa M ∧ ε ∉ nfa_lang M
+  ⇒
+  nfa_lang (nfa_plus M) ⊆ KPLUS (nfa_lang M)
 Proof
-  simp[regularLanguage_def, recogLangD_def, PULL_EXISTS] >>
-  simp[EXTENSION] >>
-  qx_gen_tac ‘D’ >> strip_tac >>
-  drule_then (qx_choose_then ‘GN’ strip_assume_tac) dfa_to_gnfa_correct >>
-  simp[] >>
-  drule_then strip_assume_tac reduced_gnfa_same >> simp[] >>
-  ‘wfm_gnfa (reduced_gnfa GN)’ by simp[wfm_gnfa_reduced] >>
-  ONCE_REWRITE_TAC [gnfa_accepts_cases] >>
-  ‘GN.C ≠ GN.q_0’ by gvs[wfm_gnfa_def] >> simp[reduced_gnfas_have_two_states] >>
-  qexists_tac ‘(reduced_gnfa GN).tf GN.q_0 GN.C’ >> qx_gen_tac ‘str’ >> eq_tac
-  >- (strip_tac >> qexistsl_tac [‘str’, ‘[]’, ‘GN.C’] >>
-      simp[Once gnfa_accepts_cases, reduced_gnfas_have_two_states]) >>
-  rw[] >- gvs[wfm_gnfa_def] >>
-  ‘c2 = []’ suffices_by simp[] >>
-  pop_assum mp_tac >> ONCE_REWRITE_TAC[gnfa_accepts_cases] >>
-  rw[] >> gvs[wfm_gnfa_def]
+  strip_tac >> simp[SUBSET_DEF] >>
+  ‘wf_nfa M ∧ wf_nfa (nfa_plus M)’ by
+     metis_tac [is_dfa_def,wf_nfa_plus] >>
+  rw [in_nfa_lang_iff_accepting_exec] >>
+  rw [IN_KPLUS_LIST] >>
+  rw [in_nfa_lang_iff_accepting_exec] >>
+  drule_all nfa_plus_exec_to_nfa_execs >> rw[] >>
+  first_x_assum (irule_at Any) >> rw[] >>
+  metis_tac [LIST_REL_EVERY_R]
 QED
 
-Theorem thm_1_54:
-  regularLanguage l ⇔ ∃r. regexp_lang r = l
+Theorem REGULAR_CLOSED_UNDER_EPSILON_FREE_KPLUS:
+  ε ∉ L ∧ (L,A) ∈ REGULAR ⇒ (KPLUS L, A) ∈ REGULAR
 Proof
-  metis_tac[thm_1_54_ltr, lemma_1_55]
+  disch_then (strip_assume_tac o SRULE [IN_REGULAR_AS_DFA]) >> rw[] >>
+  rw [IN_REGULAR] >> qexists_tac ‘nfa_plus M’ >> rpt conj_tac
+  >- rw [nfa_plus_def]
+  >- metis_tac[wf_nfa_plus,is_dfa_def]
+  >- metis_tac [SET_EQ_SUBSET, KPLUS_SUBSET_NFA_PLUS, NFA_PLUS_SUBSET_KPLUS]
 QED
 
-Definition exp_def:
-  (exp s 0 = []) ∧
-  (exp s (SUC n) = s ++ (exp s n))
-End
-
-Theorem wf_dfa_remain_Q:
-  ∀M. wf_dfa M ⇒
-    ∀ss.
-      (∀n. n < LENGTH ss - 1 ⇒
-          ∃c.
-            M.tf (EL n ss) c = (EL (SUC n) ss)) ∧
-      HD ss ∈ M.Q ⇒
-      (∀e. MEM e ss ⇒ e ∈ M.Q)
+Theorem REGULAR_CLOSED_UNDER_KSTAR:
+  (L,A) ∈ REGULAR ⇒ (KSTAR L,A) ∈ REGULAR
 Proof
- ntac 2 strip_tac >>
- Induct_on ‘ss’ >> simp[DISJ_IMP_THM,FORALL_AND_THM] >>
- rw[] >>
- first_x_assum irule >>
- rw[]
- >- (first_x_assum (qspec_then ‘SUC n’ assume_tac) >>
-     rfs[] >> metis_tac[])
- >- (first_x_assum (qspec_then ‘0’ assume_tac) >>
-     Cases_on ‘ss’ >> fs[wf_dfa_def] >>
-     metis_tac[])
+  strip_tac >>
+  strip_assume_tac (Q.ISPEC ‘L:num list->bool’ isolate_corner_cases) >>
+  rename1 ‘s ⊆ {ε}’ >> ONCE_ASM_REWRITE_TAC[] >>
+  rw [KSTAR_UNION,KSTAR_TRIVIAL,DOT_EMPTYSTRING] >>
+  rw [GSYM KPLUS_UNION_EPSILON_EQ_KSTAR] >>
+  irule REGULAR_CLOSED_UNDER_UNION >> reverse conj_tac
+  >- metis_tac [EPSILON_LANG_IN_REGULAR,REGULAR_SIGMA_FINITE]
+  >- (irule REGULAR_CLOSED_UNDER_EPSILON_FREE_KPLUS >> rw[] >>
+      metis_tac [REGULAR_CLOSED_UNDER_EPSILON_DELETION])
 QED
 
-Theorem Delta_segment:
-∀i j ss s M.
-  (∀n. n < LENGTH ss − 1 ⇒ M.tf (EL n ss) (EL n s) = EL (n + 1) ss) ∧
-  i < LENGTH ss ∧ j ≤ i ∧ LENGTH ss = LENGTH s + 1 ⇒
-  Delta M (EL j ss) (DROP j (TAKE i s)) = EL i ss
+(*===========================================================================*)
+(* The Regular languages coincide with the Finite State languages.           *)
+(*===========================================================================*)
+
+Theorem REGULAR_SUBSET_FINITE_STATE:
+  REGULAR ⊆ FINITE_STATE
 Proof
-  Induct_on ‘i - j’ >> rw[] >- (‘i = j’ by simp[] >> rw[DROP_TAKE]) >>
-  ‘v = i - (SUC j)’ by simp[] >>
-  ‘DROP j (TAKE i s) = EL j s :: DROP (SUC j) (TAKE i s)’
-    by simp[DROP_CONS_EL, LENGTH_TAKE, EL_TAKE] >>
-  simp[] >> fs[ADD1]
+ cheat
 QED
 
-Theorem pumpingLemma:
-  ∀l. regularLanguage l ⇒
-      ∃p.∀s.
-           s ∈ l ∧ p ≤ LENGTH s ⇒
-           ∃x y z.
-             s = x ++ y ++ z ∧
-             ∀i.
-               (x ++ exp y i ++ z) ∈ l
+Theorem FINITE_STATE_SUBSET_REGULAR:
+  FINITE_STATE ⊆ REGULAR
 Proof
-  (* We decided this should be changed to use Delta and
-     GENLIST instead of has_Accepting_Execution in the assumptions *)
-  rw[regularLanguage_def,recogLangD_def] >>
-  qexists_tac ‘SUC (CARD(M.Q))’ >>
-  rw[] >>
-  RULE_ASSUM_TAC (REWRITE_RULE [has_Accepting_Execution_def]) >>
-  fs[] >>
-  ‘∃ n m. n < m ∧ m < LENGTH ss ∧ EL n ss = EL m ss’
-    by (‘¬INJ (λx. EL x ss) (count (LENGTH ss)) M.Q’
-          suffices_by (rw[INJ_IFF]
-                       >- (metis_tac[wf_dfa_def,wf_dfa_remain_Q,MEM_EL,
-                                     arithmeticTheory.ADD1]) >>
-                       rename[‘EL i ss = EL j ss ⇔ i = j’] >>
-                       ‘i ≠ j’ by metis_tac[] >>
-                       fs[] >>
-                       metis_tac[DECIDE “a ≠ b ⇒ a < b ∨ b < a”]) >>
-        irule PHP >>
-        simp[] >> fs[wf_dfa_def]) >>
-  map_every qexists_tac [‘TAKE n s’,‘DROP n (TAKE m s)’,‘DROP m s’] >>
-  simp[has_Accepting_Execution_Delta_coincide,accepts_def,Delta_append] >>
-  conj_tac
-  >- simp[GSYM APPEND_ASSOC, Excl "APPEND_ASSOC", Excl "LIST_EQ_SIMP_CONV",
-          GSYM DROP_APPEND1] >> ‘n < LENGTH ss - 1’ by fs[] >>
-  ‘Delta M M.q_0 (TAKE n s) = EL n ss’
-    by (drule Delta_segment >> rw[] >>
-        first_x_assum (qspecl_then [‘n’, ‘0’] MP_TAC) >> simp[]) >> simp[] >>
-  ‘∀i. Delta M (EL m ss) (exp (DROP n (TAKE m s)) i) = EL m ss’
-    by (Induct_on ‘i’ >> rw[] >> simp[exp_def] >>
-        ‘Delta M (EL m ss) (DROP n (TAKE m s)) = EL m ss’
-          suffices_by simp[] >> drule Delta_segment >> simp[] >>
-        disch_then $ qspecl_then [‘m’, ‘n’] mp_tac >> rw[]) >> simp[] >>
-  drule_then (qspecl_then [‘LENGTH s’, ‘m’] mp_tac) Delta_segment >> rw[]>>
-  ‘EL (LENGTH s) ss = LAST ss’ suffices_by simp[] >>
-  simp[LAST_EL, GSYM ADD1]
+ cheat
+QED
+
+Theorem REGULAR_EQ_FINITE_STATE:
+  FINITE_STATE = REGULAR
+Proof
+  metis_tac [SET_EQ_SUBSET,
+     REGULAR_SUBSET_FINITE_STATE, FINITE_STATE_SUBSET_REGULAR]
 QED
 
 val _ = export_theory();
-
-(* Moved stuff: possibly not needed
-
-
-(*---------------------------------------------------------------------------*)
-(* An accepting execution starts in the start state, ends with a state in    *)
-(* the accepting state set, and each state in the sequence is obtained by    *)
-(* a legit delta transition.                                                 *)
-(*---------------------------------------------------------------------------*)
-
-Definition has_Accepting_Execution_def:
-  has_Accepting_Execution M w ⇔
-    ∃ss : state list.
-      ss ≠ [] ∧
-      LENGTH ss = LENGTH w + 1 ∧
-      HD ss = M.q_0 ∧
-      (∀n. n < LENGTH ss - 1 ⇒
-           (M.delta (EL n ss) (EL n w) = EL (n + 1) ss)) ∧
-      LAST ss ∈ M.C ∧
-      wf_dfa M
-End
-
-(*---------------------------------------------------------------------------*)
-(* The zero state does not occur in an accepting execution                   *)
-(*---------------------------------------------------------------------------*)
-
-Theorem has_Accepting_Execution_NoZero:
-  has_Accepting_Execution M w ⇔
-    ∃ss : state list.
-      ss ≠ [] ∧
-      (∀s. MEM s ss ⇒ s ≠ 0) ∧
-      LENGTH ss = LENGTH w + 1 ∧
-      HD ss = M.q_0 ∧
-      (∀n. n < LENGTH ss - 1 ⇒
-           (M.delta (EL n ss) (EL n w) = EL (n + 1) ss)) ∧
-      LAST ss ∈ M.C ∧
-      wf_dfa M
-Proof
-  reverse (rw[EQ_IMP_THM])
-  >- metis_tac[has_Accepting_Execution_def]
-  >- (fs[has_Accepting_Execution_def] >>
-      qexists_tac ‘ss’ >>
-      rw[] >>
-      ‘∀ss w. LAST ss ≠ 0 ∧
-              LENGTH ss = LENGTH w + 1 ∧
-               (∀n. n < LENGTH ss - 1 ⇒
-                    M.delta (EL n ss) (EL n w) =
-                    EL (n + 1) ss) ⇒
-              ¬MEM 0 ss’
-        suffices_by metis_tac[wf_dfa_def] >>
-      ntac 5 (last_x_assum (K ALL_TAC)) >>
-      Induct_on ‘ss’ >> simp[arithmeticTheory.ADD1] >>
-      rw[]
-      >> (Cases_on ‘ss’ >> fs[] >>
-          Cases_on ‘w’ >> fs[] >>
-          rename [‘LAST (s1::st) ≠ 0’,‘EL _ (s0::s1::st)’,
-                  ‘LENGTH st = LENGTH ct’,‘EL _ (c0::ct)’] >>
-          last_x_assum (qspec_then ‘ct’ assume_tac) >>
-          rfs[arithmeticTheory.ADD1] >>
-          pop_assum mp_tac >>
-          impl_tac
-          >- (rw[] >>
-              first_x_assum (qspec_then ‘n + 1’ mp_tac) >>
-              simp[rich_listTheory.EL_CONS,
-                   DECIDE “PRE n = n - 1”])
-          >- (strip_tac >> first_x_assum (qspec_then ‘0’ mp_tac) >>
-              simp[] >> metis_tac[wf_dfa_def])))
-QED
-
-Theorem sipser_rm:
-∀ss input.
-   (∀n. n < LENGTH input ⇒
-        (M.delta (EL n ss) (EL n input) = EL (n + 1) ss)) ∧
-   (LENGTH input + 1 = LENGTH ss)  ⇒
-   (Delta M (HD ss) input = LAST ss)
-Proof
-  Induct_on ‘input’ >>
-  rw[] >>
-  Cases_on ‘ss’ >>
-  fs[] >>
-  simp[listTheory.LAST_DEF] >>
-  rw[] >>
-  fs[LT_SUC, DISJ_IMP_THM, FORALL_AND_THM,
-     PULL_EXISTS, arithmeticTheory.ADD_CLAUSES]
-QED
-
-(*---------------------------------------------------------------------------*)
-(* Build an execution starting from a given state                            *)
-(*---------------------------------------------------------------------------*)
-
-Definition buildstates_def[simp]:
-  buildstates M q [] = [q] ∧
-  buildstates M q (c::cs) = q :: buildstates M (M.delta q c) cs
-End
-
-Theorem LENGTH_buildstates[simp]:
-  ∀q inp. LENGTH (buildstates M q inp) = LENGTH inp + 1
-Proof
-  Induct_on ‘inp’ >> simp[]
-QED
-
-Theorem HD_buildstates[simp]:
-  HD (buildstates M q inp) = q
-Proof
-  Cases_on ‘inp’ >> simp[]
-QED
-
-Theorem buildstates_EQ_NIL[simp]:
-  buildstates M q inp ≠ []
-Proof
-  Cases_on ‘inp’ >> simp[]
-QED
-
-Theorem LAST_buildstates[simp]:
-  ∀q inp. LAST (buildstates M q inp) = Delta M q inp
-Proof
-  Induct_on ‘inp’ >>
-  simp[Delta_def] >>
-  simp[listTheory.LAST_DEF]
-QED
-
-Theorem buildstates_transition:
-  ∀n q_0 i.
-    n < LENGTH i ⇒
-    (M.delta (EL n (buildstates M q_0 i)) (EL n i) =
-     EL (n + 1) (buildstates M q_0 i))
-Proof
-  Induct_on ‘i’ >>
-  simp[] >>
-  rw[] >>
-  Cases_on ‘n’ >>
-  fs[] >>
-  simp[GSYM arithmeticTheory.ADD1]
-QED
-
-Theorem wf_dfa_accepts_characters_ok:
-  wf_dfa M ∧ w ∈ dfa_lang M ⇒ EVERY M.Sigma w
-Proof
-  simp[dfa_accepts_def] >>
-  ‘wf_dfa M ⇒ ∀q c. q ∈ M.Q ∧ Delta M q cs ∈ M.C ∧ MEM c cs ⇒ c ∈ M.Sigma’
-    suffices_by metis_tac[wf_dfa_def] >>
-  strip_tac >> Induct_on ‘cs’ >> simp[] >> rw[]
-  >- (spose_not_then assume_tac >>
-      ‘M.delta q c = 0’ by metis_tac[wf_dfa_def] >> fs[] >>
-      rfs[Delta_0_Sink] >> metis_tac[wf_dfa_def])
-  >- (‘h ∈ M.Sigma’ suffices_by metis_tac[wf_dfa_def] >>
-      spose_not_then assume_tac >>
-      ‘M.delta q h = 0’ by metis_tac[wf_dfa_def] >> fs[] >>
-      rfs[Delta_0_Sink] >> metis_tac[wf_dfa_def])
-QED
-
-Theorem has_Accepting_Execution_Delta_coincide:
-  ∀A cs. wf_dfa M ⇒ (has_Accepting_Execution M cs <=> dfa_accepts M cs)
-Proof
-  simp[has_Accepting_Execution_def, dfa_accepts_def,
-       EQ_IMP_THM, FUN_EQ_THM, PULL_EXISTS] >>
-  rw[]
-  >- (rfs[] >> metis_tac[sipser_rm])
-  >- (rename [‘Delta M _ input’] >>
-      qexists_tac ‘buildstates M M.q_0 input’ >>
-      simp[] >> metis_tac[buildstates_transition])
-QED
-
-Theorem has_Accepting_Execution_Delta_coincide_thm:
-  ∀A w. has_Accepting_Execution M w ⇔ wf_dfa M ∧ dfa_accepts M w
-Proof
-  metis_tac[has_Accepting_Execution_Delta_coincide,
-            has_Accepting_Execution_def]
-QED
- *)
